src/FLeXClass.v
@@ -1,36 +1,47 @@
-Require Import Coq.Program.Basics. 
-Require Import Coq.Logic.FunctionalExtensionality. 
-Require Import Coq.Program.Combinators. 
-Require Import FinProof.ProgrammingWith. 
-Require Import String. 
+
  
-Require Import FinProof.ProgrammingWith.
-Require Import FinProof.Types.IsoTypes.
-Require Import FinProof.Common.
-Require Import FinProof.MonadTransformers21.
-Require Import FinProof.StateMonad21.
-Require Import FinProof.EpsilonMonad.
-
-Require Import UMLang.SolidityNotations2.
-Require Import UMLang.SML_NG26.
-Require Import UrsusTVM.tvmFunc.
-
-Local Open Scope record.
-Local Open Scope program_scope. 
-
-Require Import UMLang.ProofEnvironment2.
-
-
-Module LedgerClass (xt: XTypesSig) (sm: StateMonadSig) <: ClassSig xt.
-
-
-Module Export SolidityNotationsClass := SolidityNotations xt  sm.
-Module Export VMStateModule := VMStateModule xt  sm.
-
-Import xt. 
-Existing Instance monadStateT. 
-Existing Instance monadStateStateT.
-
+ Require Import Coq.Program.Basics. 
+ Require Import Coq.Logic.FunctionalExtensionality. 
+ Require Import Coq.Program.Combinators. 
+ Require Import FinProof.ProgrammingWith. 
+ Require Import String. 
+ 
+ Require Import FinProof.ProgrammingWith. 
+ Require Import FinProof.Types.IsoTypes. 
+ Require Import FinProof.Common. 
+ Require Import FinProof.MonadTransformers21. 
+ Require Import FinProof.StateMonad21. 
+ Require Import FinProof.EpsilonMonad. 
+ 
+ Require Import UMLang.SolidityNotations2. 
+ Require Import UMLang.SML_NG26. 
+ Require Import UrsusTVM.tvmFunc. 
+ 
+ Local Open Scope record. 
+ Local Open Scope program_scope. 
+ 
+ Require Import UMLang.ProofEnvironment2. 
+ 
+ 
+ Module LedgerClass (xt: XTypesSig) (sm: StateMonadSig) <: ClassSig xt. 
+ 
+ 
+ Module Export SolidityNotationsClass := SolidityNotations xt sm. 
+ Module Export VMStateModule := VMStateModule xt sm. 
+ 
+ Import xt. 
+ Existing Instance monadStateT. 
+ Existing Instance monadStateStateT. 
+ 
+ Definition IFLeXNotifyPtr := XAddress. 
+ Definition ITONTokenWalletPtr := XAddress. 
+ Definition IPricePtr := XAddress. 
+ Definition TokensType := XInteger128. 
+ Definition WalletGramsType := XInteger128. 
+ Definition Grams := XInteger16 . 
+ Definition auto := XInteger . 
+ Definition addr_std_compact := XAddress . 
+ 
 
 (* 1 *) Inductive TickTockFields := | TickTock_ι_tick | TickTock_ι_tock .
 (* 2 *) Definition TickTock := 
@@ -43,8 +54,6 @@ Existing Instance monadStateStateT.
  XMaybe TvmCell * 
  XMaybe TvmCell * 
  XMaybe TvmCell )%type .
-
-
 (* 1 *) Inductive TonsConfigFields := | TonsConfig_ι_transfer_tip3 | TonsConfig_ι_return_ownership | TonsConfig_ι_trading_pair_deploy | TonsConfig_ι_order_answer | TonsConfig_ι_process_queue | TonsConfig_ι_send_notify .
 (* 2 *) Definition TonsConfig := 
  ( XInteger128 * 
@@ -53,7 +62,7 @@ Existing Instance monadStateStateT.
  XInteger128 * 
  XInteger128 * 
  XInteger128 )%type .
-(* 1 *) Inductive FLeXFields := | FLeX_ι_deployer_pubkey_ | FLeX_ι_tons_cfg_ | FLeX_ι_pair_code_ | FLeX_ι_xchg_pair_code_ | FLeX_ι_price_code_ | FLeX_ι_xchg_price_code_ | FLeX_ι_min_amount_ | FLeX_ι_deals_limit_ | FLeX_ι_notify_addr_ .
+(* 1 *) Inductive FLeXFields := | FLeX_ι_deployer_pubkey_ | FLeX_ι_tons_cfg_ | FLeX_ι_pair_code_ | FLeX_ι_xchg_pair_code_ | FLeX_ι_price_code_ | FLeX_ι_xchg_price_code_ | FLeX_ι_deals_limit_ | FLeX_ι_notify_addr_ .
 (* 2 *) Definition FLeX := 
  ( XInteger256 * 
  TonsConfig * 
@@ -61,8 +70,7 @@ Existing Instance monadStateStateT.
  XMaybe TvmCell * 
  XMaybe TvmCell * 
  XMaybe TvmCell * 
- XInteger128 * 
- XInteger8  * 
+ XInteger8 * 
  XAddress )%type .
 (* 1 *) Inductive TradingPairFields := | TradingPair_ι_flex_addr_ | TradingPair_ι_tip3_root_ | TradingPair_ι_deploy_value_ .
 (* 2 *) Definition TradingPair := 
@@ -75,8 +83,7 @@ Existing Instance monadStateStateT.
  XAddress * 
  XAddress * 
  XInteger128 )%type .
-
-(* 1 *) Inductive LocalStateFields := | LocalState_ι_int | LocalState_ι_optcell | LocalState_ι_tpladdressaddress | LocalState_ι_uint256 | LocalState_ι_uint128 | LocalState_ι_uint8 | LocalState_ι_address | LocalState_ι_cell | LocalState_ι_XchgPair | LocalState_ι_bool | LocalState_ι_TradingPair | LocalState_ι_intIndex | LocalState_ι_optcellIndex | LocalState_ι_tpladdressaddressIndex | LocalState_ι_uint256Index | LocalState_ι_uint128Index | LocalState_ι_uint8Index | LocalState_ι_addressIndex | LocalState_ι_cellIndex | LocalState_ι_XchgPairIndex | LocalState_ι_boolIndex | LocalState_ι_TradingPairIndex .
+(* 1 *) Inductive LocalStateFields := | LocalState_ι_int | LocalState_ι_optcell | LocalState_ι_tpladdressaddress | LocalState_ι_uint256 | LocalState_ι_uint128 | LocalState_ι_uint8 | LocalState_ι_address | LocalState_ι_cell | LocalState_ι_XchgPair | LocalState_ι_bool | LocalState_ι_TradingPair | LocalState_ι_tplStateInituint256 | LocalState_ι_intIndex | LocalState_ι_optcellIndex | LocalState_ι_tpladdressaddressIndex | LocalState_ι_uint256Index | LocalState_ι_uint128Index | LocalState_ι_uint8Index | LocalState_ι_addressIndex | LocalState_ι_cellIndex | LocalState_ι_XchgPairIndex | LocalState_ι_boolIndex | LocalState_ι_TradingPairIndex | LocalState_ι_tplStateInituint256Index .
 (* 2 *) Definition LocalState := 
  ( XHMap (string*nat) XInteger * 
  XHMap (string*nat) ( XMaybe TvmCell ) * 
@@ -89,6 +96,8 @@ Existing Instance monadStateStateT.
  XHMap (string*nat) XchgPair * 
  XHMap (string*nat) XBool * 
  XHMap (string*nat) TradingPair * 
+ XHMap (string*nat) ( StateInit * XInteger256 ) * 
+ XHMap string nat * 
  XHMap string nat * 
  XHMap string nat * 
  XHMap string nat * 
@@ -100,8 +109,6 @@ Existing Instance monadStateStateT.
  XHMap string nat * 
  XHMap string nat * 
  XHMap string nat )%type .
-
-
 (* 1 *) Inductive LedgerFieldsI := | Ledger_ι_FLeX | Ledger_ι_VMState | Ledger_ι_LocalState | Ledger_ι_LocalStateCopy .
 (* 2 *) Definition Ledger := 
  ( FLeX * 
@@ -109,8 +116,8 @@ Existing Instance monadStateStateT.
  LocalState * 
  LocalState )%type .
 
+ Definition LedgerFields := LedgerFieldsI. 
 
-Definition LedgerFields := LedgerFieldsI.
 
 (* 3 *) Definition TickTock_field_type f : Type :=  
 match f with 
@@ -153,10 +160,10 @@ match f with
  let '( r1 , r2 , r3 , r4 , r5 ) := r in 
  match f, v with 
  | StateInit_ι_split_depth , v' => ( v' , r2 , r3 , r4 , r5 ) 
- | StateInit_ι_special , v' =>     ( r1 , v' , r3 , r4 , r5 ) 
- | StateInit_ι_code , v' =>        ( r1 , r2 , v' , r4 , r5 ) 
- | StateInit_ι_data , v' =>        ( r1 , r2 , r3 , v' , r5 ) 
- | StateInit_ι_library , v' =>     ( r1 , r2 , r3 , r4 , v' ) 
+ | StateInit_ι_special , v' => ( r1 , v' , r3 , r4 , r5 ) 
+ | StateInit_ι_code , v' => ( r1 , r2 , v' , r4 , r5 ) 
+ | StateInit_ι_data , v' => ( r1 , r2 , r3 , v' , r5 ) 
+ | StateInit_ι_library , v' => ( r1 , r2 , r3 , r4 , v' ) 
  end .
 (* 7 *) Global Instance StateInit_PruvendoRecord : PruvendoRecord StateInit StateInitFields :=
 {
@@ -164,17 +171,9 @@ match f with
   getPruvendoRecord := @StateInit_get ;
   setPruvendoRecord := @StateInit_set ;
 } .
-
-
 (* 3 *) Definition TonsConfig_field_type f : Type :=  
 match f with 
- | TonsConfig_ι_transfer_tip3 => XInteger128 
- | TonsConfig_ι_return_ownership => XInteger128 
- | TonsConfig_ι_trading_pair_deploy => XInteger128 
- | TonsConfig_ι_order_answer => XInteger128 
- | TonsConfig_ι_process_queue => XInteger128 
- | TonsConfig_ι_send_notify => XInteger128 
-end .
+ | TonsConfig_ι_transfer_tip3 => XInteger128 | TonsConfig_ι_return_ownership => XInteger128 | TonsConfig_ι_trading_pair_deploy => XInteger128 | TonsConfig_ι_order_answer => XInteger128 | TonsConfig_ι_process_queue => XInteger128 | TonsConfig_ι_send_notify => XInteger128 end .
 (* 4 *) Definition TonsConfig_get (f: TonsConfigFields )(r: TonsConfig ) :  TonsConfig_field_type f := 
  let '( r1 , r2 , r3 , r4 , r5 , r6 ) := r in 
  match f with 
@@ -203,12 +202,11 @@ end .
   getPruvendoRecord := @TonsConfig_get ;
   setPruvendoRecord := @TonsConfig_set ;
 } .
-
 (* 3 *) Definition FLeX_field_type f : Type :=  
 match f with 
- | FLeX_ι_deployer_pubkey_ => XInteger256 | FLeX_ι_tons_cfg_ => TonsConfig | FLeX_ι_pair_code_ => XMaybe TvmCell | FLeX_ι_xchg_pair_code_ => XMaybe TvmCell | FLeX_ι_price_code_ => XMaybe TvmCell | FLeX_ι_xchg_price_code_ => XMaybe TvmCell | FLeX_ι_min_amount_ => XInteger128 | FLeX_ι_deals_limit_ => XInteger8 | FLeX_ι_notify_addr_ => XAddress end .
+ | FLeX_ι_deployer_pubkey_ => XInteger256 | FLeX_ι_tons_cfg_ => TonsConfig | FLeX_ι_pair_code_ => XMaybe TvmCell | FLeX_ι_xchg_pair_code_ => XMaybe TvmCell | FLeX_ι_price_code_ => XMaybe TvmCell | FLeX_ι_xchg_price_code_ => XMaybe TvmCell | FLeX_ι_deals_limit_ => XInteger8 | FLeX_ι_notify_addr_ => XAddress end .
 (* 4 *) Definition FLeX_get (f: FLeXFields )(r: FLeX ) :  FLeX_field_type f := 
- let '( r1 , r2 , r3 , r4 , r5 , r6 , r7 , r8 , r9 ) := r in 
+ let '( r1 , r2 , r3 , r4 , r5 , r6 , r7 , r8 ) := r in 
  match f with 
  | FLeX_ι_deployer_pubkey_ => r1 
  | FLeX_ι_tons_cfg_ => r2 
@@ -216,24 +214,22 @@ match f with
  | FLeX_ι_xchg_pair_code_ => r4 
  | FLeX_ι_price_code_ => r5 
  | FLeX_ι_xchg_price_code_ => r6 
- | FLeX_ι_min_amount_ => r7 
- | FLeX_ι_deals_limit_ => r8 
- | FLeX_ι_notify_addr_ => r9 
+ | FLeX_ι_deals_limit_ => r7 
+ | FLeX_ι_notify_addr_ => r8 
  end .
 (* 5 *) Coercion FLeX_get : FLeXFields >-> Funclass .
 (* 6 *) Definition FLeX_set (f: FLeXFields ) 
 (v: FLeX_field_type f) (r: FLeX ): FLeX := 
- let '( r1 , r2 , r3 , r4 , r5 , r6 , r7 , r8 , r9 ) := r in 
+ let '( r1 , r2 , r3 , r4 , r5 , r6 , r7 , r8 ) := r in 
  match f, v with 
- | FLeX_ι_deployer_pubkey_ , v' => ( v' , r2 , r3 , r4 , r5 , r6 , r7 , r8 , r9 ) 
- | FLeX_ι_tons_cfg_ , v' => ( r1 , v' , r3 , r4 , r5 , r6 , r7 , r8 , r9 ) 
- | FLeX_ι_pair_code_ , v' => ( r1 , r2 , v' , r4 , r5 , r6 , r7 , r8 , r9 ) 
- | FLeX_ι_xchg_pair_code_ , v' => ( r1 , r2 , r3 , v' , r5 , r6 , r7 , r8 , r9 ) 
- | FLeX_ι_price_code_ , v' => ( r1 , r2 , r3 , r4 , v' , r6 , r7 , r8 , r9 ) 
- | FLeX_ι_xchg_price_code_ , v' => ( r1 , r2 , r3 , r4 , r5 , v' , r7 , r8 , r9 ) 
- | FLeX_ι_min_amount_ , v' => ( r1 , r2 , r3 , r4 , r5 , r6 , v' , r8 , r9 ) 
- | FLeX_ι_deals_limit_ , v' => ( r1 , r2 , r3 , r4 , r5 , r6 , r7 , v' , r9 ) 
- | FLeX_ι_notify_addr_ , v' => ( r1 , r2 , r3 , r4 , r5 , r6 , r7 , r8 , v' ) 
+ | FLeX_ι_deployer_pubkey_ , v' => ( v' , r2 , r3 , r4 , r5 , r6 , r7 , r8 ) 
+ | FLeX_ι_tons_cfg_ , v' => ( r1 , v' , r3 , r4 , r5 , r6 , r7 , r8 ) 
+ | FLeX_ι_pair_code_ , v' => ( r1 , r2 , v' , r4 , r5 , r6 , r7 , r8 ) 
+ | FLeX_ι_xchg_pair_code_ , v' => ( r1 , r2 , r3 , v' , r5 , r6 , r7 , r8 ) 
+ | FLeX_ι_price_code_ , v' => ( r1 , r2 , r3 , r4 , v' , r6 , r7 , r8 ) 
+ | FLeX_ι_xchg_price_code_ , v' => ( r1 , r2 , r3 , r4 , r5 , v' , r7 , r8 ) 
+ | FLeX_ι_deals_limit_ , v' => ( r1 , r2 , r3 , r4 , r5 , r6 , v' , r8 ) 
+ | FLeX_ι_notify_addr_ , v' => ( r1 , r2 , r3 , r4 , r5 , r6 , r7 , v' ) 
  end .
 (* 7 *) Global Instance FLeX_PruvendoRecord : PruvendoRecord FLeX FLeXFields :=
 {
@@ -241,7 +237,6 @@ match f with
   getPruvendoRecord := @FLeX_get ;
   setPruvendoRecord := @FLeX_set ;
 } .
-
 (* 3 *) Definition TradingPair_field_type f : Type :=  
 match f with 
  | TradingPair_ι_flex_addr_ => XAddress | TradingPair_ι_tip3_root_ => XAddress | TradingPair_ι_deploy_value_ => XInteger128 end .
@@ -267,7 +262,6 @@ match f with
   getPruvendoRecord := @TradingPair_get ;
   setPruvendoRecord := @TradingPair_set ;
 } .
-
 (* 3 *) Definition XchgPair_field_type f : Type :=  
 match f with 
  | XchgPair_ι_flex_addr_ => XAddress | XchgPair_ι_tip3_major_root_ => XAddress | XchgPair_ι_tip3_minor_root_ => XAddress | XchgPair_ι_deploy_value_ => XInteger128 end .
@@ -295,12 +289,11 @@ match f with
   getPruvendoRecord := @XchgPair_get ;
   setPruvendoRecord := @XchgPair_set ;
 } .
-
 (* 3 *) Definition LocalState_field_type f : Type :=  
 match f with 
- | LocalState_ι_int => XHMap (string*nat) XInteger | LocalState_ι_optcell => XHMap (string*nat) ( XMaybe TvmCell ) | LocalState_ι_tpladdressaddress => XHMap (string*nat) ( XAddress * XAddress ) | LocalState_ι_uint256 => XHMap (string*nat) XInteger256 | LocalState_ι_uint128 => XHMap (string*nat) XInteger128 | LocalState_ι_uint8 => XHMap (string*nat) XInteger8 | LocalState_ι_address => XHMap (string*nat) XAddress | LocalState_ι_cell => XHMap (string*nat) TvmCell | LocalState_ι_XchgPair => XHMap (string*nat) XchgPair | LocalState_ι_bool => XHMap (string*nat) XBool | LocalState_ι_TradingPair => XHMap (string*nat) TradingPair | LocalState_ι_intIndex => XHMap string nat | LocalState_ι_optcellIndex => XHMap string nat | LocalState_ι_tpladdressaddressIndex => XHMap string nat | LocalState_ι_uint256Index => XHMap string nat | LocalState_ι_uint128Index => XHMap string nat | LocalState_ι_uint8Index => XHMap string nat | LocalState_ι_addressIndex => XHMap string nat | LocalState_ι_cellIndex => XHMap string nat | LocalState_ι_XchgPairIndex => XHMap string nat | LocalState_ι_boolIndex => XHMap string nat | LocalState_ι_TradingPairIndex => XHMap string nat end .
+ | LocalState_ι_int => XHMap (string*nat) XInteger | LocalState_ι_optcell => XHMap (string*nat) ( XMaybe TvmCell ) | LocalState_ι_tpladdressaddress => XHMap (string*nat) ( XAddress * XAddress ) | LocalState_ι_uint256 => XHMap (string*nat) XInteger256 | LocalState_ι_uint128 => XHMap (string*nat) XInteger128 | LocalState_ι_uint8 => XHMap (string*nat) XInteger8 | LocalState_ι_address => XHMap (string*nat) XAddress | LocalState_ι_cell => XHMap (string*nat) TvmCell | LocalState_ι_XchgPair => XHMap (string*nat) XchgPair | LocalState_ι_bool => XHMap (string*nat) XBool | LocalState_ι_TradingPair => XHMap (string*nat) TradingPair | LocalState_ι_tplStateInituint256 => XHMap (string*nat) ( StateInit * XInteger256 ) | LocalState_ι_intIndex => XHMap string nat | LocalState_ι_optcellIndex => XHMap string nat | LocalState_ι_tpladdressaddressIndex => XHMap string nat | LocalState_ι_uint256Index => XHMap string nat | LocalState_ι_uint128Index => XHMap string nat | LocalState_ι_uint8Index => XHMap string nat | LocalState_ι_addressIndex => XHMap string nat | LocalState_ι_cellIndex => XHMap string nat | LocalState_ι_XchgPairIndex => XHMap string nat | LocalState_ι_boolIndex => XHMap string nat | LocalState_ι_TradingPairIndex => XHMap string nat | LocalState_ι_tplStateInituint256Index => XHMap string nat end .
 (* 4 *) Definition LocalState_get (f: LocalStateFields )(r: LocalState ) :  LocalState_field_type f := 
- let '( r1 , r2 , r3 , r4 , r5 , r6 , r7 , r8 , r9 , r10 , r11 , r12 , r13 , r14 , r15 , r16 , r17 , r18 , r19 , r20 , r21 , r22 ) := r in 
+ let '( r1 , r2 , r3 , r4 , r5 , r6 , r7 , r8 , r9 , r10 , r11 , r12 , r13 , r14 , r15 , r16 , r17 , r18 , r19 , r20 , r21 , r22 , r23 , r24 ) := r in 
  match f with 
  | LocalState_ι_int => r1 
  | LocalState_ι_optcell => r2 
@@ -313,45 +306,49 @@ match f with
  | LocalState_ι_XchgPair => r9 
  | LocalState_ι_bool => r10 
  | LocalState_ι_TradingPair => r11 
- | LocalState_ι_intIndex => r12 
- | LocalState_ι_optcellIndex => r13 
- | LocalState_ι_tpladdressaddressIndex => r14 
- | LocalState_ι_uint256Index => r15 
- | LocalState_ι_uint128Index => r16 
- | LocalState_ι_uint8Index => r17 
- | LocalState_ι_addressIndex => r18 
- | LocalState_ι_cellIndex => r19 
- | LocalState_ι_XchgPairIndex => r20 
- | LocalState_ι_boolIndex => r21 
- | LocalState_ι_TradingPairIndex => r22 
+ | LocalState_ι_tplStateInituint256 => r12 
+ | LocalState_ι_intIndex => r13 
+ | LocalState_ι_optcellIndex => r14 
+ | LocalState_ι_tpladdressaddressIndex => r15 
+ | LocalState_ι_uint256Index => r16 
+ | LocalState_ι_uint128Index => r17 
+ | LocalState_ι_uint8Index => r18 
+ | LocalState_ι_addressIndex => r19 
+ | LocalState_ι_cellIndex => r20 
+ | LocalState_ι_XchgPairIndex => r21 
+ | LocalState_ι_boolIndex => r22 
+ | LocalState_ι_TradingPairIndex => r23 
+ | LocalState_ι_tplStateInituint256Index => r24 
  end .
 (* 5 *) Coercion LocalState_get : LocalStateFields >-> Funclass .
 (* 6 *) Definition LocalState_set (f: LocalStateFields ) 
 (v: LocalState_field_type f) (r: LocalState ): LocalState := 
- let '( r1 , r2 , r3 , r4 , r5 , r6 , r7 , r8 , r9 , r10 , r11 , r12 , r13 , r14 , r15 , r16 , r17 , r18 , r19 , r20 , r21 , r22 ) := r in 
+ let '( r1 , r2 , r3 , r4 , r5 , r6 , r7 , r8 , r9 , r10 , r11 , r12 , r13 , r14 , r15 , r16 , r17 , r18 , r19 , r20 , r21 , r22 , r23 , r24 ) := r in 
  match f, v with 
- | LocalState_ι_int , v' => ( v' , r2 , r3 , r4 , r5 , r6 , r7 , r8 , r9 , r10 , r11 , r12 , r13 , r14 , r15 , r16 , r17 , r18 , r19 , r20 , r21 , r22 ) 
- | LocalState_ι_optcell , v' => ( r1 , v' , r3 , r4 , r5 , r6 , r7 , r8 , r9 , r10 , r11 , r12 , r13 , r14 , r15 , r16 , r17 , r18 , r19 , r20 , r21 , r22 ) 
- | LocalState_ι_tpladdressaddress , v' => ( r1 , r2 , v' , r4 , r5 , r6 , r7 , r8 , r9 , r10 , r11 , r12 , r13 , r14 , r15 , r16 , r17 , r18 , r19 , r20 , r21 , r22 ) 
- | LocalState_ι_uint256 , v' => ( r1 , r2 , r3 , v' , r5 , r6 , r7 , r8 , r9 , r10 , r11 , r12 , r13 , r14 , r15 , r16 , r17 , r18 , r19 , r20 , r21 , r22 ) 
- | LocalState_ι_uint128 , v' => ( r1 , r2 , r3 , r4 , v' , r6 , r7 , r8 , r9 , r10 , r11 , r12 , r13 , r14 , r15 , r16 , r17 , r18 , r19 , r20 , r21 , r22 ) 
- | LocalState_ι_uint8 , v' => ( r1 , r2 , r3 , r4 , r5 , v' , r7 , r8 , r9 , r10 , r11 , r12 , r13 , r14 , r15 , r16 , r17 , r18 , r19 , r20 , r21 , r22 ) 
- | LocalState_ι_address , v' => ( r1 , r2 , r3 , r4 , r5 , r6 , v' , r8 , r9 , r10 , r11 , r12 , r13 , r14 , r15 , r16 , r17 , r18 , r19 , r20 , r21 , r22 ) 
- | LocalState_ι_cell , v' => ( r1 , r2 , r3 , r4 , r5 , r6 , r7 , v' , r9 , r10 , r11 , r12 , r13 , r14 , r15 , r16 , r17 , r18 , r19 , r20 , r21 , r22 ) 
- | LocalState_ι_XchgPair , v' => ( r1 , r2 , r3 , r4 , r5 , r6 , r7 , r8 , v' , r10 , r11 , r12 , r13 , r14 , r15 , r16 , r17 , r18 , r19 , r20 , r21 , r22 ) 
- | LocalState_ι_bool , v' => ( r1 , r2 , r3 , r4 , r5 , r6 , r7 , r8 , r9 , v' , r11 , r12 , r13 , r14 , r15 , r16 , r17 , r18 , r19 , r20 , r21 , r22 ) 
- | LocalState_ι_TradingPair , v' => ( r1 , r2 , r3 , r4 , r5 , r6 , r7 , r8 , r9 , r10 , v' , r12 , r13 , r14 , r15 , r16 , r17 , r18 , r19 , r20 , r21 , r22 ) 
- | LocalState_ι_intIndex , v' => ( r1 , r2 , r3 , r4 , r5 , r6 , r7 , r8 , r9 , r10 , r11 , v' , r13 , r14 , r15 , r16 , r17 , r18 , r19 , r20 , r21 , r22 ) 
- | LocalState_ι_optcellIndex , v' => ( r1 , r2 , r3 , r4 , r5 , r6 , r7 , r8 , r9 , r10 , r11 , r12 , v' , r14 , r15 , r16 , r17 , r18 , r19 , r20 , r21 , r22 ) 
- | LocalState_ι_tpladdressaddressIndex , v' => ( r1 , r2 , r3 , r4 , r5 , r6 , r7 , r8 , r9 , r10 , r11 , r12 , r13 , v' , r15 , r16 , r17 , r18 , r19 , r20 , r21 , r22 ) 
- | LocalState_ι_uint256Index , v' => ( r1 , r2 , r3 , r4 , r5 , r6 , r7 , r8 , r9 , r10 , r11 , r12 , r13 , r14 , v' , r16 , r17 , r18 , r19 , r20 , r21 , r22 ) 
- | LocalState_ι_uint128Index , v' => ( r1 , r2 , r3 , r4 , r5 , r6 , r7 , r8 , r9 , r10 , r11 , r12 , r13 , r14 , r15 , v' , r17 , r18 , r19 , r20 , r21 , r22 ) 
- | LocalState_ι_uint8Index , v' => ( r1 , r2 , r3 , r4 , r5 , r6 , r7 , r8 , r9 , r10 , r11 , r12 , r13 , r14 , r15 , r16 , v' , r18 , r19 , r20 , r21 , r22 ) 
- | LocalState_ι_addressIndex , v' => ( r1 , r2 , r3 , r4 , r5 , r6 , r7 , r8 , r9 , r10 , r11 , r12 , r13 , r14 , r15 , r16 , r17 , v' , r19 , r20 , r21 , r22 ) 
- | LocalState_ι_cellIndex , v' => ( r1 , r2 , r3 , r4 , r5 , r6 , r7 , r8 , r9 , r10 , r11 , r12 , r13 , r14 , r15 , r16 , r17 , r18 , v' , r20 , r21 , r22 ) 
- | LocalState_ι_XchgPairIndex , v' => ( r1 , r2 , r3 , r4 , r5 , r6 , r7 , r8 , r9 , r10 , r11 , r12 , r13 , r14 , r15 , r16 , r17 , r18 , r19 , v' , r21 , r22 ) 
- | LocalState_ι_boolIndex , v' => ( r1 , r2 , r3 , r4 , r5 , r6 , r7 , r8 , r9 , r10 , r11 , r12 , r13 , r14 , r15 , r16 , r17 , r18 , r19 , r20 , v' , r22 ) 
- | LocalState_ι_TradingPairIndex , v' => ( r1 , r2 , r3 , r4 , r5 , r6 , r7 , r8 , r9 , r10 , r11 , r12 , r13 , r14 , r15 , r16 , r17 , r18 , r19 , r20 , r21 , v' ) 
+ | LocalState_ι_int , v' => ( v' , r2 , r3 , r4 , r5 , r6 , r7 , r8 , r9 , r10 , r11 , r12 , r13 , r14 , r15 , r16 , r17 , r18 , r19 , r20 , r21 , r22 , r23 , r24 ) 
+ | LocalState_ι_optcell , v' => ( r1 , v' , r3 , r4 , r5 , r6 , r7 , r8 , r9 , r10 , r11 , r12 , r13 , r14 , r15 , r16 , r17 , r18 , r19 , r20 , r21 , r22 , r23 , r24 ) 
+ | LocalState_ι_tpladdressaddress , v' => ( r1 , r2 , v' , r4 , r5 , r6 , r7 , r8 , r9 , r10 , r11 , r12 , r13 , r14 , r15 , r16 , r17 , r18 , r19 , r20 , r21 , r22 , r23 , r24 ) 
+ | LocalState_ι_uint256 , v' => ( r1 , r2 , r3 , v' , r5 , r6 , r7 , r8 , r9 , r10 , r11 , r12 , r13 , r14 , r15 , r16 , r17 , r18 , r19 , r20 , r21 , r22 , r23 , r24 ) 
+ | LocalState_ι_uint128 , v' => ( r1 , r2 , r3 , r4 , v' , r6 , r7 , r8 , r9 , r10 , r11 , r12 , r13 , r14 , r15 , r16 , r17 , r18 , r19 , r20 , r21 , r22 , r23 , r24 ) 
+ | LocalState_ι_uint8 , v' => ( r1 , r2 , r3 , r4 , r5 , v' , r7 , r8 , r9 , r10 , r11 , r12 , r13 , r14 , r15 , r16 , r17 , r18 , r19 , r20 , r21 , r22 , r23 , r24 ) 
+ | LocalState_ι_address , v' => ( r1 , r2 , r3 , r4 , r5 , r6 , v' , r8 , r9 , r10 , r11 , r12 , r13 , r14 , r15 , r16 , r17 , r18 , r19 , r20 , r21 , r22 , r23 , r24 ) 
+ | LocalState_ι_cell , v' => ( r1 , r2 , r3 , r4 , r5 , r6 , r7 , v' , r9 , r10 , r11 , r12 , r13 , r14 , r15 , r16 , r17 , r18 , r19 , r20 , r21 , r22 , r23 , r24 ) 
+ | LocalState_ι_XchgPair , v' => ( r1 , r2 , r3 , r4 , r5 , r6 , r7 , r8 , v' , r10 , r11 , r12 , r13 , r14 , r15 , r16 , r17 , r18 , r19 , r20 , r21 , r22 , r23 , r24 ) 
+ | LocalState_ι_bool , v' => ( r1 , r2 , r3 , r4 , r5 , r6 , r7 , r8 , r9 , v' , r11 , r12 , r13 , r14 , r15 , r16 , r17 , r18 , r19 , r20 , r21 , r22 , r23 , r24 ) 
+ | LocalState_ι_TradingPair , v' => ( r1 , r2 , r3 , r4 , r5 , r6 , r7 , r8 , r9 , r10 , v' , r12 , r13 , r14 , r15 , r16 , r17 , r18 , r19 , r20 , r21 , r22 , r23 , r24 ) 
+ | LocalState_ι_tplStateInituint256 , v' => ( r1 , r2 , r3 , r4 , r5 , r6 , r7 , r8 , r9 , r10 , r11 , v' , r13 , r14 , r15 , r16 , r17 , r18 , r19 , r20 , r21 , r22 , r23 , r24 ) 
+ | LocalState_ι_intIndex , v' => ( r1 , r2 , r3 , r4 , r5 , r6 , r7 , r8 , r9 , r10 , r11 , r12 , v' , r14 , r15 , r16 , r17 , r18 , r19 , r20 , r21 , r22 , r23 , r24 ) 
+ | LocalState_ι_optcellIndex , v' => ( r1 , r2 , r3 , r4 , r5 , r6 , r7 , r8 , r9 , r10 , r11 , r12 , r13 , v' , r15 , r16 , r17 , r18 , r19 , r20 , r21 , r22 , r23 , r24 ) 
+ | LocalState_ι_tpladdressaddressIndex , v' => ( r1 , r2 , r3 , r4 , r5 , r6 , r7 , r8 , r9 , r10 , r11 , r12 , r13 , r14 , v' , r16 , r17 , r18 , r19 , r20 , r21 , r22 , r23 , r24 ) 
+ | LocalState_ι_uint256Index , v' => ( r1 , r2 , r3 , r4 , r5 , r6 , r7 , r8 , r9 , r10 , r11 , r12 , r13 , r14 , r15 , v' , r17 , r18 , r19 , r20 , r21 , r22 , r23 , r24 ) 
+ | LocalState_ι_uint128Index , v' => ( r1 , r2 , r3 , r4 , r5 , r6 , r7 , r8 , r9 , r10 , r11 , r12 , r13 , r14 , r15 , r16 , v' , r18 , r19 , r20 , r21 , r22 , r23 , r24 ) 
+ | LocalState_ι_uint8Index , v' => ( r1 , r2 , r3 , r4 , r5 , r6 , r7 , r8 , r9 , r10 , r11 , r12 , r13 , r14 , r15 , r16 , r17 , v' , r19 , r20 , r21 , r22 , r23 , r24 ) 
+ | LocalState_ι_addressIndex , v' => ( r1 , r2 , r3 , r4 , r5 , r6 , r7 , r8 , r9 , r10 , r11 , r12 , r13 , r14 , r15 , r16 , r17 , r18 , v' , r20 , r21 , r22 , r23 , r24 ) 
+ | LocalState_ι_cellIndex , v' => ( r1 , r2 , r3 , r4 , r5 , r6 , r7 , r8 , r9 , r10 , r11 , r12 , r13 , r14 , r15 , r16 , r17 , r18 , r19 , v' , r21 , r22 , r23 , r24 ) 
+ | LocalState_ι_XchgPairIndex , v' => ( r1 , r2 , r3 , r4 , r5 , r6 , r7 , r8 , r9 , r10 , r11 , r12 , r13 , r14 , r15 , r16 , r17 , r18 , r19 , r20 , v' , r22 , r23 , r24 ) 
+ | LocalState_ι_boolIndex , v' => ( r1 , r2 , r3 , r4 , r5 , r6 , r7 , r8 , r9 , r10 , r11 , r12 , r13 , r14 , r15 , r16 , r17 , r18 , r19 , r20 , r21 , v' , r23 , r24 ) 
+ | LocalState_ι_TradingPairIndex , v' => ( r1 , r2 , r3 , r4 , r5 , r6 , r7 , r8 , r9 , r10 , r11 , r12 , r13 , r14 , r15 , r16 , r17 , r18 , r19 , r20 , r21 , r22 , v' , r24 ) 
+ | LocalState_ι_tplStateInituint256Index , v' => ( r1 , r2 , r3 , r4 , r5 , r6 , r7 , r8 , r9 , r10 , r11 , r12 , r13 , r14 , r15 , r16 , r17 , r18 , r19 , r20 , r21 , r22 , r23 , v' ) 
  end .
 (* 7 *) Global Instance LocalState_PruvendoRecord : PruvendoRecord LocalState LocalStateFields :=
 {
@@ -359,8 +356,6 @@ match f with
   getPruvendoRecord := @LocalState_get ;
   setPruvendoRecord := @LocalState_set ;
 } .
-
-
 (* 3 *) Definition Ledger_field_type f : Type :=  
 match f with 
  | Ledger_ι_FLeX => FLeX | Ledger_ι_VMState => VMState | Ledger_ι_LocalState => LocalState | Ledger_ι_LocalStateCopy => LocalState end .
@@ -388,19 +383,18 @@ match f with
   getPruvendoRecord := @Ledger_get ;
   setPruvendoRecord := @Ledger_set ;
 } .
-
 Definition T1 := FLeX .
 Definition T2 := VMState .
 Definition T3 := LocalState .
 Definition T4 := LocalState .
 
+ 
  Definition projEmbed_T1 : Ledger -> T1 := getPruvendoRecord (PruvendoRecord := Ledger_PruvendoRecord) Ledger_ι_FLeX. 
  Definition injEmbed_T1 : T1 -> Ledger -> Ledger := setPruvendoRecord (PruvendoRecord := Ledger_PruvendoRecord) Ledger_ι_FLeX. 
-
+ 
  Lemma projinj_T1 : forall ( t : T1 ) ( s : Ledger ), projEmbed_T1 ( injEmbed_T1 t s ) = t . 
  Proof. 
-         intros. destruct s. destruct p. destruct p. compute. 
- auto.
+ intros. destruct s. destruct p. destruct p. compute. auto. 
  Qed. 
  
  Lemma injproj_T1 : forall ( s : Ledger ) , injEmbed_T1 ( projEmbed_T1 s ) s = s . 
@@ -430,7 +424,7 @@ Definition T4 := LocalState .
  projinj := projinj_T1 ; 
  injproj := injproj_T1 ; 
  injinj := injinj_T1 ; 
- } .
+ } . 
  
 
 
@@ -440,7 +434,7 @@ Definition T4 := LocalState .
  
  Lemma projinj_T2 : forall ( t : T2 ) ( s : Ledger ), projEmbed_T2 ( injEmbed_T2 t s ) = t . 
  Proof. 
- intros. destruct s. destruct p. destruct p. auto. 
+ intros. destruct s. destruct p. destruct p. compute. auto. 
  Qed. 
  
  Lemma injproj_T2 : forall ( s : Ledger ) , injEmbed_T2 ( projEmbed_T2 s ) s = s . 
@@ -480,7 +474,7 @@ Definition T4 := LocalState .
  
  Lemma projinj_T3 : forall ( t : T3 ) ( s : Ledger ), projEmbed_T3 ( injEmbed_T3 t s ) = t . 
  Proof. 
- intros. destruct s. destruct p. destruct p. auto. 
+ intros. destruct s. destruct p. destruct p. compute. auto. 
  Qed. 
  
  Lemma injproj_T3 : forall ( s : Ledger ) , injEmbed_T3 ( projEmbed_T3 s ) s = s . 
@@ -520,7 +514,7 @@ Definition T4 := LocalState .
  
  Lemma projinj_T4 : forall ( t : T4 ) ( s : Ledger ), projEmbed_T4 ( injEmbed_T4 t s ) = t . 
  Proof. 
- intros. destruct s. destruct p. destruct p. auto. 
+ intros. destruct s. destruct p. destruct p. compute. auto. 
  Qed. 
  
  Lemma injproj_T4 : forall ( s : Ledger ) , injEmbed_T4 ( projEmbed_T4 s ) s = s . 
@@ -551,13 +545,16 @@ Definition T4 := LocalState .
  injproj := injproj_T4 ; 
  injinj := injinj_T4 ; 
  } . 
+ 
+
+
 
 Lemma injcommute_T1_T2: 
                forall ( u : T2 ) ( t : T1 ) 
                       ( s:Ledger ), 
       ( injEmbed (EmbeddedType:=embeddedT2) u ( injEmbed t s ) ) = ( injEmbed t ( injEmbed (EmbeddedType:=embeddedT2) u s ) ).
 Proof.
- intros. destruct s. destruct p. destruct p. auto.
+ intros. destruct s. destruct p. destruct p. compute.   auto.
 Qed.
 
 Instance InjectCommutableStates_T1_T2 : 
@@ -582,7 +579,7 @@ Lemma injcommute_T1xT2_T3 :
       ( injEmbed (EmbeddedType:=embeddedT3) u ( injEmbed t s ) ) = 
       ( injEmbed t ( injEmbed (EmbeddedType:=embeddedT3) u s ) ).
 Proof.
- intros. destruct s. destruct p. destruct p. auto.
+ intros. destruct s. destruct p. destruct p. compute. auto.
 Qed.
 
 Instance InjectCommutableStates_T1xT2_T3 : 
@@ -607,7 +604,7 @@ Lemma injcommute_T1xT2xT3_T4 :
       ( injEmbed (EmbeddedType:=embeddedT4) u ( injEmbed t s ) ) = 
       ( injEmbed t ( injEmbed (EmbeddedType:=embeddedT4) u s ) ).
 Proof.
- intros. destruct s. destruct p. destruct p. auto.
+ intros. destruct s. destruct p. destruct p. compute. auto.
 Qed.
 
 Instance InjectCommutableStates_T1xT2xT3_T4 : 
@@ -625,22 +622,27 @@ Definition embeddedProduct_T1xT2xT3_T4 :=
 
 Existing Instance embeddedProduct_T1xT2xT3_T4 . 
 
+
+ 
  Lemma fullState_T1xT2xT3_T4 : forall s s0, 
  injEmbed ( T := (((T1 * T2)%xprod * T3)%xprod * T4)%xprod ) 
  ( projEmbed s ) ( injEmbed ( T := T4 ) ( projEmbed s ) s0 ) = s. 
- Proof.
- intros. destruct s. destruct p. destruct p. destruct s0. destruct p. destruct p.
+ Proof. 
+ intros. destruct s. destruct p. destruct p. destruct s0. 
  repeat match goal with 
  | p : _ * _ |- _ => destruct p 
  end. auto. 
  Qed. 
-
-(* Instance FullState_T1xT2xT3_T4 : 
+ 
+ Check FullState. 
+ 
+ (* Instance FullState_T1xT2xT3_T4 : 
  FullState Ledger ((T1 * T2)%xprod * T3)%xprod T4 := 
  { 
  injComm := InjectCommutableStates_T1xT2xT3_T4 ; 
  fullState := fullState_T1xT2xT3_T4 
- } . 
+ } .  *)
+ 
 
 Local Open Scope solidity_scope.
 Notation "'↑ε4' m ":= (liftEmbeddedState ( H := embeddedT4 ) ( ε m )%sol ) (at level 10, left associativity): solidity_scope.
@@ -660,8 +662,8 @@ Notation "'↑↑1' m ":= (liftEmbeddedState ( H := embeddedT1 ) ) (at level 10,
 
 Notation "'↑0' m " := ( liftEmbeddedState ( H :=  embeddedProduct_T1xT2xT3_T4 ) ( m )) (at level 10, left associativity): solidity_scope.
 Notation "'↑↑0'" := ( liftEmbeddedState ( H :=  embeddedProduct_T1xT2xT3_T4 )) (at level 32, left associativity): solidity_scope.
-Notation " ↓ m " := ( callEmbeddedStateAdj m default (H0 :=  FullState_T1xT2xT3_T4 ) ) (at level 31, left associativity): solidity_scope.
- *)Global Instance iso_T1 : IsoTypes T1 (field_type (R:=Ledger) Ledger_ι_FLeX) :=
+(* Notation " ↓ m " := ( callEmbeddedStateAdj m default (H0 :=  FullState_T1xT2xT3_T4 ) ) (at level 31, left associativity): solidity_scope. *)
+Global Instance iso_T1 : IsoTypes T1 (field_type (R:=Ledger) Ledger_ι_FLeX) :=
 {
   x2y := Datatypes.id;
   y2x := Datatypes.id;
@@ -692,19 +694,9 @@ Global Instance iso_T4 : IsoTypes T4 (field_type (R:=Ledger) Ledger_ι_LocalStat
   x2x := eq_refl;
   y2y := eq_refl
 }.
-(****************************************************************************)
 
-Definition  FLeX_ι_tons_cfg_TonsConfig  :
- PruvendoRecord (field_type (R:=FLeX) 
-                 FLeX_ι_tons_cfg_ ) TonsConfigFields := TonsConfig_PruvendoRecord.
 
-Existing Instance FLeX_ι_tons_cfg_TonsConfig.
-
-Existing Instance Ledger_PruvendoRecord.
-
-(****************************************************************************)
-
-(***************************************************************)
+ (* TODO: Тут надо вручную вставлять поля леджера зависящие от полей *) 
 
 Class Countable (X: Type) :=
 {
@@ -788,11 +780,141 @@ Proof.
   reflexivity.
 Defined.
 
+Class LocalStateField (X:Type): Type := 
+{
+    local_index_embedded:> EmbeddedType LedgerLocalState (XHMap string nat) ;
+    local_state_field: LedgerLocalFields;
+    local_field_type_correct: field_type (PruvendoRecord:=LedgerLocalPruvendoRecord) local_state_field = XHMap (string*nat)%type X;
+}.
+
 
 (****************************************************************************)
+Definition  LocalState_ι_intIndex_Embedded_projEmbed (l:LedgerLocalState ) : XHMap string nat := 
+  LocalState_ι_intIndex l.
+
+Definition  LocalState_ι_intIndex_Embedded_injEmbed (m: XHMap string nat) (l: LedgerLocalState) : LedgerLocalState := 
+  {$$ l with  LocalState_ι_intIndex := m $$}.
+
+Print EmbeddedType.  
+
+Lemma LocalState_ι_intIndex_Embedded_projinj : forall (t : XHMap string nat) (s : LedgerLocalState), LocalState_ι_intIndex_Embedded_projEmbed (LocalState_ι_intIndex_Embedded_injEmbed t s) = t.
+Proof.
+  intros.
+  destruct s.
+  repeat destruct p.
+  reflexivity.
+Defined.
+
+Lemma LocalState_ι_intIndex_Embedded_injproj : forall s : LedgerLocalState, LocalState_ι_intIndex_Embedded_injEmbed (LocalState_ι_intIndex_Embedded_projEmbed s) s = s.
+Proof.
+  intros.
+  destruct s.
+  repeat destruct p.
+  reflexivity.
+Defined.  
+
+Lemma LocalState_ι_intIndex_Embedded_injinj : forall (t1 t2 : XHMap string nat) (s : LedgerLocalState),
+LocalState_ι_intIndex_Embedded_injEmbed t1 (LocalState_ι_intIndex_Embedded_injEmbed t2 s) = LocalState_ι_intIndex_Embedded_injEmbed t1 s.
+Proof.
+  intros.
+  destruct s.
+  repeat destruct p.
+  reflexivity.
+Defined.
 
 
+Global Instance LocalState_ι_intIndex_Embedded : EmbeddedType LedgerLocalState (XHMap string nat) :=
+{
+  projEmbed := LocalState_ι_intIndex_Embedded_projEmbed;
+	injEmbed := LocalState_ι_intIndex_Embedded_injEmbed;
+  projinj := LocalState_ι_intIndex_Embedded_projinj;
+  injproj := LocalState_ι_intIndex_Embedded_injproj;
+  injinj := LocalState_ι_intIndex_Embedded_injinj
+}.
+Definition  LocalState_ι_optcellIndex_Embedded_projEmbed (l:LedgerLocalState ) : XHMap string nat := 
+  LocalState_ι_optcellIndex l.
 
+Definition  LocalState_ι_optcellIndex_Embedded_injEmbed (m: XHMap string nat) (l: LedgerLocalState) : LedgerLocalState := 
+  {$$ l with  LocalState_ι_optcellIndex := m $$}.
+
+Print EmbeddedType.  
+
+Lemma LocalState_ι_optcellIndex_Embedded_projinj : forall (t : XHMap string nat) (s : LedgerLocalState), LocalState_ι_optcellIndex_Embedded_projEmbed (LocalState_ι_optcellIndex_Embedded_injEmbed t s) = t.
+Proof.
+  intros.
+  destruct s.
+  repeat destruct p.
+  reflexivity.
+Defined.
+
+Lemma LocalState_ι_optcellIndex_Embedded_injproj : forall s : LedgerLocalState, LocalState_ι_optcellIndex_Embedded_injEmbed (LocalState_ι_optcellIndex_Embedded_projEmbed s) s = s.
+Proof.
+  intros.
+  destruct s.
+  repeat destruct p.
+  reflexivity.
+Defined.  
+
+Lemma LocalState_ι_optcellIndex_Embedded_injinj : forall (t1 t2 : XHMap string nat) (s : LedgerLocalState),
+LocalState_ι_optcellIndex_Embedded_injEmbed t1 (LocalState_ι_optcellIndex_Embedded_injEmbed t2 s) = LocalState_ι_optcellIndex_Embedded_injEmbed t1 s.
+Proof.
+  intros.
+  destruct s.
+  repeat destruct p.
+  reflexivity.
+Defined.
+
+
+Global Instance LocalState_ι_optcellIndex_Embedded : EmbeddedType LedgerLocalState (XHMap string nat) :=
+{
+  projEmbed := LocalState_ι_optcellIndex_Embedded_projEmbed;
+	injEmbed := LocalState_ι_optcellIndex_Embedded_injEmbed;
+  projinj := LocalState_ι_optcellIndex_Embedded_projinj;
+  injproj := LocalState_ι_optcellIndex_Embedded_injproj;
+  injinj := LocalState_ι_optcellIndex_Embedded_injinj
+}.
+Definition  LocalState_ι_tpladdressaddressIndex_Embedded_projEmbed (l:LedgerLocalState ) : XHMap string nat := 
+  LocalState_ι_tpladdressaddressIndex l.
+
+Definition  LocalState_ι_tpladdressaddressIndex_Embedded_injEmbed (m: XHMap string nat) (l: LedgerLocalState) : LedgerLocalState := 
+  {$$ l with  LocalState_ι_tpladdressaddressIndex := m $$}.
+
+Print EmbeddedType.  
+
+Lemma LocalState_ι_tpladdressaddressIndex_Embedded_projinj : forall (t : XHMap string nat) (s : LedgerLocalState), LocalState_ι_tpladdressaddressIndex_Embedded_projEmbed (LocalState_ι_tpladdressaddressIndex_Embedded_injEmbed t s) = t.
+Proof.
+  intros.
+  destruct s.
+  repeat destruct p.
+  reflexivity.
+Defined.
+
+Lemma LocalState_ι_tpladdressaddressIndex_Embedded_injproj : forall s : LedgerLocalState, LocalState_ι_tpladdressaddressIndex_Embedded_injEmbed (LocalState_ι_tpladdressaddressIndex_Embedded_projEmbed s) s = s.
+Proof.
+  intros.
+  destruct s.
+  repeat destruct p.
+  reflexivity.
+Defined.  
+
+Lemma LocalState_ι_tpladdressaddressIndex_Embedded_injinj : forall (t1 t2 : XHMap string nat) (s : LedgerLocalState),
+LocalState_ι_tpladdressaddressIndex_Embedded_injEmbed t1 (LocalState_ι_tpladdressaddressIndex_Embedded_injEmbed t2 s) = LocalState_ι_tpladdressaddressIndex_Embedded_injEmbed t1 s.
+Proof.
+  intros.
+  destruct s.
+  repeat destruct p.
+  reflexivity.
+Defined.
+
+
+Global Instance LocalState_ι_tpladdressaddressIndex_Embedded : EmbeddedType LedgerLocalState (XHMap string nat) :=
+{
+  projEmbed := LocalState_ι_tpladdressaddressIndex_Embedded_projEmbed;
+	injEmbed := LocalState_ι_tpladdressaddressIndex_Embedded_injEmbed;
+  projinj := LocalState_ι_tpladdressaddressIndex_Embedded_projinj;
+  injproj := LocalState_ι_tpladdressaddressIndex_Embedded_injproj;
+  injinj := LocalState_ι_tpladdressaddressIndex_Embedded_injinj
+}.
 Definition  LocalState_ι_uint256Index_Embedded_projEmbed (l:LedgerLocalState ) : XHMap string nat := 
   LocalState_ι_uint256Index l.
 
@@ -961,49 +1083,6 @@ Global Instance LocalState_ι_addressIndex_Embedded : EmbeddedType LedgerLocalSt
   injproj := LocalState_ι_addressIndex_Embedded_injproj;
   injinj := LocalState_ι_addressIndex_Embedded_injinj
 }.
-
-Definition  LocalState_ι_TradingPairIndex_Embedded_projEmbed (l:LedgerLocalState ) : XHMap string nat := 
-  LocalState_ι_TradingPairIndex l.
-
-Definition  LocalState_ι_TradingPairIndex_Embedded_injEmbed (m: XHMap string nat) (l: LedgerLocalState) : LedgerLocalState := 
-  {$$ l with  LocalState_ι_TradingPairIndex := m $$}.
-
-Print EmbeddedType.  
-
-Lemma LocalState_ι_TradingPairIndex_Embedded_projinj : forall (t : XHMap string nat) (s : LedgerLocalState), LocalState_ι_TradingPairIndex_Embedded_projEmbed (LocalState_ι_TradingPairIndex_Embedded_injEmbed t s) = t.
-Proof.
-  intros.
-  destruct s.
-  repeat destruct p.
-  reflexivity.
-Defined.
-
-Lemma LocalState_ι_TradingPairIndex_Embedded_injproj : forall s : LedgerLocalState, LocalState_ι_TradingPairIndex_Embedded_injEmbed (LocalState_ι_TradingPairIndex_Embedded_projEmbed s) s = s.
-Proof.
-  intros.
-  destruct s.
-  repeat destruct p.
-  reflexivity.
-Defined.  
-
-Lemma LocalState_ι_TradingPairIndex_Embedded_injinj : forall (t1 t2 : XHMap string nat) (s : LedgerLocalState),
-LocalState_ι_TradingPairIndex_Embedded_injEmbed t1 (LocalState_ι_TradingPairIndex_Embedded_injEmbed t2 s) = LocalState_ι_TradingPairIndex_Embedded_injEmbed t1 s.
-Proof.
-  intros.
-  destruct s.
-  repeat destruct p.
-  reflexivity.
-Defined.
-
-
-Global Instance LocalState_ι_TradingPairIndex_Embedded : EmbeddedType LedgerLocalState (XHMap string nat) :=
-{
-  projEmbed := LocalState_ι_TradingPairIndex_Embedded_projEmbed;
-	injEmbed := LocalState_ι_TradingPairIndex_Embedded_injEmbed;
-  projinj := LocalState_ι_TradingPairIndex_Embedded_projinj;
-  injproj := LocalState_ι_TradingPairIndex_Embedded_injproj;
-  injinj := LocalState_ι_TradingPairIndex_Embedded_injinj
-}.
 Definition  LocalState_ι_cellIndex_Embedded_projEmbed (l:LedgerLocalState ) : XHMap string nat := 
   LocalState_ι_cellIndex l.
 
@@ -1088,10 +1167,6 @@ Global Instance LocalState_ι_XchgPairIndex_Embedded : EmbeddedType LedgerLocalS
   injproj := LocalState_ι_XchgPairIndex_Embedded_injproj;
   injinj := LocalState_ι_XchgPairIndex_Embedded_injinj
 }.
-
-
-
-
 Definition  LocalState_ι_boolIndex_Embedded_projEmbed (l:LedgerLocalState ) : XHMap string nat := 
   LocalState_ι_boolIndex l.
 
@@ -1100,9 +1175,7 @@ Definition  LocalState_ι_boolIndex_Embedded_injEmbed (m: XHMap string nat) (l: 
 
 Print EmbeddedType.  
 
-Lemma LocalState_ι_boolIndex_Embedded_projinj : 
-              forall (t : XHMap string nat) (s : LedgerLocalState), 
-              LocalState_ι_boolIndex_Embedded_projEmbed (LocalState_ι_boolIndex_Embedded_injEmbed t s) = t.
+Lemma LocalState_ι_boolIndex_Embedded_projinj : forall (t : XHMap string nat) (s : LedgerLocalState), LocalState_ι_boolIndex_Embedded_projEmbed (LocalState_ι_boolIndex_Embedded_injEmbed t s) = t.
 Proof.
   intros.
   destruct s.
@@ -1110,8 +1183,7 @@ Proof.
   reflexivity.
 Defined.
 
-Lemma LocalState_ι_boolIndex_Embedded_injproj : forall s : LedgerLocalState, 
-                      LocalState_ι_boolIndex_Embedded_injEmbed (LocalState_ι_boolIndex_Embedded_projEmbed s) s = s.
+Lemma LocalState_ι_boolIndex_Embedded_injproj : forall s : LedgerLocalState, LocalState_ι_boolIndex_Embedded_injEmbed (LocalState_ι_boolIndex_Embedded_projEmbed s) s = s.
 Proof.
   intros.
   destruct s.
@@ -1137,15 +1209,15 @@ Global Instance LocalState_ι_boolIndex_Embedded : EmbeddedType LedgerLocalState
   injproj := LocalState_ι_boolIndex_Embedded_injproj;
   injinj := LocalState_ι_boolIndex_Embedded_injinj
 }.
+Definition  LocalState_ι_TradingPairIndex_Embedded_projEmbed (l:LedgerLocalState ) : XHMap string nat := 
+  LocalState_ι_TradingPairIndex l.
 
+Definition  LocalState_ι_TradingPairIndex_Embedded_injEmbed (m: XHMap string nat) (l: LedgerLocalState) : LedgerLocalState := 
+  {$$ l with  LocalState_ι_TradingPairIndex := m $$}.
 
-Definition  LocalState_ι_optcellIndex_Embedded_projEmbed (l:LedgerLocalState ) : XHMap string nat := 
-  LocalState_ι_optcellIndex l.
+Print EmbeddedType.  
 
-Definition  LocalState_ι_optcellIndex_Embedded_injEmbed (m: XHMap string nat) (l: LedgerLocalState) : LedgerLocalState := 
-  {$$ l with  LocalState_ι_optcellIndex := m $$}.
-
-Lemma LocalState_ι_optcellIndex_Embedded_projinj : forall (t : XHMap string nat) (s : LedgerLocalState), LocalState_ι_optcellIndex_Embedded_projEmbed (LocalState_ι_optcellIndex_Embedded_injEmbed t s) = t.
+Lemma LocalState_ι_TradingPairIndex_Embedded_projinj : forall (t : XHMap string nat) (s : LedgerLocalState), LocalState_ι_TradingPairIndex_Embedded_projEmbed (LocalState_ι_TradingPairIndex_Embedded_injEmbed t s) = t.
 Proof.
   intros.
   destruct s.
@@ -1153,7 +1225,7 @@ Proof.
   reflexivity.
 Defined.
 
-Lemma LocalState_ι_optcellIndex_Embedded_injproj : forall s : LedgerLocalState, LocalState_ι_optcellIndex_Embedded_injEmbed (LocalState_ι_optcellIndex_Embedded_projEmbed s) s = s.
+Lemma LocalState_ι_TradingPairIndex_Embedded_injproj : forall s : LedgerLocalState, LocalState_ι_TradingPairIndex_Embedded_injEmbed (LocalState_ι_TradingPairIndex_Embedded_projEmbed s) s = s.
 Proof.
   intros.
   destruct s.
@@ -1161,8 +1233,8 @@ Proof.
   reflexivity.
 Defined.  
 
-Lemma LocalState_ι_optcellIndex_Embedded_injinj : forall (t1 t2 : XHMap string nat) (s : LedgerLocalState),
-LocalState_ι_optcellIndex_Embedded_injEmbed t1 (LocalState_ι_optcellIndex_Embedded_injEmbed t2 s) = LocalState_ι_optcellIndex_Embedded_injEmbed t1 s.
+Lemma LocalState_ι_TradingPairIndex_Embedded_injinj : forall (t1 t2 : XHMap string nat) (s : LedgerLocalState),
+LocalState_ι_TradingPairIndex_Embedded_injEmbed t1 (LocalState_ι_TradingPairIndex_Embedded_injEmbed t2 s) = LocalState_ι_TradingPairIndex_Embedded_injEmbed t1 s.
 Proof.
   intros.
   destruct s.
@@ -1171,116 +1243,168 @@ Proof.
 Defined.
 
 
-Global Instance LocalState_ι_optcellIndex_Embedded : EmbeddedType LedgerLocalState (XHMap string nat) :=
+Global Instance LocalState_ι_TradingPairIndex_Embedded : EmbeddedType LedgerLocalState (XHMap string nat) :=
 {
-  projEmbed := LocalState_ι_optcellIndex_Embedded_projEmbed;
-	injEmbed := LocalState_ι_optcellIndex_Embedded_injEmbed;
-  projinj := LocalState_ι_optcellIndex_Embedded_projinj;
-  injproj := LocalState_ι_optcellIndex_Embedded_injproj;
-  injinj := LocalState_ι_optcellIndex_Embedded_injinj
+  projEmbed := LocalState_ι_TradingPairIndex_Embedded_projEmbed;
+	injEmbed := LocalState_ι_TradingPairIndex_Embedded_injEmbed;
+  projinj := LocalState_ι_TradingPairIndex_Embedded_projinj;
+  injproj := LocalState_ι_TradingPairIndex_Embedded_injproj;
+  injinj := LocalState_ι_TradingPairIndex_Embedded_injinj
 }.
+Definition  LocalState_ι_tplStateInituint256Index_Embedded_projEmbed (l:LedgerLocalState ) : XHMap string nat := 
+  LocalState_ι_tplStateInituint256Index l.
 
+Definition  LocalState_ι_tplStateInituint256Index_Embedded_injEmbed (m: XHMap string nat) (l: LedgerLocalState) : LedgerLocalState := 
+  {$$ l with  LocalState_ι_tplStateInituint256Index := m $$}.
+
+Print EmbeddedType.  
+
+Lemma LocalState_ι_tplStateInituint256Index_Embedded_projinj : forall (t : XHMap string nat) (s : LedgerLocalState), LocalState_ι_tplStateInituint256Index_Embedded_projEmbed (LocalState_ι_tplStateInituint256Index_Embedded_injEmbed t s) = t.
+Proof.
+  intros.
+  destruct s.
+  repeat destruct p.
+  reflexivity.
+Defined.
+
+Lemma LocalState_ι_tplStateInituint256Index_Embedded_injproj : forall s : LedgerLocalState, LocalState_ι_tplStateInituint256Index_Embedded_injEmbed (LocalState_ι_tplStateInituint256Index_Embedded_projEmbed s) s = s.
+Proof.
+  intros.
+  destruct s.
+  repeat destruct p.
+  reflexivity.
+Defined.  
+
+Lemma LocalState_ι_tplStateInituint256Index_Embedded_injinj : forall (t1 t2 : XHMap string nat) (s : LedgerLocalState),
+LocalState_ι_tplStateInituint256Index_Embedded_injEmbed t1 (LocalState_ι_tplStateInituint256Index_Embedded_injEmbed t2 s) = LocalState_ι_tplStateInituint256Index_Embedded_injEmbed t1 s.
+Proof.
+  intros.
+  destruct s.
+  repeat destruct p.
+  reflexivity.
+Defined.
+
+
+Global Instance LocalState_ι_tplStateInituint256Index_Embedded : EmbeddedType LedgerLocalState (XHMap string nat) :=
+{
+  projEmbed := LocalState_ι_tplStateInituint256Index_Embedded_projEmbed;
+	injEmbed := LocalState_ι_tplStateInituint256Index_Embedded_injEmbed;
+  projinj := LocalState_ι_tplStateInituint256Index_Embedded_projinj;
+  injproj := LocalState_ι_tplStateInituint256Index_Embedded_injproj;
+  injinj := LocalState_ι_tplStateInituint256Index_Embedded_injinj
+}.
 (****************************************************************************)
 
-Class LocalStateField (X:Type): Type := 
+Global Instance LocalState_intIndex: LocalStateField XInteger :=
 {
-    local_index_embedded:> EmbeddedType LedgerLocalState (XHMap string nat) ;
-    local_state_field: LedgerLocalFields;
-    local_field_type_correct: field_type (PruvendoRecord:=LedgerLocalPruvendoRecord) local_state_field = XHMap (string*nat)%type X;
+  local_index_embedded := LocalState_ι_intIndex_Embedded;
+  local_state_field := LocalState_ι_int; 
+  local_field_type_correct := eq_refl
 }.
 
-Global Instance LocalState_optcellIndex: LocalStateField (XMaybe TvmCell) :=
+ 
+ 
+Global Instance LocalState_optcellIndex: LocalStateField ( XMaybe TvmCell ) :=
 {
   local_index_embedded := LocalState_ι_optcellIndex_Embedded;
   local_state_field := LocalState_ι_optcell; 
   local_field_type_correct := eq_refl
 }.
 
+ 
+ 
+Global Instance LocalState_tpladdressaddressIndex: LocalStateField ( XAddress * XAddress ) :=
+{
+  local_index_embedded := LocalState_ι_tpladdressaddressIndex_Embedded;
+  local_state_field := LocalState_ι_tpladdressaddress; 
+  local_field_type_correct := eq_refl
+}.
 
-(* 
-(* Global Instance LocalState_ι_uint256Index: LocalStateField XInteger256 :=
+ 
+ 
+Global Instance LocalState_uint256Index: LocalStateField XInteger256 :=
 {
   local_index_embedded := LocalState_ι_uint256Index_Embedded;
   local_state_field := LocalState_ι_uint256; 
   local_field_type_correct := eq_refl
 }.
- *)
 
-*)
-(* 
-Global Instance LocalState_ι_cellIndex: LocalStateField TvmCell :=
-{
-  local_index_embedded := LocalState_ι_cellIndex_Embedded;
-  local_state_field := LocalState_ι_cell; 
-  local_field_type_correct := eq_refl
-}. *)
-
-(*
-
-Global Instance LocalState_ι_uint8Index: LocalStateField XInteger8 :=
-{
-  local_index_embedded := LocalState_ι_uint8Index_Embedded;
-  local_state_field := LocalState_ι_uint8; 
-  local_field_type_correct := eq_refl
-}.
-
-
-
-Global Instance LocalState_ι_addressIndex: LocalStateField XAddress :=
-{
-  local_index_embedded := LocalState_ι_addressIndex_Embedded;
-  local_state_field := LocalState_ι_address; 
-  local_field_type_correct := eq_refl
-}.
-
-
-
-Global Instance LocalState_ι_uint128Index: LocalStateField XInteger128 :=
+ 
+ 
+Global Instance LocalState_uint128Index: LocalStateField XInteger128 :=
 {
   local_index_embedded := LocalState_ι_uint128Index_Embedded;
   local_state_field := LocalState_ι_uint128; 
   local_field_type_correct := eq_refl
 }.
 
-Global Instance LocalState_ι_DTradingPairIndex : LocalStateField TradingPair :=
-{
-  local_index_embedded := LocalState_ι_DTradingPairIndex_Embedded;
-  local_state_field := LocalState_ι_DTradingPair; 
-  local_field_type_correct := eq_refl
-}.
-
-
-Global Instance LocalState_ι_DXchgPairIndex: LocalStateField XchgPair :=
-{
-  local_index_embedded := LocalState_ι_DXchgPairIndex_Embedded;
-  local_state_field := LocalState_ι_DXchgPair; 
-  local_field_type_correct := eq_refl
-}. *)
-
-Global Instance LocalStateField_XInteger: LocalStateField XInteger8 :=
+ 
+ 
+Global Instance LocalState_uint8Index: LocalStateField XInteger8 :=
 {
   local_index_embedded := LocalState_ι_uint8Index_Embedded;
   local_state_field := LocalState_ι_uint8; 
   local_field_type_correct := eq_refl
 }.
 
-Global Instance LocalStateField_XBool: LocalStateField XBool :=
+ 
+ 
+Global Instance LocalState_addressIndex: LocalStateField XAddress :=
 {
-  local_index_embedded := LocalState_ι_boolIndex_Embedded;
-  local_state_field := LocalState_ι_bool; 
+  local_index_embedded := LocalState_ι_addressIndex_Embedded;
+  local_state_field := LocalState_ι_address; 
   local_field_type_correct := eq_refl
 }.
 
-Global Instance LocalStateField_TvmCell : LocalStateField TvmCell :=
+ 
+ 
+Global Instance LocalState_cellIndex: LocalStateField TvmCell :=
 {
   local_index_embedded := LocalState_ι_cellIndex_Embedded;
   local_state_field := LocalState_ι_cell; 
   local_field_type_correct := eq_refl
 }.
 
+ 
+ 
+Global Instance LocalState_XchgPairIndex: LocalStateField XchgPair :=
+{
+  local_index_embedded := LocalState_ι_XchgPairIndex_Embedded;
+  local_state_field := LocalState_ι_XchgPair; 
+  local_field_type_correct := eq_refl
+}.
+
+ 
+ 
+Global Instance LocalState_boolIndex: LocalStateField XBool :=
+{
+  local_index_embedded := LocalState_ι_boolIndex_Embedded;
+  local_state_field := LocalState_ι_bool; 
+  local_field_type_correct := eq_refl
+}.
+
+ 
+ 
+Global Instance LocalState_TradingPairIndex: LocalStateField TradingPair :=
+{
+  local_index_embedded := LocalState_ι_TradingPairIndex_Embedded;
+  local_state_field := LocalState_ι_TradingPair; 
+  local_field_type_correct := eq_refl
+}.
+
+ 
+ 
+Global Instance LocalState_tplStateInituint256Index: LocalStateField ( StateInit * XInteger256 ) :=
+{
+  local_index_embedded := LocalState_ι_tplStateInituint256Index_Embedded;
+  local_state_field := LocalState_ι_tplStateInituint256; 
+  local_field_type_correct := eq_refl
+}.
+
+ 
+
 Definition LedgerVMStateEmbedded := embeddedT2. 
 Definition LedgerVMStateField := Ledger_ι_VMState .
 Definition isoVMState := iso_T2.
-
 
 End LedgerClass .
