src/FLeXClientClass.v
@@ -1,0 +1,2570 @@
+ Require Import Coq.Program.Basics. 
+ Require Import Coq.Logic.FunctionalExtensionality. 
+ Require Import Coq.Program.Combinators. 
+ Require Import FinProof.ProgrammingWith. 
+ Require Import String. 
+ 
+ Require Import FinProof.ProgrammingWith. 
+ Require Import FinProof.Types.IsoTypes. 
+ Require Import FinProof.Common. 
+ Require Import FinProof.MonadTransformers21. 
+ Require Import FinProof.StateMonad21. 
+ Require Import FinProof.EpsilonMonad. 
+ 
+ Require Import UMLang.SolidityNotations2. 
+ Require Import UMLang.SML_NG26. 
+ Require Import UrsusTVM.tvmFunc. 
+ 
+ Local Open Scope record. 
+ Local Open Scope program_scope. 
+ 
+ Require Import UMLang.ProofEnvironment2. 
+ 
+ 
+ Module LedgerClass (xt: XTypesSig) (sm: StateMonadSig) <: ClassSig xt. 
+ 
+ 
+ Module Export SolidityNotationsClass := SolidityNotations xt sm. 
+ Module Export VMStateModule := VMStateModule xt sm. 
+ 
+ Import xt. 
+ Existing Instance monadStateT. 
+ Existing Instance monadStateStateT. 
+ 
+ Definition IFLeXNotifyPtr := XAddress. 
+ Definition ITONTokenWalletPtr := XAddress. 
+ Definition IPricePtr := XAddress. 
+ Definition TokensType := XInteger128. 
+ Definition WalletGramsType := XInteger128. 
+ Definition Grams := XInteger16 . 
+ Definition auto := XInteger . 
+ Definition addr_std_compact := XAddress . 
+Definition varuint32 := XInteger32 .
+ 
+
+(* 1 *) Inductive TickTockFields := | TickTock_ι_tick | TickTock_ι_tock .
+(* 2 *) Definition TickTock := 
+ ( XBool * 
+ XBool )%type .
+(* 1 *) Inductive StateInitFields := | StateInit_ι_split_depth | StateInit_ι_special | StateInit_ι_code | StateInit_ι_data | StateInit_ι_library .
+(* 2 *) Definition StateInit := 
+ ( XMaybe XInteger * 
+ XMaybe TickTock * 
+ XMaybe TvmCell * 
+ XMaybe TvmCell * 
+ XMaybe TvmCell )%type .
+(* 1 *) Inductive anycast_infoFields := | anycast_info_ι_rewrite_pfx .
+(* 2 *) Definition anycast_info := 
+ ( varuint32 )%type .
+(* 1 *) Inductive addr_stdFields := | addr_std_ι_kind | addr_std_ι_Anycast | addr_std_ι_workchain_id | addr_std_ι_address .
+(* 2 *) Definition addr_std := 
+ ( XInteger * 
+ XMaybe anycast_info * 
+ XInteger8 * 
+ XInteger256 )%type .
+(* 1 *) Inductive addr_std_fixedFields := | addr_std_fixed_ι_workchain_id | addr_std_fixed_ι_address .
+(* 2 *) Definition addr_std_fixed := 
+ ( XInteger8 * 
+ XInteger256 )%type .
+(* 1 *) Inductive SellArgsFields := | SellArgs_ι_amount | SellArgs_ι_receive_wallet .
+(* 2 *) Definition SellArgs := 
+ ( XInteger128 * 
+ addr_std_fixed )%type .
+(* 1 *) Inductive FlexBurnWalletArgsFields := | FlexBurnWalletArgs_ι_tons_value | FlexBurnWalletArgs_ι_out_pubkey | FlexBurnWalletArgs_ι_out_internal_owner | FlexBurnWalletArgs_ι_my_tip3_addr .
+(* 2 *) Definition FlexBurnWalletArgs := 
+ ( XInteger128 * 
+ XInteger256 * 
+ XAddress * 
+ XAddress )%type .
+(* 1 *) Inductive TonsConfigFields := | TonsConfig_ι_transfer_tip3 | TonsConfig_ι_return_ownership | TonsConfig_ι_trading_pair_deploy | TonsConfig_ι_order_answer | TonsConfig_ι_process_queue | TonsConfig_ι_send_notify .
+(* 2 *) Definition TonsConfig := 
+ ( XInteger128 * 
+ XInteger128 * 
+ XInteger128 * 
+ XInteger128 * 
+ XInteger128 * 
+ XInteger128 )%type .
+(* 1 *) Inductive FLeXClientFields := | FLeXClient_ι_owner_ | FLeXClient_ι_trading_pair_code_ | FLeXClient_ι_xchg_pair_code_ | FLeXClient_ι_workchain_id_ | FLeXClient_ι_tons_cfg_ | FLeXClient_ι_flex_ | FLeXClient_ι_notify_addr_ | FLeXClient_ι_ext_wallet_code_ | FLeXClient_ι_flex_wallet_code_ | FLeXClient_ι_flex_wrapper_code_ .
+(* 2 *) Definition FLeXClient := 
+ ( XInteger256 * 
+ TvmCell * 
+ TvmCell * 
+ XInteger8 * 
+ TonsConfig * 
+ addr_std_compact * 
+ addr_std_compact * 
+ XMaybe TvmCell * 
+ XMaybe TvmCell * 
+ XMaybe TvmCell )%type .
+(* 1 *) Inductive FLeXSellArgsAddrsFields := | FLeXSellArgsAddrs_ι_my_tip3_addr .
+(* 2 *) Definition FLeXSellArgsAddrs := 
+ ( XAddress )%type .
+(* 1 *) Inductive FLeXSellArgsFields := | FLeXSellArgs_ι_price | FLeXSellArgs_ι_amount | FLeXSellArgs_ι_lend_finish_time | FLeXSellArgs_ι_min_amount | FLeXSellArgs_ι_deals_limit | FLeXSellArgs_ι_tons_value | FLeXSellArgs_ι_price_code | FLeXSellArgs_ι_addrs | FLeXSellArgs_ι_tip3_code | FLeXSellArgs_ι_tip3cfg .
+(* 2 *) Definition FLeXSellArgs := 
+ ( XInteger128 * 
+ XInteger128 * 
+ XInteger32 * 
+ XInteger128 * 
+ XInteger8 * 
+ XInteger128 * 
+ TvmCell * 
+ XAddress * 
+ TvmCell * 
+ XAddress )%type .
+(* 1 *) Inductive FLeXBuyArgsFields := | FLeXBuyArgs_ι_price | FLeXBuyArgs_ι_amount | FLeXBuyArgs_ι_order_finish_time | FLeXBuyArgs_ι_min_amount | FLeXBuyArgs_ι_deals_limit | FLeXBuyArgs_ι_deploy_value | FLeXBuyArgs_ι_price_code | FLeXBuyArgs_ι_my_tip3_addr | FLeXBuyArgs_ι_tip3_code | FLeXBuyArgs_ι_tip3cfg .
+(* 2 *) Definition FLeXBuyArgs := 
+ ( XInteger128 * 
+ XInteger128 * 
+ XInteger32 * 
+ XInteger128 * 
+ XInteger8 * 
+ XInteger128 * 
+ TvmCell * 
+ XAddress * 
+ TvmCell * 
+ XAddress )%type .
+(* 1 *) Inductive FLeXXchgCfgsFields := | FLeXXchgCfgs_ι_major_tip3cfg | FLeXXchgCfgs_ι_minor_tip3cfg .
+(* 2 *) Definition FLeXXchgCfgs := 
+ ( XAddress * 
+ XAddress )%type .
+(* 1 *) Inductive FLeXXchgArgsFields := | FLeXXchgArgs_ι_sell | FLeXXchgArgs_ι_price_num | FLeXXchgArgs_ι_price_denum | FLeXXchgArgs_ι_amount | FLeXXchgArgs_ι_lend_amount | FLeXXchgArgs_ι_lend_finish_time | FLeXXchgArgs_ι_min_amount | FLeXXchgArgs_ι_deals_limit | FLeXXchgArgs_ι_tons_value | FLeXXchgArgs_ι_xchg_price_code | FLeXXchgArgs_ι_addrs | FLeXXchgArgs_ι_tip3_code | FLeXXchgArgs_ι_tip3cfgs .
+(* 2 *) Definition FLeXXchgArgs := 
+ ( XBool * 
+ XInteger128 * 
+ XInteger128 * 
+ XInteger128 * 
+ XInteger128 * 
+ XInteger32 * 
+ XInteger128 * 
+ XInteger8 * 
+ XInteger128 * 
+ TvmCell * 
+ XAddress * 
+ TvmCell * 
+ XAddress )%type .
+(* 1 *) Inductive FLeXCancelArgsFields := | FLeXCancelArgs_ι_price | FLeXCancelArgs_ι_min_amount | FLeXCancelArgs_ι_deals_limit | FLeXCancelArgs_ι_value | FLeXCancelArgs_ι_price_code | FLeXCancelArgs_ι_tip3_code | FLeXCancelArgs_ι_tip3cfg .
+(* 2 *) Definition FLeXCancelArgs := 
+ ( XInteger128 * 
+ XInteger128 * 
+ XInteger8 * 
+ XInteger128 * 
+ TvmCell * 
+ TvmCell * 
+ XAddress )%type .
+(* 1 *) Inductive FLeXXchgCancelArgsFields := | FLeXXchgCancelArgs_ι_sell | FLeXXchgCancelArgs_ι_price_num | FLeXXchgCancelArgs_ι_price_denum | FLeXXchgCancelArgs_ι_min_amount | FLeXXchgCancelArgs_ι_deals_limit | FLeXXchgCancelArgs_ι_value | FLeXXchgCancelArgs_ι_xchg_price_code | FLeXXchgCancelArgs_ι_tip3_code | FLeXXchgCancelArgs_ι_tip3cfgs .
+(* 2 *) Definition FLeXXchgCancelArgs := 
+ ( XBool * 
+ XInteger128 * 
+ XInteger128 * 
+ XInteger128 * 
+ XInteger8 * 
+ XInteger128 * 
+ TvmCell * 
+ TvmCell * 
+ XAddress )%type .
+(* 1 *) Inductive XchgPairFields := | XchgPair_ι_flex_addr_ | XchgPair_ι_tip3_major_root_ | XchgPair_ι_tip3_minor_root_ | XchgPair_ι_deploy_value_ .
+(* 2 *) Definition XchgPair := 
+ ( XAddress * 
+ XAddress * 
+ XAddress * 
+ XInteger128 )%type .
+(* 1 *) Inductive OrderInfoFields := | OrderInfo_ι_original_amount | OrderInfo_ι_amount | OrderInfo_ι_account | OrderInfo_ι_tip3_wallet | OrderInfo_ι_client_addr | OrderInfo_ι_order_finish_time .
+(* 2 *) Definition OrderInfo := 
+ ( XInteger128 * 
+ XInteger128 * 
+ XInteger128 * 
+ addr_std_fixed * 
+ addr_std_fixed * 
+ XInteger32 )%type .
+(* 1 *) Inductive Tip3ConfigFields := | Tip3Config_ι_name | Tip3Config_ι_symbol | Tip3Config_ι_decimals | Tip3Config_ι_root_public_key | Tip3Config_ι_root_address .
+(* 2 *) Definition Tip3Config := 
+ ( XString * 
+ XString * 
+ XInteger8 * 
+ XInteger256 * 
+ XAddress )%type .
+(* 1 *) Inductive PriceFields := | Price_ι_price_ | Price_ι_sells_amount_ | Price_ι_buys_amount_ | Price_ι_flex_ | Price_ι_min_amount_ | Price_ι_deals_limit_ | Price_ι_notify_addr_ | Price_ι_workchain_id_ | Price_ι_tons_cfg_ | Price_ι_tip3_code_ | Price_ι_tip3cfg_ | Price_ι_sells_ | Price_ι_buys_ .
+(* 2 *) Definition Price := 
+ ( XInteger128 * 
+ XInteger128 * 
+ XInteger128 * 
+ addr_std_fixed * 
+ XInteger128 * 
+ XInteger8 * 
+ IFLeXNotifyPtr * 
+ XInteger8 * 
+ TonsConfig * 
+ TvmCell * 
+ Tip3Config * 
+ XList OrderInfo * 
+ XList OrderInfo )%type .
+(* 1 *) Inductive RationalPriceFields := | RationalPrice_ι_num | RationalPrice_ι_denum .
+(* 2 *) Definition RationalPrice := 
+ ( XInteger128 * 
+ XInteger128 )%type .
+(* 1 *) Inductive PriceXchgFields := | PriceXchg_ι_price_ | PriceXchg_ι_sells_amount_ | PriceXchg_ι_buys_amount_ | PriceXchg_ι_flex_ | PriceXchg_ι_min_amount_ | PriceXchg_ι_deals_limit_ | PriceXchg_ι_notify_addr_ | PriceXchg_ι_workchain_id_ | PriceXchg_ι_tons_cfg_ | PriceXchg_ι_tip3_code_ | PriceXchg_ι_major_tip3cfg_ | PriceXchg_ι_minor_tip3cfg_ .
+(* 2 *) Definition PriceXchg := 
+ ( RationalPrice * 
+ XInteger128 * 
+ XInteger128 * 
+ addr_std_fixed * 
+ XInteger128 * 
+ XInteger8 * 
+ IFLeXNotifyPtr * 
+ XInteger8 * 
+ TonsConfig * 
+ TvmCell * 
+ Tip3Config * 
+ Tip3Config )%type .
+(* 1 *) Inductive TradingPairFields := | TradingPair_ι_flex_addr_ | TradingPair_ι_tip3_root_ | TradingPair_ι_deploy_value_ .
+(* 2 *) Definition TradingPair := 
+ ( XAddress * 
+ XAddress * 
+ XInteger128 )%type .
+(* 1 *) Inductive PayloadArgsFields := | PayloadArgs_ι_sell | PayloadArgs_ι_amount | PayloadArgs_ι_receive_tip3_wallet | PayloadArgs_ι_client_addr .
+(* 2 *) Definition PayloadArgs := 
+ ( XBool * 
+ XInteger128 * 
+ XAddress * 
+ XAddress )%type .
+(* 1 *) Inductive LocalStateFields := | LocalState_ι_uint256 | LocalState_ι_cell | LocalState_ι_TonsConfig | LocalState_ι_address | LocalState_ι_uint128 | LocalState_ι_TradingPair | LocalState_ι_tplStateInituint256 | LocalState_ι_StateInit | LocalState_ι_XchgPair | LocalState_ι_tplStateInitaddress | LocalState_ι_SellArgs | LocalState_ι_ITONTokenWalletPtr | LocalState_ι_IPricePtr | LocalState_ι_int | LocalState_ι_Price | LocalState_ι_uint8 | LocalState_ι_uint32 | LocalState_ι_Tip3Config | LocalState_ι_PriceXchg | LocalState_ι_PayloadArgs | LocalState_ι_uint256Index | LocalState_ι_cellIndex | LocalState_ι_TonsConfigIndex | LocalState_ι_addressIndex | LocalState_ι_uint128Index | LocalState_ι_TradingPairIndex | LocalState_ι_tplStateInituint256Index | LocalState_ι_StateInitIndex | LocalState_ι_XchgPairIndex | LocalState_ι_tplStateInitaddressIndex | LocalState_ι_SellArgsIndex | LocalState_ι_ITONTokenWalletPtrIndex | LocalState_ι_IPricePtrIndex | LocalState_ι_intIndex | LocalState_ι_PriceIndex | LocalState_ι_uint8Index | LocalState_ι_uint32Index | LocalState_ι_Tip3ConfigIndex | LocalState_ι_PriceXchgIndex | LocalState_ι_PayloadArgsIndex .
+(* 2 *) Definition LocalState := 
+ ( XHMap (string*nat) XInteger256 * 
+ XHMap (string*nat) TvmCell * 
+ XHMap (string*nat) TonsConfig * 
+ XHMap (string*nat) XAddress * 
+ XHMap (string*nat) XInteger128 * 
+ XHMap (string*nat) TradingPair * 
+ XHMap (string*nat) ( StateInit * XInteger256 ) * 
+ XHMap (string*nat) StateInit * 
+ XHMap (string*nat) XchgPair * 
+ XHMap (string*nat) ( StateInit * XAddress * XInteger256 ) * 
+ XHMap (string*nat) SellArgs * 
+ XHMap (string*nat) ITONTokenWalletPtr * 
+ XHMap (string*nat) IPricePtr * 
+ XHMap (string*nat) XInteger * 
+ XHMap (string*nat) Price * 
+ XHMap (string*nat) XInteger8 * 
+ XHMap (string*nat) XInteger32 * 
+ XHMap (string*nat) Tip3Config * 
+ XHMap (string*nat) PriceXchg * 
+ XHMap (string*nat) PayloadArgs * 
+ XHMap string nat * 
+ XHMap string nat * 
+ XHMap string nat * 
+ XHMap string nat * 
+ XHMap string nat * 
+ XHMap string nat * 
+ XHMap string nat * 
+ XHMap string nat * 
+ XHMap string nat * 
+ XHMap string nat * 
+ XHMap string nat * 
+ XHMap string nat * 
+ XHMap string nat * 
+ XHMap string nat * 
+ XHMap string nat * 
+ XHMap string nat * 
+ XHMap string nat * 
+ XHMap string nat * 
+ XHMap string nat * 
+ XHMap string nat )%type .
+(* 1 *) Inductive LedgerFieldsI := | Ledger_ι_FLeXClient | Ledger_ι_VMState | Ledger_ι_LocalState | Ledger_ι_LocalStateCopy .
+(* 2 *) Definition Ledger := 
+ ( FLeXClient * 
+ VMState * 
+ LocalState * 
+ LocalState )%type .
+
+ Definition LedgerFields := LedgerFieldsI. 
+
+
+(* 3 *) Definition TickTock_field_type f : Type :=  
+match f with 
+ | TickTock_ι_tick => XBool | TickTock_ι_tock => XBool end .
+(* 4 *) Definition TickTock_get (f: TickTockFields )(r: TickTock ) :  TickTock_field_type f := 
+ let '( r1 , r2 ) := r in 
+ match f with 
+ | TickTock_ι_tick => r1 
+ | TickTock_ι_tock => r2 
+ end .
+(* 5 *) Coercion TickTock_get : TickTockFields >-> Funclass .
+(* 6 *) Definition TickTock_set (f: TickTockFields ) 
+(v: TickTock_field_type f) (r: TickTock ): TickTock := 
+ let '( r1 , r2 ) := r in 
+ match f, v with 
+ | TickTock_ι_tick , v' => ( v' , r2 ) 
+ | TickTock_ι_tock , v' => ( r1 , v' ) 
+ end .
+(* 7 *) Global Instance TickTock_PruvendoRecord : PruvendoRecord TickTock TickTockFields :=
+{
+  field_type := TickTock_field_type; 
+  getPruvendoRecord := @TickTock_get ;
+  setPruvendoRecord := @TickTock_set ;
+} .
+(* 3 *) Definition StateInit_field_type f : Type :=  
+match f with 
+ | StateInit_ι_split_depth => XMaybe XInteger | StateInit_ι_special => XMaybe TickTock | StateInit_ι_code => XMaybe TvmCell | StateInit_ι_data => XMaybe TvmCell | StateInit_ι_library => XMaybe TvmCell end .
+(* 4 *) Definition StateInit_get (f: StateInitFields )(r: StateInit ) :  StateInit_field_type f := 
+ let '( r1 , r2 , r3 , r4 , r5 ) := r in 
+ match f with 
+ | StateInit_ι_split_depth => r1 
+ | StateInit_ι_special => r2 
+ | StateInit_ι_code => r3 
+ | StateInit_ι_data => r4 
+ | StateInit_ι_library => r5 
+ end .
+(* 5 *) Coercion StateInit_get : StateInitFields >-> Funclass .
+(* 6 *) Definition StateInit_set (f: StateInitFields ) 
+(v: StateInit_field_type f) (r: StateInit ): StateInit := 
+ let '( r1 , r2 , r3 , r4 , r5 ) := r in 
+ match f, v with 
+ | StateInit_ι_split_depth , v' => ( v' , r2 , r3 , r4 , r5 ) 
+ | StateInit_ι_special , v' => ( r1 , v' , r3 , r4 , r5 ) 
+ | StateInit_ι_code , v' => ( r1 , r2 , v' , r4 , r5 ) 
+ | StateInit_ι_data , v' => ( r1 , r2 , r3 , v' , r5 ) 
+ | StateInit_ι_library , v' => ( r1 , r2 , r3 , r4 , v' ) 
+ end .
+(* 7 *) Global Instance StateInit_PruvendoRecord : PruvendoRecord StateInit StateInitFields :=
+{
+  field_type := StateInit_field_type; 
+  getPruvendoRecord := @StateInit_get ;
+  setPruvendoRecord := @StateInit_set ;
+} .
+(* 3 *) Definition anycast_info_field_type f : Type :=  
+match f with 
+ | anycast_info_ι_rewrite_pfx => varuint32 end .
+(* 4 *) Definition anycast_info_get (f: anycast_infoFields )(r: anycast_info ) :  anycast_info_field_type f := 
+ let '( r1 ) := r in 
+ match f with 
+ | anycast_info_ι_rewrite_pfx => r1 
+ end .
+(* 5 *) Coercion anycast_info_get : anycast_infoFields >-> Funclass .
+(* 6 *) Definition anycast_info_set (f: anycast_infoFields ) 
+(v: anycast_info_field_type f) (r: anycast_info ): anycast_info := 
+ let '( r1 ) := r in 
+ match f, v with 
+ | anycast_info_ι_rewrite_pfx , v' => ( v' ) 
+ end .
+(* 7 *) Global Instance anycast_info_PruvendoRecord : PruvendoRecord anycast_info anycast_infoFields :=
+{
+  field_type := anycast_info_field_type; 
+  getPruvendoRecord := @anycast_info_get ;
+  setPruvendoRecord := @anycast_info_set ;
+} .
+(* 3 *) Definition addr_std_field_type f : Type :=  
+match f with 
+ | addr_std_ι_kind => XInteger | addr_std_ι_Anycast => XMaybe anycast_info | addr_std_ι_workchain_id => XInteger8 | addr_std_ι_address => XInteger256 end .
+(* 4 *) Definition addr_std_get (f: addr_stdFields )(r: addr_std ) :  addr_std_field_type f := 
+ let '( r1 , r2 , r3 , r4 ) := r in 
+ match f with 
+ | addr_std_ι_kind => r1 
+ | addr_std_ι_Anycast => r2 
+ | addr_std_ι_workchain_id => r3 
+ | addr_std_ι_address => r4 
+ end .
+(* 5 *) Coercion addr_std_get : addr_stdFields >-> Funclass .
+(* 6 *) Definition addr_std_set (f: addr_stdFields ) 
+(v: addr_std_field_type f) (r: addr_std ): addr_std := 
+ let '( r1 , r2 , r3 , r4 ) := r in 
+ match f, v with 
+ | addr_std_ι_kind , v' => ( v' , r2 , r3 , r4 ) 
+ | addr_std_ι_Anycast , v' => ( r1 , v' , r3 , r4 ) 
+ | addr_std_ι_workchain_id , v' => ( r1 , r2 , v' , r4 ) 
+ | addr_std_ι_address , v' => ( r1 , r2 , r3 , v' ) 
+ end .
+(* 7 *) Global Instance addr_std_PruvendoRecord : PruvendoRecord addr_std addr_stdFields :=
+{
+  field_type := addr_std_field_type; 
+  getPruvendoRecord := @addr_std_get ;
+  setPruvendoRecord := @addr_std_set ;
+} .
+(* 3 *) Definition addr_std_fixed_field_type f : Type :=  
+match f with 
+ | addr_std_fixed_ι_workchain_id => XInteger8 | addr_std_fixed_ι_address => XInteger256 end .
+(* 4 *) Definition addr_std_fixed_get (f: addr_std_fixedFields )(r: addr_std_fixed ) :  addr_std_fixed_field_type f := 
+ let '( r1 , r2 ) := r in 
+ match f with 
+ | addr_std_fixed_ι_workchain_id => r1 
+ | addr_std_fixed_ι_address => r2 
+ end .
+(* 5 *) Coercion addr_std_fixed_get : addr_std_fixedFields >-> Funclass .
+(* 6 *) Definition addr_std_fixed_set (f: addr_std_fixedFields ) 
+(v: addr_std_fixed_field_type f) (r: addr_std_fixed ): addr_std_fixed := 
+ let '( r1 , r2 ) := r in 
+ match f, v with 
+ | addr_std_fixed_ι_workchain_id , v' => ( v' , r2 ) 
+ | addr_std_fixed_ι_address , v' => ( r1 , v' ) 
+ end .
+(* 7 *) Global Instance addr_std_fixed_PruvendoRecord : PruvendoRecord addr_std_fixed addr_std_fixedFields :=
+{
+  field_type := addr_std_fixed_field_type; 
+  getPruvendoRecord := @addr_std_fixed_get ;
+  setPruvendoRecord := @addr_std_fixed_set ;
+} .
+(* 3 *) Definition SellArgs_field_type f : Type :=  
+match f with 
+ | SellArgs_ι_amount => XInteger128 | SellArgs_ι_receive_wallet => addr_std_fixed end .
+(* 4 *) Definition SellArgs_get (f: SellArgsFields )(r: SellArgs ) :  SellArgs_field_type f := 
+ let '( r1 , r2 ) := r in 
+ match f with 
+ | SellArgs_ι_amount => r1 
+ | SellArgs_ι_receive_wallet => r2 
+ end .
+(* 5 *) Coercion SellArgs_get : SellArgsFields >-> Funclass .
+(* 6 *) Definition SellArgs_set (f: SellArgsFields ) 
+(v: SellArgs_field_type f) (r: SellArgs ): SellArgs := 
+ let '( r1 , r2 ) := r in 
+ match f, v with 
+ | SellArgs_ι_amount , v' => ( v' , r2 ) 
+ | SellArgs_ι_receive_wallet , v' => ( r1 , v' ) 
+ end .
+(* 7 *) Global Instance SellArgs_PruvendoRecord : PruvendoRecord SellArgs SellArgsFields :=
+{
+  field_type := SellArgs_field_type; 
+  getPruvendoRecord := @SellArgs_get ;
+  setPruvendoRecord := @SellArgs_set ;
+} .
+(* 3 *) Definition FlexBurnWalletArgs_field_type f : Type :=  
+match f with 
+ | FlexBurnWalletArgs_ι_tons_value => XInteger128 | FlexBurnWalletArgs_ι_out_pubkey => XInteger256 | FlexBurnWalletArgs_ι_out_internal_owner => XAddress | FlexBurnWalletArgs_ι_my_tip3_addr => XAddress end .
+(* 4 *) Definition FlexBurnWalletArgs_get (f: FlexBurnWalletArgsFields )(r: FlexBurnWalletArgs ) :  FlexBurnWalletArgs_field_type f := 
+ let '( r1 , r2 , r3 , r4 ) := r in 
+ match f with 
+ | FlexBurnWalletArgs_ι_tons_value => r1 
+ | FlexBurnWalletArgs_ι_out_pubkey => r2 
+ | FlexBurnWalletArgs_ι_out_internal_owner => r3 
+ | FlexBurnWalletArgs_ι_my_tip3_addr => r4 
+ end .
+(* 5 *) Coercion FlexBurnWalletArgs_get : FlexBurnWalletArgsFields >-> Funclass .
+(* 6 *) Definition FlexBurnWalletArgs_set (f: FlexBurnWalletArgsFields ) 
+(v: FlexBurnWalletArgs_field_type f) (r: FlexBurnWalletArgs ): FlexBurnWalletArgs := 
+ let '( r1 , r2 , r3 , r4 ) := r in 
+ match f, v with 
+ | FlexBurnWalletArgs_ι_tons_value , v' => ( v' , r2 , r3 , r4 ) 
+ | FlexBurnWalletArgs_ι_out_pubkey , v' => ( r1 , v' , r3 , r4 ) 
+ | FlexBurnWalletArgs_ι_out_internal_owner , v' => ( r1 , r2 , v' , r4 ) 
+ | FlexBurnWalletArgs_ι_my_tip3_addr , v' => ( r1 , r2 , r3 , v' ) 
+ end .
+(* 7 *) Global Instance FlexBurnWalletArgs_PruvendoRecord : PruvendoRecord FlexBurnWalletArgs FlexBurnWalletArgsFields :=
+{
+  field_type := FlexBurnWalletArgs_field_type; 
+  getPruvendoRecord := @FlexBurnWalletArgs_get ;
+  setPruvendoRecord := @FlexBurnWalletArgs_set ;
+} .
+(* 3 *) Definition TonsConfig_field_type f : Type :=  
+match f with 
+ | TonsConfig_ι_transfer_tip3 => XInteger128 | TonsConfig_ι_return_ownership => XInteger128 | TonsConfig_ι_trading_pair_deploy => XInteger128 | TonsConfig_ι_order_answer => XInteger128 | TonsConfig_ι_process_queue => XInteger128 | TonsConfig_ι_send_notify => XInteger128 end .
+(* 4 *) Definition TonsConfig_get (f: TonsConfigFields )(r: TonsConfig ) :  TonsConfig_field_type f := 
+ let '( r1 , r2 , r3 , r4 , r5 , r6 ) := r in 
+ match f with 
+ | TonsConfig_ι_transfer_tip3 => r1 
+ | TonsConfig_ι_return_ownership => r2 
+ | TonsConfig_ι_trading_pair_deploy => r3 
+ | TonsConfig_ι_order_answer => r4 
+ | TonsConfig_ι_process_queue => r5 
+ | TonsConfig_ι_send_notify => r6 
+ end .
+(* 5 *) Coercion TonsConfig_get : TonsConfigFields >-> Funclass .
+(* 6 *) Definition TonsConfig_set (f: TonsConfigFields ) 
+(v: TonsConfig_field_type f) (r: TonsConfig ): TonsConfig := 
+ let '( r1 , r2 , r3 , r4 , r5 , r6 ) := r in 
+ match f, v with 
+ | TonsConfig_ι_transfer_tip3 , v' => ( v' , r2 , r3 , r4 , r5 , r6 ) 
+ | TonsConfig_ι_return_ownership , v' => ( r1 , v' , r3 , r4 , r5 , r6 ) 
+ | TonsConfig_ι_trading_pair_deploy , v' => ( r1 , r2 , v' , r4 , r5 , r6 ) 
+ | TonsConfig_ι_order_answer , v' => ( r1 , r2 , r3 , v' , r5 , r6 ) 
+ | TonsConfig_ι_process_queue , v' => ( r1 , r2 , r3 , r4 , v' , r6 ) 
+ | TonsConfig_ι_send_notify , v' => ( r1 , r2 , r3 , r4 , r5 , v' ) 
+ end .
+(* 7 *) Global Instance TonsConfig_PruvendoRecord : PruvendoRecord TonsConfig TonsConfigFields :=
+{
+  field_type := TonsConfig_field_type; 
+  getPruvendoRecord := @TonsConfig_get ;
+  setPruvendoRecord := @TonsConfig_set ;
+} .
+(* 3 *) Definition FLeXClient_field_type f : Type :=  
+match f with 
+ | FLeXClient_ι_owner_ => XInteger256 | FLeXClient_ι_trading_pair_code_ => TvmCell | FLeXClient_ι_xchg_pair_code_ => TvmCell | FLeXClient_ι_workchain_id_ => XInteger8 | FLeXClient_ι_tons_cfg_ => TonsConfig | FLeXClient_ι_flex_ => addr_std_compact | FLeXClient_ι_notify_addr_ => addr_std_compact | FLeXClient_ι_ext_wallet_code_ => XMaybe TvmCell | FLeXClient_ι_flex_wallet_code_ => XMaybe TvmCell | FLeXClient_ι_flex_wrapper_code_ => XMaybe TvmCell end .
+(* 4 *) Definition FLeXClient_get (f: FLeXClientFields )(r: FLeXClient ) :  FLeXClient_field_type f := 
+ let '( r1 , r2 , r3 , r4 , r5 , r6 , r7 , r8 , r9 , r10 ) := r in 
+ match f with 
+ | FLeXClient_ι_owner_ => r1 
+ | FLeXClient_ι_trading_pair_code_ => r2 
+ | FLeXClient_ι_xchg_pair_code_ => r3 
+ | FLeXClient_ι_workchain_id_ => r4 
+ | FLeXClient_ι_tons_cfg_ => r5 
+ | FLeXClient_ι_flex_ => r6 
+ | FLeXClient_ι_notify_addr_ => r7 
+ | FLeXClient_ι_ext_wallet_code_ => r8 
+ | FLeXClient_ι_flex_wallet_code_ => r9 
+ | FLeXClient_ι_flex_wrapper_code_ => r10 
+ end .
+(* 5 *) Coercion FLeXClient_get : FLeXClientFields >-> Funclass .
+(* 6 *) Definition FLeXClient_set (f: FLeXClientFields ) 
+(v: FLeXClient_field_type f) (r: FLeXClient ): FLeXClient := 
+ let '( r1 , r2 , r3 , r4 , r5 , r6 , r7 , r8 , r9 , r10 ) := r in 
+ match f, v with 
+ | FLeXClient_ι_owner_ , v' => ( v' , r2 , r3 , r4 , r5 , r6 , r7 , r8 , r9 , r10 ) 
+ | FLeXClient_ι_trading_pair_code_ , v' => ( r1 , v' , r3 , r4 , r5 , r6 , r7 , r8 , r9 , r10 ) 
+ | FLeXClient_ι_xchg_pair_code_ , v' => ( r1 , r2 , v' , r4 , r5 , r6 , r7 , r8 , r9 , r10 ) 
+ | FLeXClient_ι_workchain_id_ , v' => ( r1 , r2 , r3 , v' , r5 , r6 , r7 , r8 , r9 , r10 ) 
+ | FLeXClient_ι_tons_cfg_ , v' => ( r1 , r2 , r3 , r4 , v' , r6 , r7 , r8 , r9 , r10 ) 
+ | FLeXClient_ι_flex_ , v' => ( r1 , r2 , r3 , r4 , r5 , v' , r7 , r8 , r9 , r10 ) 
+ | FLeXClient_ι_notify_addr_ , v' => ( r1 , r2 , r3 , r4 , r5 , r6 , v' , r8 , r9 , r10 ) 
+ | FLeXClient_ι_ext_wallet_code_ , v' => ( r1 , r2 , r3 , r4 , r5 , r6 , r7 , v' , r9 , r10 ) 
+ | FLeXClient_ι_flex_wallet_code_ , v' => ( r1 , r2 , r3 , r4 , r5 , r6 , r7 , r8 , v' , r10 ) 
+ | FLeXClient_ι_flex_wrapper_code_ , v' => ( r1 , r2 , r3 , r4 , r5 , r6 , r7 , r8 , r9 , v' ) 
+ end .
+(* 7 *) Global Instance FLeXClient_PruvendoRecord : PruvendoRecord FLeXClient FLeXClientFields :=
+{
+  field_type := FLeXClient_field_type; 
+  getPruvendoRecord := @FLeXClient_get ;
+  setPruvendoRecord := @FLeXClient_set ;
+} .
+(* 3 *) Definition FLeXSellArgsAddrs_field_type f : Type :=  
+match f with 
+ | FLeXSellArgsAddrs_ι_my_tip3_addr => XAddress end .
+(* 4 *) Definition FLeXSellArgsAddrs_get (f: FLeXSellArgsAddrsFields )(r: FLeXSellArgsAddrs ) :  FLeXSellArgsAddrs_field_type f := 
+ let '( r1 ) := r in 
+ match f with 
+ | FLeXSellArgsAddrs_ι_my_tip3_addr => r1 
+ end .
+(* 5 *) Coercion FLeXSellArgsAddrs_get : FLeXSellArgsAddrsFields >-> Funclass .
+(* 6 *) Definition FLeXSellArgsAddrs_set (f: FLeXSellArgsAddrsFields ) 
+(v: FLeXSellArgsAddrs_field_type f) (r: FLeXSellArgsAddrs ): FLeXSellArgsAddrs := 
+ let '( r1 ) := r in 
+ match f, v with 
+ | FLeXSellArgsAddrs_ι_my_tip3_addr , v' => ( v' ) 
+ end .
+(* 7 *) Global Instance FLeXSellArgsAddrs_PruvendoRecord : PruvendoRecord FLeXSellArgsAddrs FLeXSellArgsAddrsFields :=
+{
+  field_type := FLeXSellArgsAddrs_field_type; 
+  getPruvendoRecord := @FLeXSellArgsAddrs_get ;
+  setPruvendoRecord := @FLeXSellArgsAddrs_set ;
+} .
+(* 3 *) Definition FLeXSellArgs_field_type f : Type :=  
+match f with 
+ | FLeXSellArgs_ι_price => XInteger128 | FLeXSellArgs_ι_amount => XInteger128 | FLeXSellArgs_ι_lend_finish_time => XInteger32 | FLeXSellArgs_ι_min_amount => XInteger128 | FLeXSellArgs_ι_deals_limit => XInteger8 | FLeXSellArgs_ι_tons_value => XInteger128 | FLeXSellArgs_ι_price_code => TvmCell | FLeXSellArgs_ι_addrs => XAddress | FLeXSellArgs_ι_tip3_code => TvmCell | FLeXSellArgs_ι_tip3cfg => XAddress end .
+(* 4 *) Definition FLeXSellArgs_get (f: FLeXSellArgsFields )(r: FLeXSellArgs ) :  FLeXSellArgs_field_type f := 
+ let '( r1 , r2 , r3 , r4 , r5 , r6 , r7 , r8 , r9 , r10 ) := r in 
+ match f with 
+ | FLeXSellArgs_ι_price => r1 
+ | FLeXSellArgs_ι_amount => r2 
+ | FLeXSellArgs_ι_lend_finish_time => r3 
+ | FLeXSellArgs_ι_min_amount => r4 
+ | FLeXSellArgs_ι_deals_limit => r5 
+ | FLeXSellArgs_ι_tons_value => r6 
+ | FLeXSellArgs_ι_price_code => r7 
+ | FLeXSellArgs_ι_addrs => r8 
+ | FLeXSellArgs_ι_tip3_code => r9 
+ | FLeXSellArgs_ι_tip3cfg => r10 
+ end .
+(* 5 *) Coercion FLeXSellArgs_get : FLeXSellArgsFields >-> Funclass .
+(* 6 *) Definition FLeXSellArgs_set (f: FLeXSellArgsFields ) 
+(v: FLeXSellArgs_field_type f) (r: FLeXSellArgs ): FLeXSellArgs := 
+ let '( r1 , r2 , r3 , r4 , r5 , r6 , r7 , r8 , r9 , r10 ) := r in 
+ match f, v with 
+ | FLeXSellArgs_ι_price , v' => ( v' , r2 , r3 , r4 , r5 , r6 , r7 , r8 , r9 , r10 ) 
+ | FLeXSellArgs_ι_amount , v' => ( r1 , v' , r3 , r4 , r5 , r6 , r7 , r8 , r9 , r10 ) 
+ | FLeXSellArgs_ι_lend_finish_time , v' => ( r1 , r2 , v' , r4 , r5 , r6 , r7 , r8 , r9 , r10 ) 
+ | FLeXSellArgs_ι_min_amount , v' => ( r1 , r2 , r3 , v' , r5 , r6 , r7 , r8 , r9 , r10 ) 
+ | FLeXSellArgs_ι_deals_limit , v' => ( r1 , r2 , r3 , r4 , v' , r6 , r7 , r8 , r9 , r10 ) 
+ | FLeXSellArgs_ι_tons_value , v' => ( r1 , r2 , r3 , r4 , r5 , v' , r7 , r8 , r9 , r10 ) 
+ | FLeXSellArgs_ι_price_code , v' => ( r1 , r2 , r3 , r4 , r5 , r6 , v' , r8 , r9 , r10 ) 
+ | FLeXSellArgs_ι_addrs , v' => ( r1 , r2 , r3 , r4 , r5 , r6 , r7 , v' , r9 , r10 ) 
+ | FLeXSellArgs_ι_tip3_code , v' => ( r1 , r2 , r3 , r4 , r5 , r6 , r7 , r8 , v' , r10 ) 
+ | FLeXSellArgs_ι_tip3cfg , v' => ( r1 , r2 , r3 , r4 , r5 , r6 , r7 , r8 , r9 , v' ) 
+ end .
+(* 7 *) Global Instance FLeXSellArgs_PruvendoRecord : PruvendoRecord FLeXSellArgs FLeXSellArgsFields :=
+{
+  field_type := FLeXSellArgs_field_type; 
+  getPruvendoRecord := @FLeXSellArgs_get ;
+  setPruvendoRecord := @FLeXSellArgs_set ;
+} .
+(* 3 *) Definition FLeXBuyArgs_field_type f : Type :=  
+match f with 
+ | FLeXBuyArgs_ι_price => XInteger128 | FLeXBuyArgs_ι_amount => XInteger128 | FLeXBuyArgs_ι_order_finish_time => XInteger32 | FLeXBuyArgs_ι_min_amount => XInteger128 | FLeXBuyArgs_ι_deals_limit => XInteger8 | FLeXBuyArgs_ι_deploy_value => XInteger128 | FLeXBuyArgs_ι_price_code => TvmCell | FLeXBuyArgs_ι_my_tip3_addr => XAddress | FLeXBuyArgs_ι_tip3_code => TvmCell | FLeXBuyArgs_ι_tip3cfg => XAddress end .
+(* 4 *) Definition FLeXBuyArgs_get (f: FLeXBuyArgsFields )(r: FLeXBuyArgs ) :  FLeXBuyArgs_field_type f := 
+ let '( r1 , r2 , r3 , r4 , r5 , r6 , r7 , r8 , r9 , r10 ) := r in 
+ match f with 
+ | FLeXBuyArgs_ι_price => r1 
+ | FLeXBuyArgs_ι_amount => r2 
+ | FLeXBuyArgs_ι_order_finish_time => r3 
+ | FLeXBuyArgs_ι_min_amount => r4 
+ | FLeXBuyArgs_ι_deals_limit => r5 
+ | FLeXBuyArgs_ι_deploy_value => r6 
+ | FLeXBuyArgs_ι_price_code => r7 
+ | FLeXBuyArgs_ι_my_tip3_addr => r8 
+ | FLeXBuyArgs_ι_tip3_code => r9 
+ | FLeXBuyArgs_ι_tip3cfg => r10 
+ end .
+(* 5 *) Coercion FLeXBuyArgs_get : FLeXBuyArgsFields >-> Funclass .
+(* 6 *) Definition FLeXBuyArgs_set (f: FLeXBuyArgsFields ) 
+(v: FLeXBuyArgs_field_type f) (r: FLeXBuyArgs ): FLeXBuyArgs := 
+ let '( r1 , r2 , r3 , r4 , r5 , r6 , r7 , r8 , r9 , r10 ) := r in 
+ match f, v with 
+ | FLeXBuyArgs_ι_price , v' => ( v' , r2 , r3 , r4 , r5 , r6 , r7 , r8 , r9 , r10 ) 
+ | FLeXBuyArgs_ι_amount , v' => ( r1 , v' , r3 , r4 , r5 , r6 , r7 , r8 , r9 , r10 ) 
+ | FLeXBuyArgs_ι_order_finish_time , v' => ( r1 , r2 , v' , r4 , r5 , r6 , r7 , r8 , r9 , r10 ) 
+ | FLeXBuyArgs_ι_min_amount , v' => ( r1 , r2 , r3 , v' , r5 , r6 , r7 , r8 , r9 , r10 ) 
+ | FLeXBuyArgs_ι_deals_limit , v' => ( r1 , r2 , r3 , r4 , v' , r6 , r7 , r8 , r9 , r10 ) 
+ | FLeXBuyArgs_ι_deploy_value , v' => ( r1 , r2 , r3 , r4 , r5 , v' , r7 , r8 , r9 , r10 ) 
+ | FLeXBuyArgs_ι_price_code , v' => ( r1 , r2 , r3 , r4 , r5 , r6 , v' , r8 , r9 , r10 ) 
+ | FLeXBuyArgs_ι_my_tip3_addr , v' => ( r1 , r2 , r3 , r4 , r5 , r6 , r7 , v' , r9 , r10 ) 
+ | FLeXBuyArgs_ι_tip3_code , v' => ( r1 , r2 , r3 , r4 , r5 , r6 , r7 , r8 , v' , r10 ) 
+ | FLeXBuyArgs_ι_tip3cfg , v' => ( r1 , r2 , r3 , r4 , r5 , r6 , r7 , r8 , r9 , v' ) 
+ end .
+(* 7 *) Global Instance FLeXBuyArgs_PruvendoRecord : PruvendoRecord FLeXBuyArgs FLeXBuyArgsFields :=
+{
+  field_type := FLeXBuyArgs_field_type; 
+  getPruvendoRecord := @FLeXBuyArgs_get ;
+  setPruvendoRecord := @FLeXBuyArgs_set ;
+} .
+(* 3 *) Definition FLeXXchgCfgs_field_type f : Type :=  
+match f with 
+ | FLeXXchgCfgs_ι_major_tip3cfg => XAddress | FLeXXchgCfgs_ι_minor_tip3cfg => XAddress end .
+(* 4 *) Definition FLeXXchgCfgs_get (f: FLeXXchgCfgsFields )(r: FLeXXchgCfgs ) :  FLeXXchgCfgs_field_type f := 
+ let '( r1 , r2 ) := r in 
+ match f with 
+ | FLeXXchgCfgs_ι_major_tip3cfg => r1 
+ | FLeXXchgCfgs_ι_minor_tip3cfg => r2 
+ end .
+(* 5 *) Coercion FLeXXchgCfgs_get : FLeXXchgCfgsFields >-> Funclass .
+(* 6 *) Definition FLeXXchgCfgs_set (f: FLeXXchgCfgsFields ) 
+(v: FLeXXchgCfgs_field_type f) (r: FLeXXchgCfgs ): FLeXXchgCfgs := 
+ let '( r1 , r2 ) := r in 
+ match f, v with 
+ | FLeXXchgCfgs_ι_major_tip3cfg , v' => ( v' , r2 ) 
+ | FLeXXchgCfgs_ι_minor_tip3cfg , v' => ( r1 , v' ) 
+ end .
+(* 7 *) Global Instance FLeXXchgCfgs_PruvendoRecord : PruvendoRecord FLeXXchgCfgs FLeXXchgCfgsFields :=
+{
+  field_type := FLeXXchgCfgs_field_type; 
+  getPruvendoRecord := @FLeXXchgCfgs_get ;
+  setPruvendoRecord := @FLeXXchgCfgs_set ;
+} .
+(* 3 *) Definition FLeXXchgArgs_field_type f : Type :=  
+match f with 
+ | FLeXXchgArgs_ι_sell => XBool | FLeXXchgArgs_ι_price_num => XInteger128 | FLeXXchgArgs_ι_price_denum => XInteger128 | FLeXXchgArgs_ι_amount => XInteger128 | FLeXXchgArgs_ι_lend_amount => XInteger128 | FLeXXchgArgs_ι_lend_finish_time => XInteger32 | FLeXXchgArgs_ι_min_amount => XInteger128 | FLeXXchgArgs_ι_deals_limit => XInteger8 | FLeXXchgArgs_ι_tons_value => XInteger128 | FLeXXchgArgs_ι_xchg_price_code => TvmCell | FLeXXchgArgs_ι_addrs => XAddress | FLeXXchgArgs_ι_tip3_code => TvmCell | FLeXXchgArgs_ι_tip3cfgs => XAddress end .
+(* 4 *) Definition FLeXXchgArgs_get (f: FLeXXchgArgsFields )(r: FLeXXchgArgs ) :  FLeXXchgArgs_field_type f := 
+ let '( r1 , r2 , r3 , r4 , r5 , r6 , r7 , r8 , r9 , r10 , r11 , r12 , r13 ) := r in 
+ match f with 
+ | FLeXXchgArgs_ι_sell => r1 
+ | FLeXXchgArgs_ι_price_num => r2 
+ | FLeXXchgArgs_ι_price_denum => r3 
+ | FLeXXchgArgs_ι_amount => r4 
+ | FLeXXchgArgs_ι_lend_amount => r5 
+ | FLeXXchgArgs_ι_lend_finish_time => r6 
+ | FLeXXchgArgs_ι_min_amount => r7 
+ | FLeXXchgArgs_ι_deals_limit => r8 
+ | FLeXXchgArgs_ι_tons_value => r9 
+ | FLeXXchgArgs_ι_xchg_price_code => r10 
+ | FLeXXchgArgs_ι_addrs => r11 
+ | FLeXXchgArgs_ι_tip3_code => r12 
+ | FLeXXchgArgs_ι_tip3cfgs => r13 
+ end .
+(* 5 *) Coercion FLeXXchgArgs_get : FLeXXchgArgsFields >-> Funclass .
+(* 6 *) Definition FLeXXchgArgs_set (f: FLeXXchgArgsFields ) 
+(v: FLeXXchgArgs_field_type f) (r: FLeXXchgArgs ): FLeXXchgArgs := 
+ let '( r1 , r2 , r3 , r4 , r5 , r6 , r7 , r8 , r9 , r10 , r11 , r12 , r13 ) := r in 
+ match f, v with 
+ | FLeXXchgArgs_ι_sell , v' => ( v' , r2 , r3 , r4 , r5 , r6 , r7 , r8 , r9 , r10 , r11 , r12 , r13 ) 
+ | FLeXXchgArgs_ι_price_num , v' => ( r1 , v' , r3 , r4 , r5 , r6 , r7 , r8 , r9 , r10 , r11 , r12 , r13 ) 
+ | FLeXXchgArgs_ι_price_denum , v' => ( r1 , r2 , v' , r4 , r5 , r6 , r7 , r8 , r9 , r10 , r11 , r12 , r13 ) 
+ | FLeXXchgArgs_ι_amount , v' => ( r1 , r2 , r3 , v' , r5 , r6 , r7 , r8 , r9 , r10 , r11 , r12 , r13 ) 
+ | FLeXXchgArgs_ι_lend_amount , v' => ( r1 , r2 , r3 , r4 , v' , r6 , r7 , r8 , r9 , r10 , r11 , r12 , r13 ) 
+ | FLeXXchgArgs_ι_lend_finish_time , v' => ( r1 , r2 , r3 , r4 , r5 , v' , r7 , r8 , r9 , r10 , r11 , r12 , r13 ) 
+ | FLeXXchgArgs_ι_min_amount , v' => ( r1 , r2 , r3 , r4 , r5 , r6 , v' , r8 , r9 , r10 , r11 , r12 , r13 ) 
+ | FLeXXchgArgs_ι_deals_limit , v' => ( r1 , r2 , r3 , r4 , r5 , r6 , r7 , v' , r9 , r10 , r11 , r12 , r13 ) 
+ | FLeXXchgArgs_ι_tons_value , v' => ( r1 , r2 , r3 , r4 , r5 , r6 , r7 , r8 , v' , r10 , r11 , r12 , r13 ) 
+ | FLeXXchgArgs_ι_xchg_price_code , v' => ( r1 , r2 , r3 , r4 , r5 , r6 , r7 , r8 , r9 , v' , r11 , r12 , r13 ) 
+ | FLeXXchgArgs_ι_addrs , v' => ( r1 , r2 , r3 , r4 , r5 , r6 , r7 , r8 , r9 , r10 , v' , r12 , r13 ) 
+ | FLeXXchgArgs_ι_tip3_code , v' => ( r1 , r2 , r3 , r4 , r5 , r6 , r7 , r8 , r9 , r10 , r11 , v' , r13 ) 
+ | FLeXXchgArgs_ι_tip3cfgs , v' => ( r1 , r2 , r3 , r4 , r5 , r6 , r7 , r8 , r9 , r10 , r11 , r12 , v' ) 
+ end .
+(* 7 *) Global Instance FLeXXchgArgs_PruvendoRecord : PruvendoRecord FLeXXchgArgs FLeXXchgArgsFields :=
+{
+  field_type := FLeXXchgArgs_field_type; 
+  getPruvendoRecord := @FLeXXchgArgs_get ;
+  setPruvendoRecord := @FLeXXchgArgs_set ;
+} .
+(* 3 *) Definition FLeXCancelArgs_field_type f : Type :=  
+match f with 
+ | FLeXCancelArgs_ι_price => XInteger128 | FLeXCancelArgs_ι_min_amount => XInteger128 | FLeXCancelArgs_ι_deals_limit => XInteger8 | FLeXCancelArgs_ι_value => XInteger128 | FLeXCancelArgs_ι_price_code => TvmCell | FLeXCancelArgs_ι_tip3_code => TvmCell | FLeXCancelArgs_ι_tip3cfg => XAddress end .
+(* 4 *) Definition FLeXCancelArgs_get (f: FLeXCancelArgsFields )(r: FLeXCancelArgs ) :  FLeXCancelArgs_field_type f := 
+ let '( r1 , r2 , r3 , r4 , r5 , r6 , r7 ) := r in 
+ match f with 
+ | FLeXCancelArgs_ι_price => r1 
+ | FLeXCancelArgs_ι_min_amount => r2 
+ | FLeXCancelArgs_ι_deals_limit => r3 
+ | FLeXCancelArgs_ι_value => r4 
+ | FLeXCancelArgs_ι_price_code => r5 
+ | FLeXCancelArgs_ι_tip3_code => r6 
+ | FLeXCancelArgs_ι_tip3cfg => r7 
+ end .
+(* 5 *) Coercion FLeXCancelArgs_get : FLeXCancelArgsFields >-> Funclass .
+(* 6 *) Definition FLeXCancelArgs_set (f: FLeXCancelArgsFields ) 
+(v: FLeXCancelArgs_field_type f) (r: FLeXCancelArgs ): FLeXCancelArgs := 
+ let '( r1 , r2 , r3 , r4 , r5 , r6 , r7 ) := r in 
+ match f, v with 
+ | FLeXCancelArgs_ι_price , v' => ( v' , r2 , r3 , r4 , r5 , r6 , r7 ) 
+ | FLeXCancelArgs_ι_min_amount , v' => ( r1 , v' , r3 , r4 , r5 , r6 , r7 ) 
+ | FLeXCancelArgs_ι_deals_limit , v' => ( r1 , r2 , v' , r4 , r5 , r6 , r7 ) 
+ | FLeXCancelArgs_ι_value , v' => ( r1 , r2 , r3 , v' , r5 , r6 , r7 ) 
+ | FLeXCancelArgs_ι_price_code , v' => ( r1 , r2 , r3 , r4 , v' , r6 , r7 ) 
+ | FLeXCancelArgs_ι_tip3_code , v' => ( r1 , r2 , r3 , r4 , r5 , v' , r7 ) 
+ | FLeXCancelArgs_ι_tip3cfg , v' => ( r1 , r2 , r3 , r4 , r5 , r6 , v' ) 
+ end .
+(* 7 *) Global Instance FLeXCancelArgs_PruvendoRecord : PruvendoRecord FLeXCancelArgs FLeXCancelArgsFields :=
+{
+  field_type := FLeXCancelArgs_field_type; 
+  getPruvendoRecord := @FLeXCancelArgs_get ;
+  setPruvendoRecord := @FLeXCancelArgs_set ;
+} .
+(* 3 *) Definition FLeXXchgCancelArgs_field_type f : Type :=  
+match f with 
+ | FLeXXchgCancelArgs_ι_sell => XBool | FLeXXchgCancelArgs_ι_price_num => XInteger128 | FLeXXchgCancelArgs_ι_price_denum => XInteger128 | FLeXXchgCancelArgs_ι_min_amount => XInteger128 | FLeXXchgCancelArgs_ι_deals_limit => XInteger8 | FLeXXchgCancelArgs_ι_value => XInteger128 | FLeXXchgCancelArgs_ι_xchg_price_code => TvmCell | FLeXXchgCancelArgs_ι_tip3_code => TvmCell | FLeXXchgCancelArgs_ι_tip3cfgs => XAddress end .
+(* 4 *) Definition FLeXXchgCancelArgs_get (f: FLeXXchgCancelArgsFields )(r: FLeXXchgCancelArgs ) :  FLeXXchgCancelArgs_field_type f := 
+ let '( r1 , r2 , r3 , r4 , r5 , r6 , r7 , r8 , r9 ) := r in 
+ match f with 
+ | FLeXXchgCancelArgs_ι_sell => r1 
+ | FLeXXchgCancelArgs_ι_price_num => r2 
+ | FLeXXchgCancelArgs_ι_price_denum => r3 
+ | FLeXXchgCancelArgs_ι_min_amount => r4 
+ | FLeXXchgCancelArgs_ι_deals_limit => r5 
+ | FLeXXchgCancelArgs_ι_value => r6 
+ | FLeXXchgCancelArgs_ι_xchg_price_code => r7 
+ | FLeXXchgCancelArgs_ι_tip3_code => r8 
+ | FLeXXchgCancelArgs_ι_tip3cfgs => r9 
+ end .
+(* 5 *) Coercion FLeXXchgCancelArgs_get : FLeXXchgCancelArgsFields >-> Funclass .
+(* 6 *) Definition FLeXXchgCancelArgs_set (f: FLeXXchgCancelArgsFields ) 
+(v: FLeXXchgCancelArgs_field_type f) (r: FLeXXchgCancelArgs ): FLeXXchgCancelArgs := 
+ let '( r1 , r2 , r3 , r4 , r5 , r6 , r7 , r8 , r9 ) := r in 
+ match f, v with 
+ | FLeXXchgCancelArgs_ι_sell , v' => ( v' , r2 , r3 , r4 , r5 , r6 , r7 , r8 , r9 ) 
+ | FLeXXchgCancelArgs_ι_price_num , v' => ( r1 , v' , r3 , r4 , r5 , r6 , r7 , r8 , r9 ) 
+ | FLeXXchgCancelArgs_ι_price_denum , v' => ( r1 , r2 , v' , r4 , r5 , r6 , r7 , r8 , r9 ) 
+ | FLeXXchgCancelArgs_ι_min_amount , v' => ( r1 , r2 , r3 , v' , r5 , r6 , r7 , r8 , r9 ) 
+ | FLeXXchgCancelArgs_ι_deals_limit , v' => ( r1 , r2 , r3 , r4 , v' , r6 , r7 , r8 , r9 ) 
+ | FLeXXchgCancelArgs_ι_value , v' => ( r1 , r2 , r3 , r4 , r5 , v' , r7 , r8 , r9 ) 
+ | FLeXXchgCancelArgs_ι_xchg_price_code , v' => ( r1 , r2 , r3 , r4 , r5 , r6 , v' , r8 , r9 ) 
+ | FLeXXchgCancelArgs_ι_tip3_code , v' => ( r1 , r2 , r3 , r4 , r5 , r6 , r7 , v' , r9 ) 
+ | FLeXXchgCancelArgs_ι_tip3cfgs , v' => ( r1 , r2 , r3 , r4 , r5 , r6 , r7 , r8 , v' ) 
+ end .
+(* 7 *) Global Instance FLeXXchgCancelArgs_PruvendoRecord : PruvendoRecord FLeXXchgCancelArgs FLeXXchgCancelArgsFields :=
+{
+  field_type := FLeXXchgCancelArgs_field_type; 
+  getPruvendoRecord := @FLeXXchgCancelArgs_get ;
+  setPruvendoRecord := @FLeXXchgCancelArgs_set ;
+} .
+(* 3 *) Definition XchgPair_field_type f : Type :=  
+match f with 
+ | XchgPair_ι_flex_addr_ => XAddress | XchgPair_ι_tip3_major_root_ => XAddress | XchgPair_ι_tip3_minor_root_ => XAddress | XchgPair_ι_deploy_value_ => XInteger128 end .
+(* 4 *) Definition XchgPair_get (f: XchgPairFields )(r: XchgPair ) :  XchgPair_field_type f := 
+ let '( r1 , r2 , r3 , r4 ) := r in 
+ match f with 
+ | XchgPair_ι_flex_addr_ => r1 
+ | XchgPair_ι_tip3_major_root_ => r2 
+ | XchgPair_ι_tip3_minor_root_ => r3 
+ | XchgPair_ι_deploy_value_ => r4 
+ end .
+(* 5 *) Coercion XchgPair_get : XchgPairFields >-> Funclass .
+(* 6 *) Definition XchgPair_set (f: XchgPairFields ) 
+(v: XchgPair_field_type f) (r: XchgPair ): XchgPair := 
+ let '( r1 , r2 , r3 , r4 ) := r in 
+ match f, v with 
+ | XchgPair_ι_flex_addr_ , v' => ( v' , r2 , r3 , r4 ) 
+ | XchgPair_ι_tip3_major_root_ , v' => ( r1 , v' , r3 , r4 ) 
+ | XchgPair_ι_tip3_minor_root_ , v' => ( r1 , r2 , v' , r4 ) 
+ | XchgPair_ι_deploy_value_ , v' => ( r1 , r2 , r3 , v' ) 
+ end .
+(* 7 *) Global Instance XchgPair_PruvendoRecord : PruvendoRecord XchgPair XchgPairFields :=
+{
+  field_type := XchgPair_field_type; 
+  getPruvendoRecord := @XchgPair_get ;
+  setPruvendoRecord := @XchgPair_set ;
+} .
+(* 3 *) Definition OrderInfo_field_type f : Type :=  
+match f with 
+ | OrderInfo_ι_original_amount => XInteger128 | OrderInfo_ι_amount => XInteger128 | OrderInfo_ι_account => XInteger128 | OrderInfo_ι_tip3_wallet => addr_std_fixed | OrderInfo_ι_client_addr => addr_std_fixed | OrderInfo_ι_order_finish_time => XInteger32 end .
+(* 4 *) Definition OrderInfo_get (f: OrderInfoFields )(r: OrderInfo ) :  OrderInfo_field_type f := 
+ let '( r1 , r2 , r3 , r4 , r5 , r6 ) := r in 
+ match f with 
+ | OrderInfo_ι_original_amount => r1 
+ | OrderInfo_ι_amount => r2 
+ | OrderInfo_ι_account => r3 
+ | OrderInfo_ι_tip3_wallet => r4 
+ | OrderInfo_ι_client_addr => r5 
+ | OrderInfo_ι_order_finish_time => r6 
+ end .
+(* 5 *) Coercion OrderInfo_get : OrderInfoFields >-> Funclass .
+(* 6 *) Definition OrderInfo_set (f: OrderInfoFields ) 
+(v: OrderInfo_field_type f) (r: OrderInfo ): OrderInfo := 
+ let '( r1 , r2 , r3 , r4 , r5 , r6 ) := r in 
+ match f, v with 
+ | OrderInfo_ι_original_amount , v' => ( v' , r2 , r3 , r4 , r5 , r6 ) 
+ | OrderInfo_ι_amount , v' => ( r1 , v' , r3 , r4 , r5 , r6 ) 
+ | OrderInfo_ι_account , v' => ( r1 , r2 , v' , r4 , r5 , r6 ) 
+ | OrderInfo_ι_tip3_wallet , v' => ( r1 , r2 , r3 , v' , r5 , r6 ) 
+ | OrderInfo_ι_client_addr , v' => ( r1 , r2 , r3 , r4 , v' , r6 ) 
+ | OrderInfo_ι_order_finish_time , v' => ( r1 , r2 , r3 , r4 , r5 , v' ) 
+ end .
+(* 7 *) Global Instance OrderInfo_PruvendoRecord : PruvendoRecord OrderInfo OrderInfoFields :=
+{
+  field_type := OrderInfo_field_type; 
+  getPruvendoRecord := @OrderInfo_get ;
+  setPruvendoRecord := @OrderInfo_set ;
+} .
+(* 3 *) Definition Tip3Config_field_type f : Type :=  
+match f with 
+ | Tip3Config_ι_name => XString | Tip3Config_ι_symbol => XString | Tip3Config_ι_decimals => XInteger8 | Tip3Config_ι_root_public_key => XInteger256 | Tip3Config_ι_root_address => XAddress end .
+(* 4 *) Definition Tip3Config_get (f: Tip3ConfigFields )(r: Tip3Config ) :  Tip3Config_field_type f := 
+ let '( r1 , r2 , r3 , r4 , r5 ) := r in 
+ match f with 
+ | Tip3Config_ι_name => r1 
+ | Tip3Config_ι_symbol => r2 
+ | Tip3Config_ι_decimals => r3 
+ | Tip3Config_ι_root_public_key => r4 
+ | Tip3Config_ι_root_address => r5 
+ end .
+(* 5 *) Coercion Tip3Config_get : Tip3ConfigFields >-> Funclass .
+(* 6 *) Definition Tip3Config_set (f: Tip3ConfigFields ) 
+(v: Tip3Config_field_type f) (r: Tip3Config ): Tip3Config := 
+ let '( r1 , r2 , r3 , r4 , r5 ) := r in 
+ match f, v with 
+ | Tip3Config_ι_name , v' => ( v' , r2 , r3 , r4 , r5 ) 
+ | Tip3Config_ι_symbol , v' => ( r1 , v' , r3 , r4 , r5 ) 
+ | Tip3Config_ι_decimals , v' => ( r1 , r2 , v' , r4 , r5 ) 
+ | Tip3Config_ι_root_public_key , v' => ( r1 , r2 , r3 , v' , r5 ) 
+ | Tip3Config_ι_root_address , v' => ( r1 , r2 , r3 , r4 , v' ) 
+ end .
+(* 7 *) Global Instance Tip3Config_PruvendoRecord : PruvendoRecord Tip3Config Tip3ConfigFields :=
+{
+  field_type := Tip3Config_field_type; 
+  getPruvendoRecord := @Tip3Config_get ;
+  setPruvendoRecord := @Tip3Config_set ;
+} .
+(* 3 *) Definition Price_field_type f : Type :=  
+match f with 
+ | Price_ι_price_ => XInteger128 | Price_ι_sells_amount_ => XInteger128 | Price_ι_buys_amount_ => XInteger128 | Price_ι_flex_ => addr_std_fixed | Price_ι_min_amount_ => XInteger128 | Price_ι_deals_limit_ => XInteger8 | Price_ι_notify_addr_ => IFLeXNotifyPtr | Price_ι_workchain_id_ => XInteger8 | Price_ι_tons_cfg_ => TonsConfig | Price_ι_tip3_code_ => TvmCell | Price_ι_tip3cfg_ => Tip3Config | Price_ι_sells_ => XList OrderInfo | Price_ι_buys_ => XList OrderInfo end .
+(* 4 *) Definition Price_get (f: PriceFields )(r: Price ) :  Price_field_type f := 
+ let '( r1 , r2 , r3 , r4 , r5 , r6 , r7 , r8 , r9 , r10 , r11 , r12 , r13 ) := r in 
+ match f with 
+ | Price_ι_price_ => r1 
+ | Price_ι_sells_amount_ => r2 
+ | Price_ι_buys_amount_ => r3 
+ | Price_ι_flex_ => r4 
+ | Price_ι_min_amount_ => r5 
+ | Price_ι_deals_limit_ => r6 
+ | Price_ι_notify_addr_ => r7 
+ | Price_ι_workchain_id_ => r8 
+ | Price_ι_tons_cfg_ => r9 
+ | Price_ι_tip3_code_ => r10 
+ | Price_ι_tip3cfg_ => r11 
+ | Price_ι_sells_ => r12 
+ | Price_ι_buys_ => r13 
+ end .
+(* 5 *) Coercion Price_get : PriceFields >-> Funclass .
+(* 6 *) Definition Price_set (f: PriceFields ) 
+(v: Price_field_type f) (r: Price ): Price := 
+ let '( r1 , r2 , r3 , r4 , r5 , r6 , r7 , r8 , r9 , r10 , r11 , r12 , r13 ) := r in 
+ match f, v with 
+ | Price_ι_price_ , v' => ( v' , r2 , r3 , r4 , r5 , r6 , r7 , r8 , r9 , r10 , r11 , r12 , r13 ) 
+ | Price_ι_sells_amount_ , v' => ( r1 , v' , r3 , r4 , r5 , r6 , r7 , r8 , r9 , r10 , r11 , r12 , r13 ) 
+ | Price_ι_buys_amount_ , v' => ( r1 , r2 , v' , r4 , r5 , r6 , r7 , r8 , r9 , r10 , r11 , r12 , r13 ) 
+ | Price_ι_flex_ , v' => ( r1 , r2 , r3 , v' , r5 , r6 , r7 , r8 , r9 , r10 , r11 , r12 , r13 ) 
+ | Price_ι_min_amount_ , v' => ( r1 , r2 , r3 , r4 , v' , r6 , r7 , r8 , r9 , r10 , r11 , r12 , r13 ) 
+ | Price_ι_deals_limit_ , v' => ( r1 , r2 , r3 , r4 , r5 , v' , r7 , r8 , r9 , r10 , r11 , r12 , r13 ) 
+ | Price_ι_notify_addr_ , v' => ( r1 , r2 , r3 , r4 , r5 , r6 , v' , r8 , r9 , r10 , r11 , r12 , r13 ) 
+ | Price_ι_workchain_id_ , v' => ( r1 , r2 , r3 , r4 , r5 , r6 , r7 , v' , r9 , r10 , r11 , r12 , r13 ) 
+ | Price_ι_tons_cfg_ , v' => ( r1 , r2 , r3 , r4 , r5 , r6 , r7 , r8 , v' , r10 , r11 , r12 , r13 ) 
+ | Price_ι_tip3_code_ , v' => ( r1 , r2 , r3 , r4 , r5 , r6 , r7 , r8 , r9 , v' , r11 , r12 , r13 ) 
+ | Price_ι_tip3cfg_ , v' => ( r1 , r2 , r3 , r4 , r5 , r6 , r7 , r8 , r9 , r10 , v' , r12 , r13 ) 
+ | Price_ι_sells_ , v' => ( r1 , r2 , r3 , r4 , r5 , r6 , r7 , r8 , r9 , r10 , r11 , v' , r13 ) 
+ | Price_ι_buys_ , v' => ( r1 , r2 , r3 , r4 , r5 , r6 , r7 , r8 , r9 , r10 , r11 , r12 , v' ) 
+ end .
+(* 7 *) Global Instance Price_PruvendoRecord : PruvendoRecord Price PriceFields :=
+{
+  field_type := Price_field_type; 
+  getPruvendoRecord := @Price_get ;
+  setPruvendoRecord := @Price_set ;
+} .
+(* 3 *) Definition RationalPrice_field_type f : Type :=  
+match f with 
+ | RationalPrice_ι_num => XInteger128 | RationalPrice_ι_denum => XInteger128 end .
+(* 4 *) Definition RationalPrice_get (f: RationalPriceFields )(r: RationalPrice ) :  RationalPrice_field_type f := 
+ let '( r1 , r2 ) := r in 
+ match f with 
+ | RationalPrice_ι_num => r1 
+ | RationalPrice_ι_denum => r2 
+ end .
+(* 5 *) Coercion RationalPrice_get : RationalPriceFields >-> Funclass .
+(* 6 *) Definition RationalPrice_set (f: RationalPriceFields ) 
+(v: RationalPrice_field_type f) (r: RationalPrice ): RationalPrice := 
+ let '( r1 , r2 ) := r in 
+ match f, v with 
+ | RationalPrice_ι_num , v' => ( v' , r2 ) 
+ | RationalPrice_ι_denum , v' => ( r1 , v' ) 
+ end .
+(* 7 *) Global Instance RationalPrice_PruvendoRecord : PruvendoRecord RationalPrice RationalPriceFields :=
+{
+  field_type := RationalPrice_field_type; 
+  getPruvendoRecord := @RationalPrice_get ;
+  setPruvendoRecord := @RationalPrice_set ;
+} .
+(* 3 *) Definition PriceXchg_field_type f : Type :=  
+match f with 
+ | PriceXchg_ι_price_ => RationalPrice | PriceXchg_ι_sells_amount_ => XInteger128 | PriceXchg_ι_buys_amount_ => XInteger128 | PriceXchg_ι_flex_ => addr_std_fixed | PriceXchg_ι_min_amount_ => XInteger128 | PriceXchg_ι_deals_limit_ => XInteger8 | PriceXchg_ι_notify_addr_ => IFLeXNotifyPtr | PriceXchg_ι_workchain_id_ => XInteger8 | PriceXchg_ι_tons_cfg_ => TonsConfig | PriceXchg_ι_tip3_code_ => TvmCell | PriceXchg_ι_major_tip3cfg_ => Tip3Config | PriceXchg_ι_minor_tip3cfg_ => Tip3Config end .
+(* 4 *) Definition PriceXchg_get (f: PriceXchgFields )(r: PriceXchg ) :  PriceXchg_field_type f := 
+ let '( r1 , r2 , r3 , r4 , r5 , r6 , r7 , r8 , r9 , r10 , r11 , r12 ) := r in 
+ match f with 
+ | PriceXchg_ι_price_ => r1 
+ | PriceXchg_ι_sells_amount_ => r2 
+ | PriceXchg_ι_buys_amount_ => r3 
+ | PriceXchg_ι_flex_ => r4 
+ | PriceXchg_ι_min_amount_ => r5 
+ | PriceXchg_ι_deals_limit_ => r6 
+ | PriceXchg_ι_notify_addr_ => r7 
+ | PriceXchg_ι_workchain_id_ => r8 
+ | PriceXchg_ι_tons_cfg_ => r9 
+ | PriceXchg_ι_tip3_code_ => r10 
+ | PriceXchg_ι_major_tip3cfg_ => r11 
+ | PriceXchg_ι_minor_tip3cfg_ => r12 
+ end .
+(* 5 *) Coercion PriceXchg_get : PriceXchgFields >-> Funclass .
+(* 6 *) Definition PriceXchg_set (f: PriceXchgFields ) 
+(v: PriceXchg_field_type f) (r: PriceXchg ): PriceXchg := 
+ let '( r1 , r2 , r3 , r4 , r5 , r6 , r7 , r8 , r9 , r10 , r11 , r12 ) := r in 
+ match f, v with 
+ | PriceXchg_ι_price_ , v' => ( v' , r2 , r3 , r4 , r5 , r6 , r7 , r8 , r9 , r10 , r11 , r12 ) 
+ | PriceXchg_ι_sells_amount_ , v' => ( r1 , v' , r3 , r4 , r5 , r6 , r7 , r8 , r9 , r10 , r11 , r12 ) 
+ | PriceXchg_ι_buys_amount_ , v' => ( r1 , r2 , v' , r4 , r5 , r6 , r7 , r8 , r9 , r10 , r11 , r12 ) 
+ | PriceXchg_ι_flex_ , v' => ( r1 , r2 , r3 , v' , r5 , r6 , r7 , r8 , r9 , r10 , r11 , r12 ) 
+ | PriceXchg_ι_min_amount_ , v' => ( r1 , r2 , r3 , r4 , v' , r6 , r7 , r8 , r9 , r10 , r11 , r12 ) 
+ | PriceXchg_ι_deals_limit_ , v' => ( r1 , r2 , r3 , r4 , r5 , v' , r7 , r8 , r9 , r10 , r11 , r12 ) 
+ | PriceXchg_ι_notify_addr_ , v' => ( r1 , r2 , r3 , r4 , r5 , r6 , v' , r8 , r9 , r10 , r11 , r12 ) 
+ | PriceXchg_ι_workchain_id_ , v' => ( r1 , r2 , r3 , r4 , r5 , r6 , r7 , v' , r9 , r10 , r11 , r12 ) 
+ | PriceXchg_ι_tons_cfg_ , v' => ( r1 , r2 , r3 , r4 , r5 , r6 , r7 , r8 , v' , r10 , r11 , r12 ) 
+ | PriceXchg_ι_tip3_code_ , v' => ( r1 , r2 , r3 , r4 , r5 , r6 , r7 , r8 , r9 , v' , r11 , r12 ) 
+ | PriceXchg_ι_major_tip3cfg_ , v' => ( r1 , r2 , r3 , r4 , r5 , r6 , r7 , r8 , r9 , r10 , v' , r12 ) 
+ | PriceXchg_ι_minor_tip3cfg_ , v' => ( r1 , r2 , r3 , r4 , r5 , r6 , r7 , r8 , r9 , r10 , r11 , v' ) 
+ end .
+(* 7 *) Global Instance PriceXchg_PruvendoRecord : PruvendoRecord PriceXchg PriceXchgFields :=
+{
+  field_type := PriceXchg_field_type; 
+  getPruvendoRecord := @PriceXchg_get ;
+  setPruvendoRecord := @PriceXchg_set ;
+} .
+(* 3 *) Definition TradingPair_field_type f : Type :=  
+match f with 
+ | TradingPair_ι_flex_addr_ => XAddress | TradingPair_ι_tip3_root_ => XAddress | TradingPair_ι_deploy_value_ => XInteger128 end .
+(* 4 *) Definition TradingPair_get (f: TradingPairFields )(r: TradingPair ) :  TradingPair_field_type f := 
+ let '( r1 , r2 , r3 ) := r in 
+ match f with 
+ | TradingPair_ι_flex_addr_ => r1 
+ | TradingPair_ι_tip3_root_ => r2 
+ | TradingPair_ι_deploy_value_ => r3 
+ end .
+(* 5 *) Coercion TradingPair_get : TradingPairFields >-> Funclass .
+(* 6 *) Definition TradingPair_set (f: TradingPairFields ) 
+(v: TradingPair_field_type f) (r: TradingPair ): TradingPair := 
+ let '( r1 , r2 , r3 ) := r in 
+ match f, v with 
+ | TradingPair_ι_flex_addr_ , v' => ( v' , r2 , r3 ) 
+ | TradingPair_ι_tip3_root_ , v' => ( r1 , v' , r3 ) 
+ | TradingPair_ι_deploy_value_ , v' => ( r1 , r2 , v' ) 
+ end .
+(* 7 *) Global Instance TradingPair_PruvendoRecord : PruvendoRecord TradingPair TradingPairFields :=
+{
+  field_type := TradingPair_field_type; 
+  getPruvendoRecord := @TradingPair_get ;
+  setPruvendoRecord := @TradingPair_set ;
+} .
+(* 3 *) Definition PayloadArgs_field_type f : Type :=  
+match f with 
+ | PayloadArgs_ι_sell => XBool | PayloadArgs_ι_amount => XInteger128 | PayloadArgs_ι_receive_tip3_wallet => XAddress | PayloadArgs_ι_client_addr => XAddress end .
+(* 4 *) Definition PayloadArgs_get (f: PayloadArgsFields )(r: PayloadArgs ) :  PayloadArgs_field_type f := 
+ let '( r1 , r2 , r3 , r4 ) := r in 
+ match f with 
+ | PayloadArgs_ι_sell => r1 
+ | PayloadArgs_ι_amount => r2 
+ | PayloadArgs_ι_receive_tip3_wallet => r3 
+ | PayloadArgs_ι_client_addr => r4 
+ end .
+(* 5 *) Coercion PayloadArgs_get : PayloadArgsFields >-> Funclass .
+(* 6 *) Definition PayloadArgs_set (f: PayloadArgsFields ) 
+(v: PayloadArgs_field_type f) (r: PayloadArgs ): PayloadArgs := 
+ let '( r1 , r2 , r3 , r4 ) := r in 
+ match f, v with 
+ | PayloadArgs_ι_sell , v' => ( v' , r2 , r3 , r4 ) 
+ | PayloadArgs_ι_amount , v' => ( r1 , v' , r3 , r4 ) 
+ | PayloadArgs_ι_receive_tip3_wallet , v' => ( r1 , r2 , v' , r4 ) 
+ | PayloadArgs_ι_client_addr , v' => ( r1 , r2 , r3 , v' ) 
+ end .
+(* 7 *) Global Instance PayloadArgs_PruvendoRecord : PruvendoRecord PayloadArgs PayloadArgsFields :=
+{
+  field_type := PayloadArgs_field_type; 
+  getPruvendoRecord := @PayloadArgs_get ;
+  setPruvendoRecord := @PayloadArgs_set ;
+} .
+(* 3 *) Definition LocalState_field_type f : Type :=  
+match f with 
+ | LocalState_ι_uint256 => XHMap (string*nat) XInteger256 | LocalState_ι_cell => XHMap (string*nat) TvmCell | LocalState_ι_TonsConfig => XHMap (string*nat) TonsConfig | LocalState_ι_address => XHMap (string*nat) XAddress | LocalState_ι_uint128 => XHMap (string*nat) XInteger128 | LocalState_ι_TradingPair => XHMap (string*nat) TradingPair | LocalState_ι_tplStateInituint256 => XHMap (string*nat) ( StateInit * XInteger256 ) | LocalState_ι_StateInit => XHMap (string*nat) StateInit | LocalState_ι_XchgPair => XHMap (string*nat) XchgPair | LocalState_ι_tplStateInitaddress => XHMap (string*nat) ( StateInit * XAddress * XInteger256 ) | LocalState_ι_SellArgs => XHMap (string*nat) SellArgs | LocalState_ι_ITONTokenWalletPtr => XHMap (string*nat) ITONTokenWalletPtr | LocalState_ι_IPricePtr => XHMap (string*nat) IPricePtr | LocalState_ι_int => XHMap (string*nat) XInteger | LocalState_ι_Price => XHMap (string*nat) Price | LocalState_ι_uint8 => XHMap (string*nat) XInteger8 | LocalState_ι_uint32 => XHMap (string*nat) XInteger32 | LocalState_ι_Tip3Config => XHMap (string*nat) Tip3Config | LocalState_ι_PriceXchg => XHMap (string*nat) PriceXchg | LocalState_ι_PayloadArgs => XHMap (string*nat) PayloadArgs | LocalState_ι_uint256Index => XHMap string nat | LocalState_ι_cellIndex => XHMap string nat | LocalState_ι_TonsConfigIndex => XHMap string nat | LocalState_ι_addressIndex => XHMap string nat | LocalState_ι_uint128Index => XHMap string nat | LocalState_ι_TradingPairIndex => XHMap string nat | LocalState_ι_tplStateInituint256Index => XHMap string nat | LocalState_ι_StateInitIndex => XHMap string nat | LocalState_ι_XchgPairIndex => XHMap string nat | LocalState_ι_tplStateInitaddressIndex => XHMap string nat | LocalState_ι_SellArgsIndex => XHMap string nat | LocalState_ι_ITONTokenWalletPtrIndex => XHMap string nat | LocalState_ι_IPricePtrIndex => XHMap string nat | LocalState_ι_intIndex => XHMap string nat | LocalState_ι_PriceIndex => XHMap string nat | LocalState_ι_uint8Index => XHMap string nat | LocalState_ι_uint32Index => XHMap string nat | LocalState_ι_Tip3ConfigIndex => XHMap string nat | LocalState_ι_PriceXchgIndex => XHMap string nat | LocalState_ι_PayloadArgsIndex => XHMap string nat end .
+(* 4 *) Definition LocalState_get (f: LocalStateFields )(r: LocalState ) :  LocalState_field_type f := 
+ let '( r1 , r2 , r3 , r4 , r5 , r6 , r7 , r8 , r9 , r10 , r11 , r12 , r13 , r14 , r15 , r16 , r17 , r18 , r19 , r20 , r21 , r22 , r23 , r24 , r25 , r26 , r27 , r28 , r29 , r30 , r31 , r32 , r33 , r34 , r35 , r36 , r37 , r38 , r39 , r40 ) := r in 
+ match f with 
+ | LocalState_ι_uint256 => r1 
+ | LocalState_ι_cell => r2 
+ | LocalState_ι_TonsConfig => r3 
+ | LocalState_ι_address => r4 
+ | LocalState_ι_uint128 => r5 
+ | LocalState_ι_TradingPair => r6 
+ | LocalState_ι_tplStateInituint256 => r7 
+ | LocalState_ι_StateInit => r8 
+ | LocalState_ι_XchgPair => r9 
+ | LocalState_ι_tplStateInitaddress => r10 
+ | LocalState_ι_SellArgs => r11 
+ | LocalState_ι_ITONTokenWalletPtr => r12 
+ | LocalState_ι_IPricePtr => r13 
+ | LocalState_ι_int => r14 
+ | LocalState_ι_Price => r15 
+ | LocalState_ι_uint8 => r16 
+ | LocalState_ι_uint32 => r17 
+ | LocalState_ι_Tip3Config => r18 
+ | LocalState_ι_PriceXchg => r19 
+ | LocalState_ι_PayloadArgs => r20 
+ | LocalState_ι_uint256Index => r21 
+ | LocalState_ι_cellIndex => r22 
+ | LocalState_ι_TonsConfigIndex => r23 
+ | LocalState_ι_addressIndex => r24 
+ | LocalState_ι_uint128Index => r25 
+ | LocalState_ι_TradingPairIndex => r26 
+ | LocalState_ι_tplStateInituint256Index => r27 
+ | LocalState_ι_StateInitIndex => r28 
+ | LocalState_ι_XchgPairIndex => r29 
+ | LocalState_ι_tplStateInitaddressIndex => r30 
+ | LocalState_ι_SellArgsIndex => r31 
+ | LocalState_ι_ITONTokenWalletPtrIndex => r32 
+ | LocalState_ι_IPricePtrIndex => r33 
+ | LocalState_ι_intIndex => r34 
+ | LocalState_ι_PriceIndex => r35 
+ | LocalState_ι_uint8Index => r36 
+ | LocalState_ι_uint32Index => r37 
+ | LocalState_ι_Tip3ConfigIndex => r38 
+ | LocalState_ι_PriceXchgIndex => r39 
+ | LocalState_ι_PayloadArgsIndex => r40 
+ end .
+(* 5 *) Coercion LocalState_get : LocalStateFields >-> Funclass .
+(* 6 *) Definition LocalState_set (f: LocalStateFields ) 
+(v: LocalState_field_type f) (r: LocalState ): LocalState := 
+ let '( r1 , r2 , r3 , r4 , r5 , r6 , r7 , r8 , r9 , r10 , r11 , r12 , r13 , r14 , r15 , r16 , r17 , r18 , r19 , r20 , r21 , r22 , r23 , r24 , r25 , r26 , r27 , r28 , r29 , r30 , r31 , r32 , r33 , r34 , r35 , r36 , r37 , r38 , r39 , r40 ) := r in 
+ match f, v with 
+ | LocalState_ι_uint256 , v' => ( v' , r2 , r3 , r4 , r5 , r6 , r7 , r8 , r9 , r10 , r11 , r12 , r13 , r14 , r15 , r16 , r17 , r18 , r19 , r20 , r21 , r22 , r23 , r24 , r25 , r26 , r27 , r28 , r29 , r30 , r31 , r32 , r33 , r34 , r35 , r36 , r37 , r38 , r39 , r40 ) 
+ | LocalState_ι_cell , v' => ( r1 , v' , r3 , r4 , r5 , r6 , r7 , r8 , r9 , r10 , r11 , r12 , r13 , r14 , r15 , r16 , r17 , r18 , r19 , r20 , r21 , r22 , r23 , r24 , r25 , r26 , r27 , r28 , r29 , r30 , r31 , r32 , r33 , r34 , r35 , r36 , r37 , r38 , r39 , r40 ) 
+ | LocalState_ι_TonsConfig , v' => ( r1 , r2 , v' , r4 , r5 , r6 , r7 , r8 , r9 , r10 , r11 , r12 , r13 , r14 , r15 , r16 , r17 , r18 , r19 , r20 , r21 , r22 , r23 , r24 , r25 , r26 , r27 , r28 , r29 , r30 , r31 , r32 , r33 , r34 , r35 , r36 , r37 , r38 , r39 , r40 ) 
+ | LocalState_ι_address , v' => ( r1 , r2 , r3 , v' , r5 , r6 , r7 , r8 , r9 , r10 , r11 , r12 , r13 , r14 , r15 , r16 , r17 , r18 , r19 , r20 , r21 , r22 , r23 , r24 , r25 , r26 , r27 , r28 , r29 , r30 , r31 , r32 , r33 , r34 , r35 , r36 , r37 , r38 , r39 , r40 ) 
+ | LocalState_ι_uint128 , v' => ( r1 , r2 , r3 , r4 , v' , r6 , r7 , r8 , r9 , r10 , r11 , r12 , r13 , r14 , r15 , r16 , r17 , r18 , r19 , r20 , r21 , r22 , r23 , r24 , r25 , r26 , r27 , r28 , r29 , r30 , r31 , r32 , r33 , r34 , r35 , r36 , r37 , r38 , r39 , r40 ) 
+ | LocalState_ι_TradingPair , v' => ( r1 , r2 , r3 , r4 , r5 , v' , r7 , r8 , r9 , r10 , r11 , r12 , r13 , r14 , r15 , r16 , r17 , r18 , r19 , r20 , r21 , r22 , r23 , r24 , r25 , r26 , r27 , r28 , r29 , r30 , r31 , r32 , r33 , r34 , r35 , r36 , r37 , r38 , r39 , r40 ) 
+ | LocalState_ι_tplStateInituint256 , v' => ( r1 , r2 , r3 , r4 , r5 , r6 , v' , r8 , r9 , r10 , r11 , r12 , r13 , r14 , r15 , r16 , r17 , r18 , r19 , r20 , r21 , r22 , r23 , r24 , r25 , r26 , r27 , r28 , r29 , r30 , r31 , r32 , r33 , r34 , r35 , r36 , r37 , r38 , r39 , r40 ) 
+ | LocalState_ι_StateInit , v' => ( r1 , r2 , r3 , r4 , r5 , r6 , r7 , v' , r9 , r10 , r11 , r12 , r13 , r14 , r15 , r16 , r17 , r18 , r19 , r20 , r21 , r22 , r23 , r24 , r25 , r26 , r27 , r28 , r29 , r30 , r31 , r32 , r33 , r34 , r35 , r36 , r37 , r38 , r39 , r40 ) 
+ | LocalState_ι_XchgPair , v' => ( r1 , r2 , r3 , r4 , r5 , r6 , r7 , r8 , v' , r10 , r11 , r12 , r13 , r14 , r15 , r16 , r17 , r18 , r19 , r20 , r21 , r22 , r23 , r24 , r25 , r26 , r27 , r28 , r29 , r30 , r31 , r32 , r33 , r34 , r35 , r36 , r37 , r38 , r39 , r40 ) 
+ | LocalState_ι_tplStateInitaddress , v' => ( r1 , r2 , r3 , r4 , r5 , r6 , r7 , r8 , r9 , v' , r11 , r12 , r13 , r14 , r15 , r16 , r17 , r18 , r19 , r20 , r21 , r22 , r23 , r24 , r25 , r26 , r27 , r28 , r29 , r30 , r31 , r32 , r33 , r34 , r35 , r36 , r37 , r38 , r39 , r40 ) 
+ | LocalState_ι_SellArgs , v' => ( r1 , r2 , r3 , r4 , r5 , r6 , r7 , r8 , r9 , r10 , v' , r12 , r13 , r14 , r15 , r16 , r17 , r18 , r19 , r20 , r21 , r22 , r23 , r24 , r25 , r26 , r27 , r28 , r29 , r30 , r31 , r32 , r33 , r34 , r35 , r36 , r37 , r38 , r39 , r40 ) 
+ | LocalState_ι_ITONTokenWalletPtr , v' => ( r1 , r2 , r3 , r4 , r5 , r6 , r7 , r8 , r9 , r10 , r11 , v' , r13 , r14 , r15 , r16 , r17 , r18 , r19 , r20 , r21 , r22 , r23 , r24 , r25 , r26 , r27 , r28 , r29 , r30 , r31 , r32 , r33 , r34 , r35 , r36 , r37 , r38 , r39 , r40 ) 
+ | LocalState_ι_IPricePtr , v' => ( r1 , r2 , r3 , r4 , r5 , r6 , r7 , r8 , r9 , r10 , r11 , r12 , v' , r14 , r15 , r16 , r17 , r18 , r19 , r20 , r21 , r22 , r23 , r24 , r25 , r26 , r27 , r28 , r29 , r30 , r31 , r32 , r33 , r34 , r35 , r36 , r37 , r38 , r39 , r40 ) 
+ | LocalState_ι_int , v' => ( r1 , r2 , r3 , r4 , r5 , r6 , r7 , r8 , r9 , r10 , r11 , r12 , r13 , v' , r15 , r16 , r17 , r18 , r19 , r20 , r21 , r22 , r23 , r24 , r25 , r26 , r27 , r28 , r29 , r30 , r31 , r32 , r33 , r34 , r35 , r36 , r37 , r38 , r39 , r40 ) 
+ | LocalState_ι_Price , v' => ( r1 , r2 , r3 , r4 , r5 , r6 , r7 , r8 , r9 , r10 , r11 , r12 , r13 , r14 , v' , r16 , r17 , r18 , r19 , r20 , r21 , r22 , r23 , r24 , r25 , r26 , r27 , r28 , r29 , r30 , r31 , r32 , r33 , r34 , r35 , r36 , r37 , r38 , r39 , r40 ) 
+ | LocalState_ι_uint8 , v' => ( r1 , r2 , r3 , r4 , r5 , r6 , r7 , r8 , r9 , r10 , r11 , r12 , r13 , r14 , r15 , v' , r17 , r18 , r19 , r20 , r21 , r22 , r23 , r24 , r25 , r26 , r27 , r28 , r29 , r30 , r31 , r32 , r33 , r34 , r35 , r36 , r37 , r38 , r39 , r40 ) 
+ | LocalState_ι_uint32 , v' => ( r1 , r2 , r3 , r4 , r5 , r6 , r7 , r8 , r9 , r10 , r11 , r12 , r13 , r14 , r15 , r16 , v' , r18 , r19 , r20 , r21 , r22 , r23 , r24 , r25 , r26 , r27 , r28 , r29 , r30 , r31 , r32 , r33 , r34 , r35 , r36 , r37 , r38 , r39 , r40 ) 
+ | LocalState_ι_Tip3Config , v' => ( r1 , r2 , r3 , r4 , r5 , r6 , r7 , r8 , r9 , r10 , r11 , r12 , r13 , r14 , r15 , r16 , r17 , v' , r19 , r20 , r21 , r22 , r23 , r24 , r25 , r26 , r27 , r28 , r29 , r30 , r31 , r32 , r33 , r34 , r35 , r36 , r37 , r38 , r39 , r40 ) 
+ | LocalState_ι_PriceXchg , v' => ( r1 , r2 , r3 , r4 , r5 , r6 , r7 , r8 , r9 , r10 , r11 , r12 , r13 , r14 , r15 , r16 , r17 , r18 , v' , r20 , r21 , r22 , r23 , r24 , r25 , r26 , r27 , r28 , r29 , r30 , r31 , r32 , r33 , r34 , r35 , r36 , r37 , r38 , r39 , r40 ) 
+ | LocalState_ι_PayloadArgs , v' => ( r1 , r2 , r3 , r4 , r5 , r6 , r7 , r8 , r9 , r10 , r11 , r12 , r13 , r14 , r15 , r16 , r17 , r18 , r19 , v' , r21 , r22 , r23 , r24 , r25 , r26 , r27 , r28 , r29 , r30 , r31 , r32 , r33 , r34 , r35 , r36 , r37 , r38 , r39 , r40 ) 
+ | LocalState_ι_uint256Index , v' => ( r1 , r2 , r3 , r4 , r5 , r6 , r7 , r8 , r9 , r10 , r11 , r12 , r13 , r14 , r15 , r16 , r17 , r18 , r19 , r20 , v' , r22 , r23 , r24 , r25 , r26 , r27 , r28 , r29 , r30 , r31 , r32 , r33 , r34 , r35 , r36 , r37 , r38 , r39 , r40 ) 
+ | LocalState_ι_cellIndex , v' => ( r1 , r2 , r3 , r4 , r5 , r6 , r7 , r8 , r9 , r10 , r11 , r12 , r13 , r14 , r15 , r16 , r17 , r18 , r19 , r20 , r21 , v' , r23 , r24 , r25 , r26 , r27 , r28 , r29 , r30 , r31 , r32 , r33 , r34 , r35 , r36 , r37 , r38 , r39 , r40 ) 
+ | LocalState_ι_TonsConfigIndex , v' => ( r1 , r2 , r3 , r4 , r5 , r6 , r7 , r8 , r9 , r10 , r11 , r12 , r13 , r14 , r15 , r16 , r17 , r18 , r19 , r20 , r21 , r22 , v' , r24 , r25 , r26 , r27 , r28 , r29 , r30 , r31 , r32 , r33 , r34 , r35 , r36 , r37 , r38 , r39 , r40 ) 
+ | LocalState_ι_addressIndex , v' => ( r1 , r2 , r3 , r4 , r5 , r6 , r7 , r8 , r9 , r10 , r11 , r12 , r13 , r14 , r15 , r16 , r17 , r18 , r19 , r20 , r21 , r22 , r23 , v' , r25 , r26 , r27 , r28 , r29 , r30 , r31 , r32 , r33 , r34 , r35 , r36 , r37 , r38 , r39 , r40 ) 
+ | LocalState_ι_uint128Index , v' => ( r1 , r2 , r3 , r4 , r5 , r6 , r7 , r8 , r9 , r10 , r11 , r12 , r13 , r14 , r15 , r16 , r17 , r18 , r19 , r20 , r21 , r22 , r23 , r24 , v' , r26 , r27 , r28 , r29 , r30 , r31 , r32 , r33 , r34 , r35 , r36 , r37 , r38 , r39 , r40 ) 
+ | LocalState_ι_TradingPairIndex , v' => ( r1 , r2 , r3 , r4 , r5 , r6 , r7 , r8 , r9 , r10 , r11 , r12 , r13 , r14 , r15 , r16 , r17 , r18 , r19 , r20 , r21 , r22 , r23 , r24 , r25 , v' , r27 , r28 , r29 , r30 , r31 , r32 , r33 , r34 , r35 , r36 , r37 , r38 , r39 , r40 ) 
+ | LocalState_ι_tplStateInituint256Index , v' => ( r1 , r2 , r3 , r4 , r5 , r6 , r7 , r8 , r9 , r10 , r11 , r12 , r13 , r14 , r15 , r16 , r17 , r18 , r19 , r20 , r21 , r22 , r23 , r24 , r25 , r26 , v' , r28 , r29 , r30 , r31 , r32 , r33 , r34 , r35 , r36 , r37 , r38 , r39 , r40 ) 
+ | LocalState_ι_StateInitIndex , v' => ( r1 , r2 , r3 , r4 , r5 , r6 , r7 , r8 , r9 , r10 , r11 , r12 , r13 , r14 , r15 , r16 , r17 , r18 , r19 , r20 , r21 , r22 , r23 , r24 , r25 , r26 , r27 , v' , r29 , r30 , r31 , r32 , r33 , r34 , r35 , r36 , r37 , r38 , r39 , r40 ) 
+ | LocalState_ι_XchgPairIndex , v' => ( r1 , r2 , r3 , r4 , r5 , r6 , r7 , r8 , r9 , r10 , r11 , r12 , r13 , r14 , r15 , r16 , r17 , r18 , r19 , r20 , r21 , r22 , r23 , r24 , r25 , r26 , r27 , r28 , v' , r30 , r31 , r32 , r33 , r34 , r35 , r36 , r37 , r38 , r39 , r40 ) 
+ | LocalState_ι_tplStateInitaddressIndex , v' => ( r1 , r2 , r3 , r4 , r5 , r6 , r7 , r8 , r9 , r10 , r11 , r12 , r13 , r14 , r15 , r16 , r17 , r18 , r19 , r20 , r21 , r22 , r23 , r24 , r25 , r26 , r27 , r28 , r29 , v' , r31 , r32 , r33 , r34 , r35 , r36 , r37 , r38 , r39 , r40 ) 
+ | LocalState_ι_SellArgsIndex , v' => ( r1 , r2 , r3 , r4 , r5 , r6 , r7 , r8 , r9 , r10 , r11 , r12 , r13 , r14 , r15 , r16 , r17 , r18 , r19 , r20 , r21 , r22 , r23 , r24 , r25 , r26 , r27 , r28 , r29 , r30 , v' , r32 , r33 , r34 , r35 , r36 , r37 , r38 , r39 , r40 ) 
+ | LocalState_ι_ITONTokenWalletPtrIndex , v' => ( r1 , r2 , r3 , r4 , r5 , r6 , r7 , r8 , r9 , r10 , r11 , r12 , r13 , r14 , r15 , r16 , r17 , r18 , r19 , r20 , r21 , r22 , r23 , r24 , r25 , r26 , r27 , r28 , r29 , r30 , r31 , v' , r33 , r34 , r35 , r36 , r37 , r38 , r39 , r40 ) 
+ | LocalState_ι_IPricePtrIndex , v' => ( r1 , r2 , r3 , r4 , r5 , r6 , r7 , r8 , r9 , r10 , r11 , r12 , r13 , r14 , r15 , r16 , r17 , r18 , r19 , r20 , r21 , r22 , r23 , r24 , r25 , r26 , r27 , r28 , r29 , r30 , r31 , r32 , v' , r34 , r35 , r36 , r37 , r38 , r39 , r40 ) 
+ | LocalState_ι_intIndex , v' => ( r1 , r2 , r3 , r4 , r5 , r6 , r7 , r8 , r9 , r10 , r11 , r12 , r13 , r14 , r15 , r16 , r17 , r18 , r19 , r20 , r21 , r22 , r23 , r24 , r25 , r26 , r27 , r28 , r29 , r30 , r31 , r32 , r33 , v' , r35 , r36 , r37 , r38 , r39 , r40 ) 
+ | LocalState_ι_PriceIndex , v' => ( r1 , r2 , r3 , r4 , r5 , r6 , r7 , r8 , r9 , r10 , r11 , r12 , r13 , r14 , r15 , r16 , r17 , r18 , r19 , r20 , r21 , r22 , r23 , r24 , r25 , r26 , r27 , r28 , r29 , r30 , r31 , r32 , r33 , r34 , v' , r36 , r37 , r38 , r39 , r40 ) 
+ | LocalState_ι_uint8Index , v' => ( r1 , r2 , r3 , r4 , r5 , r6 , r7 , r8 , r9 , r10 , r11 , r12 , r13 , r14 , r15 , r16 , r17 , r18 , r19 , r20 , r21 , r22 , r23 , r24 , r25 , r26 , r27 , r28 , r29 , r30 , r31 , r32 , r33 , r34 , r35 , v' , r37 , r38 , r39 , r40 ) 
+ | LocalState_ι_uint32Index , v' => ( r1 , r2 , r3 , r4 , r5 , r6 , r7 , r8 , r9 , r10 , r11 , r12 , r13 , r14 , r15 , r16 , r17 , r18 , r19 , r20 , r21 , r22 , r23 , r24 , r25 , r26 , r27 , r28 , r29 , r30 , r31 , r32 , r33 , r34 , r35 , r36 , v' , r38 , r39 , r40 ) 
+ | LocalState_ι_Tip3ConfigIndex , v' => ( r1 , r2 , r3 , r4 , r5 , r6 , r7 , r8 , r9 , r10 , r11 , r12 , r13 , r14 , r15 , r16 , r17 , r18 , r19 , r20 , r21 , r22 , r23 , r24 , r25 , r26 , r27 , r28 , r29 , r30 , r31 , r32 , r33 , r34 , r35 , r36 , r37 , v' , r39 , r40 ) 
+ | LocalState_ι_PriceXchgIndex , v' => ( r1 , r2 , r3 , r4 , r5 , r6 , r7 , r8 , r9 , r10 , r11 , r12 , r13 , r14 , r15 , r16 , r17 , r18 , r19 , r20 , r21 , r22 , r23 , r24 , r25 , r26 , r27 , r28 , r29 , r30 , r31 , r32 , r33 , r34 , r35 , r36 , r37 , r38 , v' , r40 ) 
+ | LocalState_ι_PayloadArgsIndex , v' => ( r1 , r2 , r3 , r4 , r5 , r6 , r7 , r8 , r9 , r10 , r11 , r12 , r13 , r14 , r15 , r16 , r17 , r18 , r19 , r20 , r21 , r22 , r23 , r24 , r25 , r26 , r27 , r28 , r29 , r30 , r31 , r32 , r33 , r34 , r35 , r36 , r37 , r38 , r39 , v' ) 
+ end .
+(* 7 *) Global Instance LocalState_PruvendoRecord : PruvendoRecord LocalState LocalStateFields :=
+{
+  field_type := LocalState_field_type; 
+  getPruvendoRecord := @LocalState_get ;
+  setPruvendoRecord := @LocalState_set ;
+} .
+(* 3 *) Definition Ledger_field_type f : Type :=  
+match f with 
+ | Ledger_ι_FLeXClient => FLeXClient | Ledger_ι_VMState => VMState | Ledger_ι_LocalState => LocalState | Ledger_ι_LocalStateCopy => LocalState end .
+(* 4 *) Definition Ledger_get (f: LedgerFields )(r: Ledger ) :  Ledger_field_type f := 
+ let '( r1 , r2 , r3 , r4 ) := r in 
+ match f with 
+ | Ledger_ι_FLeXClient => r1 
+ | Ledger_ι_VMState => r2 
+ | Ledger_ι_LocalState => r3 
+ | Ledger_ι_LocalStateCopy => r4 
+ end .
+(* 5 *) Coercion Ledger_get : LedgerFields >-> Funclass .
+(* 6 *) Definition Ledger_set (f: LedgerFields ) 
+(v: Ledger_field_type f) (r: Ledger ): Ledger := 
+ let '( r1 , r2 , r3 , r4 ) := r in 
+ match f, v with 
+ | Ledger_ι_FLeXClient , v' => ( v' , r2 , r3 , r4 ) 
+ | Ledger_ι_VMState , v' => ( r1 , v' , r3 , r4 ) 
+ | Ledger_ι_LocalState , v' => ( r1 , r2 , v' , r4 ) 
+ | Ledger_ι_LocalStateCopy , v' => ( r1 , r2 , r3 , v' ) 
+ end .
+(* 7 *) Global Instance Ledger_PruvendoRecord : PruvendoRecord Ledger LedgerFields :=
+{
+  field_type := Ledger_field_type; 
+  getPruvendoRecord := @Ledger_get ;
+  setPruvendoRecord := @Ledger_set ;
+} .
+Definition T1 := FLeXClient .
+Definition T2 := VMState .
+Definition T3 := LocalState .
+Definition T4 := LocalState .
+
+ 
+ Definition projEmbed_T1 : Ledger -> T1 := getPruvendoRecord (PruvendoRecord := Ledger_PruvendoRecord) Ledger_ι_FLeXClient. 
+ Definition injEmbed_T1 : T1 -> Ledger -> Ledger := setPruvendoRecord (PruvendoRecord := Ledger_PruvendoRecord) Ledger_ι_FLeXClient. 
+ 
+ Lemma projinj_T1 : forall ( t : T1 ) ( s : Ledger ), projEmbed_T1 ( injEmbed_T1 t s ) = t . 
+ Proof. 
+ intros. destruct s. destruct p. destruct p. compute. auto. 
+ Qed. 
+ 
+ Lemma injproj_T1 : forall ( s : Ledger ) , injEmbed_T1 ( projEmbed_T1 s ) s = s . 
+ Proof. 
+ intros. 
+ destruct s. 
+ repeat match goal with 
+ | p : _ * _ |- _ => destruct p 
+ end. auto. 
+ Qed. 
+ 
+ 
+ Lemma injinj_T1 : forall ( t1 t2 : T1 ) ( s : Ledger ) , 
+ injEmbed_T1 t1 ( injEmbed_T1 t2 s) = 
+ injEmbed_T1 t1 s . 
+ Proof. 
+ intros. destruct s. 
+ repeat match goal with 
+ | p : _ * _ |- _ => destruct p 
+ end. auto. 
+ Qed. 
+ 
+ Global Instance embeddedT1 : EmbeddedType Ledger T1 := 
+ { 
+ projEmbed := projEmbed_T1 ; 
+ injEmbed := injEmbed_T1 ; 
+ projinj := projinj_T1 ; 
+ injproj := injproj_T1 ; 
+ injinj := injinj_T1 ; 
+ } . 
+ 
+
+
+ 
+ Definition projEmbed_T2 : Ledger -> T2 := getPruvendoRecord (PruvendoRecord := Ledger_PruvendoRecord) Ledger_ι_VMState. 
+ Definition injEmbed_T2 : T2 -> Ledger -> Ledger := setPruvendoRecord (PruvendoRecord := Ledger_PruvendoRecord) Ledger_ι_VMState. 
+ 
+ Lemma projinj_T2 : forall ( t : T2 ) ( s : Ledger ), projEmbed_T2 ( injEmbed_T2 t s ) = t . 
+ Proof. 
+ intros. destruct s. destruct p. destruct p. compute. auto. 
+ Qed. 
+ 
+ Lemma injproj_T2 : forall ( s : Ledger ) , injEmbed_T2 ( projEmbed_T2 s ) s = s . 
+ Proof. 
+ intros. 
+ destruct s. 
+ repeat match goal with 
+ | p : _ * _ |- _ => destruct p 
+ end. auto. 
+ Qed. 
+ 
+ 
+ Lemma injinj_T2 : forall ( t1 t2 : T2 ) ( s : Ledger ) , 
+ injEmbed_T2 t1 ( injEmbed_T2 t2 s) = 
+ injEmbed_T2 t1 s . 
+ Proof. 
+ intros. destruct s. 
+ repeat match goal with 
+ | p : _ * _ |- _ => destruct p 
+ end. auto. 
+ Qed. 
+ 
+ Global Instance embeddedT2 : EmbeddedType Ledger T2 := 
+ { 
+ projEmbed := projEmbed_T2 ; 
+ injEmbed := injEmbed_T2 ; 
+ projinj := projinj_T2 ; 
+ injproj := injproj_T2 ; 
+ injinj := injinj_T2 ; 
+ } . 
+ 
+
+
+ 
+ Definition projEmbed_T3 : Ledger -> T3 := getPruvendoRecord (PruvendoRecord := Ledger_PruvendoRecord) Ledger_ι_LocalState. 
+ Definition injEmbed_T3 : T3 -> Ledger -> Ledger := setPruvendoRecord (PruvendoRecord := Ledger_PruvendoRecord) Ledger_ι_LocalState. 
+ 
+ Lemma projinj_T3 : forall ( t : T3 ) ( s : Ledger ), projEmbed_T3 ( injEmbed_T3 t s ) = t . 
+ Proof. 
+ intros. destruct s. destruct p. destruct p. compute. auto. 
+ Qed. 
+ 
+ Lemma injproj_T3 : forall ( s : Ledger ) , injEmbed_T3 ( projEmbed_T3 s ) s = s . 
+ Proof. 
+ intros. 
+ destruct s. 
+ repeat match goal with 
+ | p : _ * _ |- _ => destruct p 
+ end. auto. 
+ Qed. 
+ 
+ 
+ Lemma injinj_T3 : forall ( t1 t2 : T3 ) ( s : Ledger ) , 
+ injEmbed_T3 t1 ( injEmbed_T3 t2 s) = 
+ injEmbed_T3 t1 s . 
+ Proof. 
+ intros. destruct s. 
+ repeat match goal with 
+ | p : _ * _ |- _ => destruct p 
+ end. auto. 
+ Qed. 
+ 
+ Global Instance embeddedT3 : EmbeddedType Ledger T3 := 
+ { 
+ projEmbed := projEmbed_T3 ; 
+ injEmbed := injEmbed_T3 ; 
+ projinj := projinj_T3 ; 
+ injproj := injproj_T3 ; 
+ injinj := injinj_T3 ; 
+ } . 
+ 
+
+
+ 
+ Definition projEmbed_T4 : Ledger -> T4 := getPruvendoRecord (PruvendoRecord := Ledger_PruvendoRecord) Ledger_ι_LocalStateCopy. 
+ Definition injEmbed_T4 : T4 -> Ledger -> Ledger := setPruvendoRecord (PruvendoRecord := Ledger_PruvendoRecord) Ledger_ι_LocalStateCopy. 
+ 
+ Lemma projinj_T4 : forall ( t : T4 ) ( s : Ledger ), projEmbed_T4 ( injEmbed_T4 t s ) = t . 
+ Proof. 
+ intros. destruct s. destruct p. destruct p. compute. auto. 
+ Qed. 
+ 
+ Lemma injproj_T4 : forall ( s : Ledger ) , injEmbed_T4 ( projEmbed_T4 s ) s = s . 
+ Proof. 
+ intros. 
+ destruct s. 
+ repeat match goal with 
+ | p : _ * _ |- _ => destruct p 
+ end. auto. 
+ Qed. 
+ 
+ 
+ Lemma injinj_T4 : forall ( t1 t2 : T4 ) ( s : Ledger ) , 
+ injEmbed_T4 t1 ( injEmbed_T4 t2 s) = 
+ injEmbed_T4 t1 s . 
+ Proof. 
+ intros. destruct s. 
+ repeat match goal with 
+ | p : _ * _ |- _ => destruct p 
+ end. auto. 
+ Qed. 
+ 
+ Global Instance embeddedT4 : EmbeddedType Ledger T4 := 
+ { 
+ projEmbed := projEmbed_T4 ; 
+ injEmbed := injEmbed_T4 ; 
+ projinj := projinj_T4 ; 
+ injproj := injproj_T4 ; 
+ injinj := injinj_T4 ; 
+ } . 
+ 
+
+
+
+Lemma injcommute_T1_T2: 
+               forall ( u : T2 ) ( t : T1 ) 
+                      ( s:Ledger ), 
+      ( injEmbed (EmbeddedType:=embeddedT2) u ( injEmbed t s ) ) = ( injEmbed t ( injEmbed (EmbeddedType:=embeddedT2) u s ) ).
+Proof.
+ intros. destruct s. destruct p. destruct p. compute.   auto.
+Qed.
+
+Instance InjectCommutableStates_T1_T2 : 
+@InjectCommutableStates Ledger ( T1 ) T2 := 
+{
+(*   embeddedTypeT := embeddedT1; *)
+  embeddedTypeU := embeddedT2 ;
+
+  injcommute := injcommute_T1_T2 
+}.
+
+Definition embeddedProduct_T1_T2 := 
+           @embeddedProduct Ledger ( T1 ) T2
+           InjectCommutableStates_T1_T2.
+
+Existing Instance embeddedProduct_T1_T2.
+
+
+Lemma injcommute_T1xT2_T3 : 
+               forall ( u : T3 ) ( t :  (T1 * T2)%xprod ) 
+                      ( s:Ledger ), 
+      ( injEmbed (EmbeddedType:=embeddedT3) u ( injEmbed t s ) ) = 
+      ( injEmbed t ( injEmbed (EmbeddedType:=embeddedT3) u s ) ).
+Proof.
+ intros. destruct s. destruct p. destruct p. compute. auto.
+Qed.
+
+Instance InjectCommutableStates_T1xT2_T3 : 
+@InjectCommutableStates Ledger (T1 * T2)%xprod T3 := 
+{
+  embeddedTypeU := embeddedT3 ;
+
+  injcommute := injcommute_T1xT2_T3 
+}.
+
+Definition embeddedProduct_T1xT2_T3 := 
+           @embeddedProduct Ledger (T1 * T2)%xprod T3
+  
+           InjectCommutableStates_T1xT2_T3.
+
+Existing Instance embeddedProduct_T1xT2_T3 . 
+
+
+Lemma injcommute_T1xT2xT3_T4 : 
+               forall ( u : T4 ) ( t :  ((T1 * T2)%xprod* T3)%xprod ) 
+                      ( s:Ledger ), 
+      ( injEmbed (EmbeddedType:=embeddedT4) u ( injEmbed t s ) ) = 
+      ( injEmbed t ( injEmbed (EmbeddedType:=embeddedT4) u s ) ).
+Proof.
+ intros. destruct s. destruct p. destruct p. compute. auto.
+Qed.
+
+Instance InjectCommutableStates_T1xT2xT3_T4 : 
+@InjectCommutableStates Ledger ((T1 * T2)%xprod* T3)%xprod T4 := 
+{
+  embeddedTypeU := embeddedT4 ;
+
+  injcommute := injcommute_T1xT2xT3_T4 
+}.
+
+Definition embeddedProduct_T1xT2xT3_T4 := 
+           @embeddedProduct Ledger ((T1 * T2)%xprod* T3)%xprod T4
+  
+           InjectCommutableStates_T1xT2xT3_T4.
+
+Existing Instance embeddedProduct_T1xT2xT3_T4 . 
+
+
+ 
+ Lemma fullState_T1xT2xT3_T4 : forall s s0, 
+ injEmbed ( T := (((T1 * T2)%xprod * T3)%xprod * T4)%xprod ) 
+ ( projEmbed s ) ( injEmbed ( T := T4 ) ( projEmbed s ) s0 ) = s. 
+ Proof. 
+ intros. destruct s. destruct p. destruct p. destruct s0. 
+ repeat match goal with 
+ | p : _ * _ |- _ => destruct p 
+ end. auto. 
+ Qed. 
+ 
+ Check FullState. 
+ (* 
+ Instance FullState_T1xT2xT3_T4 : 
+ FullState Ledger ((T1 * T2)%xprod * T3)%xprod T4 := 
+ { 
+ injComm := InjectCommutableStates_T1xT2xT3_T4 ; 
+ fullState := fullState_T1xT2xT3_T4 
+ } .  *)
+ 
+
+Local Open Scope solidity_scope.
+Notation "'↑ε4' m ":= (liftEmbeddedState ( H := embeddedT4 ) ( ε m )%sol ) (at level 10, left associativity): solidity_scope.
+Notation "'↑ε3' m ":= (liftEmbeddedState ( H := embeddedT3 ) ( ε m )%sol ) (at level 10, left associativity): solidity_scope.
+Notation "'↑ε2' m ":= (liftEmbeddedState ( H := embeddedT2 ) ( ε m )%sol ) (at level 10, left associativity): solidity_scope.
+Notation "'↑ε1' m ":= (liftEmbeddedState ( H := embeddedT1 ) ( ε m )%sol ) (at level 10, left associativity): solidity_scope.
+
+Notation "'↑4' m ":= (liftEmbeddedState ( H := embeddedT4 ) ( m ) ) (at level 10, left associativity): solidity_scope.
+Notation "'↑3' m ":= (liftEmbeddedState ( H := embeddedT3 ) ( m ) ) (at level 10, left associativity): solidity_scope.
+Notation "'↑2' m ":= (liftEmbeddedState ( H := embeddedT2 ) ( m ) ) (at level 10, left associativity): solidity_scope.
+Notation "'↑1' m ":= (liftEmbeddedState ( H := embeddedT1 ) ( m ) ) (at level 10, left associativity): solidity_scope.
+
+Notation "'↑↑4' m ":= (liftEmbeddedState ( H := embeddedT4 ) ) (at level 10, left associativity): solidity_scope.
+Notation "'↑↑3' m ":= (liftEmbeddedState ( H := embeddedT3 ) ) (at level 10, left associativity): solidity_scope.
+Notation "'↑↑2' m ":= (liftEmbeddedState ( H := embeddedT2 ) ) (at level 10, left associativity): solidity_scope.
+Notation "'↑↑1' m ":= (liftEmbeddedState ( H := embeddedT1 ) ) (at level 10, left associativity): solidity_scope.
+
+Notation "'↑0' m " := ( liftEmbeddedState ( H :=  embeddedProduct_T1xT2xT3_T4 ) ( m )) (at level 10, left associativity): solidity_scope.
+Notation "'↑↑0'" := ( liftEmbeddedState ( H :=  embeddedProduct_T1xT2xT3_T4 )) (at level 32, left associativity): solidity_scope.
+(* Notation " ↓ m " := ( callEmbeddedStateAdj m default (H0 :=  FullState_T1xT2xT3_T4 ) ) (at level 31, left associativity): solidity_scope. *)
+Global Instance iso_T1 : IsoTypes T1 (field_type (R:=Ledger) Ledger_ι_FLeXClient) :=
+{
+  x2y := Datatypes.id;
+  y2x := Datatypes.id;
+  x2x := eq_refl;
+  y2y := eq_refl
+}.
+
+Global Instance iso_T2 : IsoTypes T2 (field_type (R:=Ledger) Ledger_ι_VMState) :=
+{
+  x2y := Datatypes.id;
+  y2x := Datatypes.id;
+  x2x := eq_refl;
+  y2y := eq_refl
+}.
+
+Global Instance iso_T3 : IsoTypes T3 (field_type (R:=Ledger) Ledger_ι_LocalState) :=
+{
+  x2y := Datatypes.id;
+  y2x := Datatypes.id;
+  x2x := eq_refl;
+  y2y := eq_refl
+}.
+
+Global Instance iso_T4 : IsoTypes T4 (field_type (R:=Ledger) Ledger_ι_LocalStateCopy) :=
+{
+  x2y := Datatypes.id;
+  y2x := Datatypes.id;
+  x2x := eq_refl;
+  y2y := eq_refl
+}.
+
+
+ (* TODO: Тут надо вручную вставлять поля леджера зависящие от полей *) 
+
+Class Countable (X: Type) :=
+{
+   rength : nat;
+   rth : nat -> X -> {t: Type & t}
+}.
+
+Program Instance CountablePair0 : forall X Y, Countable (X*Y).
+Next Obligation.
+exact 2%nat.
+Defined.
+Next Obligation.
+destruct H.
+refine (existT id X x).
+refine (existT id Y y).
+Defined.
+Fail Next Obligation.
+
+Program Instance CountablePair_Next : forall X`{Countable X} Y, Countable (X*Y) .
+Next Obligation.
+exact (S rength).
+Defined.
+Next Obligation.
+remember (Nat.ltb H0 rength).
+destruct b.
+refine (rth  H0 x).
+refine (existT id Y y).
+Defined.
+Fail Next Obligation.
+
+Existing Instance CountablePair_Next | 0.
+Existing Instance CountablePair0 | 100.
+
+Opaque FLeXClient.
+
+Lemma Ledger1Type_eq: forall (l: Ledger), projT1 (rth 0 l) = FLeXClient.
+Proof.
+   intros.
+   compute.
+   destruct l.
+   repeat destruct p.
+   reflexivity.  
+Defined.
+
+Definition Ledger1Type (l: Ledger) := projT1 (rth 0 l).
+
+Definition Ledger1TypeFLeXClient : forall (l:Ledger), Ledger1Type l -> FLeXClient.
+intros.
+unfold Ledger1Type in X.
+rewrite Ledger1Type_eq in X.
+exact X.
+Defined.
+
+Coercion Ledger1TypeFLeXClient       : Ledger1Type >-> FLeXClient.
+
+Notation "r ₁" := ((projT2 (rth 0 r) : Ledger1Type r) : FLeXClient) (at level 10).
+
+Transparent FLeXClient.
+
+Definition LedgerPruvendoRecord := Ledger_PruvendoRecord.
+Definition LedgerLocalState := LocalState.
+Definition LedgerLocalFields := LocalStateFields.
+Definition LedgerLocalPruvendoRecord := LocalState_PruvendoRecord.
+Definition LocalEmbedded := embeddedT4.
+Definition LocalCopyEmbedded := embeddedT3.
+Definition LocalDefault : XDefault LocalState := prod_default.
+Definition Ledger_LocalState := Ledger_ι_LocalState.
+Definition Ledger_LocalStateCopy := Ledger_ι_LocalStateCopy.
+Definition iso_local := iso_T4.
+
+
+Lemma LedgerFieldsDec: forall (m1 m2: LedgerFields), {m1=m2}+{m1<>m2}.
+Proof.
+  intros.
+  decide equality.
+Defined.
+
+Lemma LocalCopySameType: field_type (PruvendoRecord:=LedgerPruvendoRecord) Ledger_LocalState = 
+field_type (PruvendoRecord:=LedgerPruvendoRecord) Ledger_LocalStateCopy.
+Proof.
+  reflexivity.
+Defined.
+
+Class LocalStateField (X:Type): Type := 
+{
+    local_index_embedded:> EmbeddedType LedgerLocalState (XHMap string nat) ;
+    local_state_field: LedgerLocalFields;
+    local_field_type_correct: field_type (PruvendoRecord:=LedgerLocalPruvendoRecord) local_state_field = XHMap (string*nat)%type X;
+}.
+
+
+(****************************************************************************)
+Definition  LocalState_ι_uint256Index_Embedded_projEmbed (l:LedgerLocalState ) : XHMap string nat := 
+  LocalState_ι_uint256Index l.
+
+Definition  LocalState_ι_uint256Index_Embedded_injEmbed (m: XHMap string nat) (l: LedgerLocalState) : LedgerLocalState := 
+  {$$ l with  LocalState_ι_uint256Index := m $$}.
+
+Print EmbeddedType.  
+
+Lemma LocalState_ι_uint256Index_Embedded_projinj : forall (t : XHMap string nat) (s : LedgerLocalState), LocalState_ι_uint256Index_Embedded_projEmbed (LocalState_ι_uint256Index_Embedded_injEmbed t s) = t.
+Proof.
+  intros.
+  destruct s.
+  repeat destruct p.
+  reflexivity.
+Defined.
+
+Lemma LocalState_ι_uint256Index_Embedded_injproj : forall s : LedgerLocalState, LocalState_ι_uint256Index_Embedded_injEmbed (LocalState_ι_uint256Index_Embedded_projEmbed s) s = s.
+Proof.
+  intros.
+  destruct s.
+  repeat destruct p.
+  reflexivity.
+Defined.  
+
+Lemma LocalState_ι_uint256Index_Embedded_injinj : forall (t1 t2 : XHMap string nat) (s : LedgerLocalState),
+LocalState_ι_uint256Index_Embedded_injEmbed t1 (LocalState_ι_uint256Index_Embedded_injEmbed t2 s) = LocalState_ι_uint256Index_Embedded_injEmbed t1 s.
+Proof.
+  intros.
+  destruct s.
+  repeat destruct p.
+  reflexivity.
+Defined.
+
+
+Global Instance LocalState_ι_uint256Index_Embedded : EmbeddedType LedgerLocalState (XHMap string nat) :=
+{
+  projEmbed := LocalState_ι_uint256Index_Embedded_projEmbed;
+	injEmbed := LocalState_ι_uint256Index_Embedded_injEmbed;
+  projinj := LocalState_ι_uint256Index_Embedded_projinj;
+  injproj := LocalState_ι_uint256Index_Embedded_injproj;
+  injinj := LocalState_ι_uint256Index_Embedded_injinj
+}.
+Definition  LocalState_ι_cellIndex_Embedded_projEmbed (l:LedgerLocalState ) : XHMap string nat := 
+  LocalState_ι_cellIndex l.
+
+Definition  LocalState_ι_cellIndex_Embedded_injEmbed (m: XHMap string nat) (l: LedgerLocalState) : LedgerLocalState := 
+  {$$ l with  LocalState_ι_cellIndex := m $$}.
+
+Print EmbeddedType.  
+
+Lemma LocalState_ι_cellIndex_Embedded_projinj : forall (t : XHMap string nat) (s : LedgerLocalState), LocalState_ι_cellIndex_Embedded_projEmbed (LocalState_ι_cellIndex_Embedded_injEmbed t s) = t.
+Proof.
+  intros.
+  destruct s.
+  repeat destruct p.
+  reflexivity.
+Defined.
+
+Lemma LocalState_ι_cellIndex_Embedded_injproj : forall s : LedgerLocalState, LocalState_ι_cellIndex_Embedded_injEmbed (LocalState_ι_cellIndex_Embedded_projEmbed s) s = s.
+Proof.
+  intros.
+  destruct s.
+  repeat destruct p.
+  reflexivity.
+Defined.  
+
+Lemma LocalState_ι_cellIndex_Embedded_injinj : forall (t1 t2 : XHMap string nat) (s : LedgerLocalState),
+LocalState_ι_cellIndex_Embedded_injEmbed t1 (LocalState_ι_cellIndex_Embedded_injEmbed t2 s) = LocalState_ι_cellIndex_Embedded_injEmbed t1 s.
+Proof.
+  intros.
+  destruct s.
+  repeat destruct p.
+  reflexivity.
+Defined.
+
+
+Global Instance LocalState_ι_cellIndex_Embedded : EmbeddedType LedgerLocalState (XHMap string nat) :=
+{
+  projEmbed := LocalState_ι_cellIndex_Embedded_projEmbed;
+	injEmbed := LocalState_ι_cellIndex_Embedded_injEmbed;
+  projinj := LocalState_ι_cellIndex_Embedded_projinj;
+  injproj := LocalState_ι_cellIndex_Embedded_injproj;
+  injinj := LocalState_ι_cellIndex_Embedded_injinj
+}.
+Definition  LocalState_ι_TonsConfigIndex_Embedded_projEmbed (l:LedgerLocalState ) : XHMap string nat := 
+  LocalState_ι_TonsConfigIndex l.
+
+Definition  LocalState_ι_TonsConfigIndex_Embedded_injEmbed (m: XHMap string nat) (l: LedgerLocalState) : LedgerLocalState := 
+  {$$ l with  LocalState_ι_TonsConfigIndex := m $$}.
+
+Print EmbeddedType.  
+
+Lemma LocalState_ι_TonsConfigIndex_Embedded_projinj : forall (t : XHMap string nat) (s : LedgerLocalState), LocalState_ι_TonsConfigIndex_Embedded_projEmbed (LocalState_ι_TonsConfigIndex_Embedded_injEmbed t s) = t.
+Proof.
+  intros.
+  destruct s.
+  repeat destruct p.
+  reflexivity.
+Defined.
+
+Lemma LocalState_ι_TonsConfigIndex_Embedded_injproj : forall s : LedgerLocalState, LocalState_ι_TonsConfigIndex_Embedded_injEmbed (LocalState_ι_TonsConfigIndex_Embedded_projEmbed s) s = s.
+Proof.
+  intros.
+  destruct s.
+  repeat destruct p.
+  reflexivity.
+Defined.  
+
+Lemma LocalState_ι_TonsConfigIndex_Embedded_injinj : forall (t1 t2 : XHMap string nat) (s : LedgerLocalState),
+LocalState_ι_TonsConfigIndex_Embedded_injEmbed t1 (LocalState_ι_TonsConfigIndex_Embedded_injEmbed t2 s) = LocalState_ι_TonsConfigIndex_Embedded_injEmbed t1 s.
+Proof.
+  intros.
+  destruct s.
+  repeat destruct p.
+  reflexivity.
+Defined.
+
+
+Global Instance LocalState_ι_TonsConfigIndex_Embedded : EmbeddedType LedgerLocalState (XHMap string nat) :=
+{
+  projEmbed := LocalState_ι_TonsConfigIndex_Embedded_projEmbed;
+	injEmbed := LocalState_ι_TonsConfigIndex_Embedded_injEmbed;
+  projinj := LocalState_ι_TonsConfigIndex_Embedded_projinj;
+  injproj := LocalState_ι_TonsConfigIndex_Embedded_injproj;
+  injinj := LocalState_ι_TonsConfigIndex_Embedded_injinj
+}.
+Definition  LocalState_ι_addressIndex_Embedded_projEmbed (l:LedgerLocalState ) : XHMap string nat := 
+  LocalState_ι_addressIndex l.
+
+Definition  LocalState_ι_addressIndex_Embedded_injEmbed (m: XHMap string nat) (l: LedgerLocalState) : LedgerLocalState := 
+  {$$ l with  LocalState_ι_addressIndex := m $$}.
+
+Print EmbeddedType.  
+
+Lemma LocalState_ι_addressIndex_Embedded_projinj : forall (t : XHMap string nat) (s : LedgerLocalState), LocalState_ι_addressIndex_Embedded_projEmbed (LocalState_ι_addressIndex_Embedded_injEmbed t s) = t.
+Proof.
+  intros.
+  destruct s.
+  repeat destruct p.
+  reflexivity.
+Defined.
+
+Lemma LocalState_ι_addressIndex_Embedded_injproj : forall s : LedgerLocalState, LocalState_ι_addressIndex_Embedded_injEmbed (LocalState_ι_addressIndex_Embedded_projEmbed s) s = s.
+Proof.
+  intros.
+  destruct s.
+  repeat destruct p.
+  reflexivity.
+Defined.  
+
+Lemma LocalState_ι_addressIndex_Embedded_injinj : forall (t1 t2 : XHMap string nat) (s : LedgerLocalState),
+LocalState_ι_addressIndex_Embedded_injEmbed t1 (LocalState_ι_addressIndex_Embedded_injEmbed t2 s) = LocalState_ι_addressIndex_Embedded_injEmbed t1 s.
+Proof.
+  intros.
+  destruct s.
+  repeat destruct p.
+  reflexivity.
+Defined.
+
+
+Global Instance LocalState_ι_addressIndex_Embedded : EmbeddedType LedgerLocalState (XHMap string nat) :=
+{
+  projEmbed := LocalState_ι_addressIndex_Embedded_projEmbed;
+	injEmbed := LocalState_ι_addressIndex_Embedded_injEmbed;
+  projinj := LocalState_ι_addressIndex_Embedded_projinj;
+  injproj := LocalState_ι_addressIndex_Embedded_injproj;
+  injinj := LocalState_ι_addressIndex_Embedded_injinj
+}.
+Definition  LocalState_ι_uint128Index_Embedded_projEmbed (l:LedgerLocalState ) : XHMap string nat := 
+  LocalState_ι_uint128Index l.
+
+Definition  LocalState_ι_uint128Index_Embedded_injEmbed (m: XHMap string nat) (l: LedgerLocalState) : LedgerLocalState := 
+  {$$ l with  LocalState_ι_uint128Index := m $$}.
+
+Print EmbeddedType.  
+
+Lemma LocalState_ι_uint128Index_Embedded_projinj : forall (t : XHMap string nat) (s : LedgerLocalState), LocalState_ι_uint128Index_Embedded_projEmbed (LocalState_ι_uint128Index_Embedded_injEmbed t s) = t.
+Proof.
+  intros.
+  destruct s.
+  repeat destruct p.
+  reflexivity.
+Defined.
+
+Lemma LocalState_ι_uint128Index_Embedded_injproj : forall s : LedgerLocalState, LocalState_ι_uint128Index_Embedded_injEmbed (LocalState_ι_uint128Index_Embedded_projEmbed s) s = s.
+Proof.
+  intros.
+  destruct s.
+  repeat destruct p.
+  reflexivity.
+Defined.  
+
+Lemma LocalState_ι_uint128Index_Embedded_injinj : forall (t1 t2 : XHMap string nat) (s : LedgerLocalState),
+LocalState_ι_uint128Index_Embedded_injEmbed t1 (LocalState_ι_uint128Index_Embedded_injEmbed t2 s) = LocalState_ι_uint128Index_Embedded_injEmbed t1 s.
+Proof.
+  intros.
+  destruct s.
+  repeat destruct p.
+  reflexivity.
+Defined.
+
+
+Global Instance LocalState_ι_uint128Index_Embedded : EmbeddedType LedgerLocalState (XHMap string nat) :=
+{
+  projEmbed := LocalState_ι_uint128Index_Embedded_projEmbed;
+	injEmbed := LocalState_ι_uint128Index_Embedded_injEmbed;
+  projinj := LocalState_ι_uint128Index_Embedded_projinj;
+  injproj := LocalState_ι_uint128Index_Embedded_injproj;
+  injinj := LocalState_ι_uint128Index_Embedded_injinj
+}.
+Definition  LocalState_ι_TradingPairIndex_Embedded_projEmbed (l:LedgerLocalState ) : XHMap string nat := 
+  LocalState_ι_TradingPairIndex l.
+
+Definition  LocalState_ι_TradingPairIndex_Embedded_injEmbed (m: XHMap string nat) (l: LedgerLocalState) : LedgerLocalState := 
+  {$$ l with  LocalState_ι_TradingPairIndex := m $$}.
+
+Print EmbeddedType.  
+
+Lemma LocalState_ι_TradingPairIndex_Embedded_projinj : forall (t : XHMap string nat) (s : LedgerLocalState), LocalState_ι_TradingPairIndex_Embedded_projEmbed (LocalState_ι_TradingPairIndex_Embedded_injEmbed t s) = t.
+Proof.
+  intros.
+  destruct s.
+  repeat destruct p.
+  reflexivity.
+Defined.
+
+Lemma LocalState_ι_TradingPairIndex_Embedded_injproj : forall s : LedgerLocalState, LocalState_ι_TradingPairIndex_Embedded_injEmbed (LocalState_ι_TradingPairIndex_Embedded_projEmbed s) s = s.
+Proof.
+  intros.
+  destruct s.
+  repeat destruct p.
+  reflexivity.
+Defined.  
+
+Lemma LocalState_ι_TradingPairIndex_Embedded_injinj : forall (t1 t2 : XHMap string nat) (s : LedgerLocalState),
+LocalState_ι_TradingPairIndex_Embedded_injEmbed t1 (LocalState_ι_TradingPairIndex_Embedded_injEmbed t2 s) = LocalState_ι_TradingPairIndex_Embedded_injEmbed t1 s.
+Proof.
+  intros.
+  destruct s.
+  repeat destruct p.
+  reflexivity.
+Defined.
+
+
+Global Instance LocalState_ι_TradingPairIndex_Embedded : EmbeddedType LedgerLocalState (XHMap string nat) :=
+{
+  projEmbed := LocalState_ι_TradingPairIndex_Embedded_projEmbed;
+	injEmbed := LocalState_ι_TradingPairIndex_Embedded_injEmbed;
+  projinj := LocalState_ι_TradingPairIndex_Embedded_projinj;
+  injproj := LocalState_ι_TradingPairIndex_Embedded_injproj;
+  injinj := LocalState_ι_TradingPairIndex_Embedded_injinj
+}.
+Definition  LocalState_ι_tplStateInituint256Index_Embedded_projEmbed (l:LedgerLocalState ) : XHMap string nat := 
+  LocalState_ι_tplStateInituint256Index l.
+
+Definition  LocalState_ι_tplStateInituint256Index_Embedded_injEmbed (m: XHMap string nat) (l: LedgerLocalState) : LedgerLocalState := 
+  {$$ l with  LocalState_ι_tplStateInituint256Index := m $$}.
+
+Print EmbeddedType.  
+
+Lemma LocalState_ι_tplStateInituint256Index_Embedded_projinj : forall (t : XHMap string nat) (s : LedgerLocalState), LocalState_ι_tplStateInituint256Index_Embedded_projEmbed (LocalState_ι_tplStateInituint256Index_Embedded_injEmbed t s) = t.
+Proof.
+  intros.
+  destruct s.
+  repeat destruct p.
+  reflexivity.
+Defined.
+
+Lemma LocalState_ι_tplStateInituint256Index_Embedded_injproj : forall s : LedgerLocalState, LocalState_ι_tplStateInituint256Index_Embedded_injEmbed (LocalState_ι_tplStateInituint256Index_Embedded_projEmbed s) s = s.
+Proof.
+  intros.
+  destruct s.
+  repeat destruct p.
+  reflexivity.
+Defined.  
+
+Lemma LocalState_ι_tplStateInituint256Index_Embedded_injinj : forall (t1 t2 : XHMap string nat) (s : LedgerLocalState),
+LocalState_ι_tplStateInituint256Index_Embedded_injEmbed t1 (LocalState_ι_tplStateInituint256Index_Embedded_injEmbed t2 s) = LocalState_ι_tplStateInituint256Index_Embedded_injEmbed t1 s.
+Proof.
+  intros.
+  destruct s.
+  repeat destruct p.
+  reflexivity.
+Defined.
+
+
+Global Instance LocalState_ι_tplStateInituint256Index_Embedded : EmbeddedType LedgerLocalState (XHMap string nat) :=
+{
+  projEmbed := LocalState_ι_tplStateInituint256Index_Embedded_projEmbed;
+	injEmbed := LocalState_ι_tplStateInituint256Index_Embedded_injEmbed;
+  projinj := LocalState_ι_tplStateInituint256Index_Embedded_projinj;
+  injproj := LocalState_ι_tplStateInituint256Index_Embedded_injproj;
+  injinj := LocalState_ι_tplStateInituint256Index_Embedded_injinj
+}.
+Definition  LocalState_ι_StateInitIndex_Embedded_projEmbed (l:LedgerLocalState ) : XHMap string nat := 
+  LocalState_ι_StateInitIndex l.
+
+Definition  LocalState_ι_StateInitIndex_Embedded_injEmbed (m: XHMap string nat) (l: LedgerLocalState) : LedgerLocalState := 
+  {$$ l with  LocalState_ι_StateInitIndex := m $$}.
+
+Print EmbeddedType.  
+
+Lemma LocalState_ι_StateInitIndex_Embedded_projinj : forall (t : XHMap string nat) (s : LedgerLocalState), LocalState_ι_StateInitIndex_Embedded_projEmbed (LocalState_ι_StateInitIndex_Embedded_injEmbed t s) = t.
+Proof.
+  intros.
+  destruct s.
+  repeat destruct p.
+  reflexivity.
+Defined.
+
+Lemma LocalState_ι_StateInitIndex_Embedded_injproj : forall s : LedgerLocalState, LocalState_ι_StateInitIndex_Embedded_injEmbed (LocalState_ι_StateInitIndex_Embedded_projEmbed s) s = s.
+Proof.
+  intros.
+  destruct s.
+  repeat destruct p.
+  reflexivity.
+Defined.  
+
+Lemma LocalState_ι_StateInitIndex_Embedded_injinj : forall (t1 t2 : XHMap string nat) (s : LedgerLocalState),
+LocalState_ι_StateInitIndex_Embedded_injEmbed t1 (LocalState_ι_StateInitIndex_Embedded_injEmbed t2 s) = LocalState_ι_StateInitIndex_Embedded_injEmbed t1 s.
+Proof.
+  intros.
+  destruct s.
+  repeat destruct p.
+  reflexivity.
+Defined.
+
+
+Global Instance LocalState_ι_StateInitIndex_Embedded : EmbeddedType LedgerLocalState (XHMap string nat) :=
+{
+  projEmbed := LocalState_ι_StateInitIndex_Embedded_projEmbed;
+	injEmbed := LocalState_ι_StateInitIndex_Embedded_injEmbed;
+  projinj := LocalState_ι_StateInitIndex_Embedded_projinj;
+  injproj := LocalState_ι_StateInitIndex_Embedded_injproj;
+  injinj := LocalState_ι_StateInitIndex_Embedded_injinj
+}.
+Definition  LocalState_ι_XchgPairIndex_Embedded_projEmbed (l:LedgerLocalState ) : XHMap string nat := 
+  LocalState_ι_XchgPairIndex l.
+
+Definition  LocalState_ι_XchgPairIndex_Embedded_injEmbed (m: XHMap string nat) (l: LedgerLocalState) : LedgerLocalState := 
+  {$$ l with  LocalState_ι_XchgPairIndex := m $$}.
+
+Print EmbeddedType.  
+
+Lemma LocalState_ι_XchgPairIndex_Embedded_projinj : forall (t : XHMap string nat) (s : LedgerLocalState), LocalState_ι_XchgPairIndex_Embedded_projEmbed (LocalState_ι_XchgPairIndex_Embedded_injEmbed t s) = t.
+Proof.
+  intros.
+  destruct s.
+  repeat destruct p.
+  reflexivity.
+Defined.
+
+Lemma LocalState_ι_XchgPairIndex_Embedded_injproj : forall s : LedgerLocalState, LocalState_ι_XchgPairIndex_Embedded_injEmbed (LocalState_ι_XchgPairIndex_Embedded_projEmbed s) s = s.
+Proof.
+  intros.
+  destruct s.
+  repeat destruct p.
+  reflexivity.
+Defined.  
+
+Lemma LocalState_ι_XchgPairIndex_Embedded_injinj : forall (t1 t2 : XHMap string nat) (s : LedgerLocalState),
+LocalState_ι_XchgPairIndex_Embedded_injEmbed t1 (LocalState_ι_XchgPairIndex_Embedded_injEmbed t2 s) = LocalState_ι_XchgPairIndex_Embedded_injEmbed t1 s.
+Proof.
+  intros.
+  destruct s.
+  repeat destruct p.
+  reflexivity.
+Defined.
+
+
+Global Instance LocalState_ι_XchgPairIndex_Embedded : EmbeddedType LedgerLocalState (XHMap string nat) :=
+{
+  projEmbed := LocalState_ι_XchgPairIndex_Embedded_projEmbed;
+	injEmbed := LocalState_ι_XchgPairIndex_Embedded_injEmbed;
+  projinj := LocalState_ι_XchgPairIndex_Embedded_projinj;
+  injproj := LocalState_ι_XchgPairIndex_Embedded_injproj;
+  injinj := LocalState_ι_XchgPairIndex_Embedded_injinj
+}.
+Definition  LocalState_ι_tplStateInitaddressIndex_Embedded_projEmbed (l:LedgerLocalState ) : XHMap string nat := 
+  LocalState_ι_tplStateInitaddressIndex l.
+
+Definition  LocalState_ι_tplStateInitaddressIndex_Embedded_injEmbed (m: XHMap string nat) (l: LedgerLocalState) : LedgerLocalState := 
+  {$$ l with  LocalState_ι_tplStateInitaddressIndex := m $$}.
+
+Print EmbeddedType.  
+
+Lemma LocalState_ι_tplStateInitaddressIndex_Embedded_projinj : forall (t : XHMap string nat) (s : LedgerLocalState), LocalState_ι_tplStateInitaddressIndex_Embedded_projEmbed (LocalState_ι_tplStateInitaddressIndex_Embedded_injEmbed t s) = t.
+Proof.
+  intros.
+  destruct s.
+  repeat destruct p.
+  reflexivity.
+Defined.
+
+Lemma LocalState_ι_tplStateInitaddressIndex_Embedded_injproj : forall s : LedgerLocalState, LocalState_ι_tplStateInitaddressIndex_Embedded_injEmbed (LocalState_ι_tplStateInitaddressIndex_Embedded_projEmbed s) s = s.
+Proof.
+  intros.
+  destruct s.
+  repeat destruct p.
+  reflexivity.
+Defined.  
+
+Lemma LocalState_ι_tplStateInitaddressIndex_Embedded_injinj : forall (t1 t2 : XHMap string nat) (s : LedgerLocalState),
+LocalState_ι_tplStateInitaddressIndex_Embedded_injEmbed t1 (LocalState_ι_tplStateInitaddressIndex_Embedded_injEmbed t2 s) = LocalState_ι_tplStateInitaddressIndex_Embedded_injEmbed t1 s.
+Proof.
+  intros.
+  destruct s.
+  repeat destruct p.
+  reflexivity.
+Defined.
+
+
+Global Instance LocalState_ι_tplStateInitaddressIndex_Embedded : EmbeddedType LedgerLocalState (XHMap string nat) :=
+{
+  projEmbed := LocalState_ι_tplStateInitaddressIndex_Embedded_projEmbed;
+	injEmbed := LocalState_ι_tplStateInitaddressIndex_Embedded_injEmbed;
+  projinj := LocalState_ι_tplStateInitaddressIndex_Embedded_projinj;
+  injproj := LocalState_ι_tplStateInitaddressIndex_Embedded_injproj;
+  injinj := LocalState_ι_tplStateInitaddressIndex_Embedded_injinj
+}.
+Definition  LocalState_ι_SellArgsIndex_Embedded_projEmbed (l:LedgerLocalState ) : XHMap string nat := 
+  LocalState_ι_SellArgsIndex l.
+
+Definition  LocalState_ι_SellArgsIndex_Embedded_injEmbed (m: XHMap string nat) (l: LedgerLocalState) : LedgerLocalState := 
+  {$$ l with  LocalState_ι_SellArgsIndex := m $$}.
+
+Print EmbeddedType.  
+
+Lemma LocalState_ι_SellArgsIndex_Embedded_projinj : forall (t : XHMap string nat) (s : LedgerLocalState), LocalState_ι_SellArgsIndex_Embedded_projEmbed (LocalState_ι_SellArgsIndex_Embedded_injEmbed t s) = t.
+Proof.
+  intros.
+  destruct s.
+  repeat destruct p.
+  reflexivity.
+Defined.
+
+Lemma LocalState_ι_SellArgsIndex_Embedded_injproj : forall s : LedgerLocalState, LocalState_ι_SellArgsIndex_Embedded_injEmbed (LocalState_ι_SellArgsIndex_Embedded_projEmbed s) s = s.
+Proof.
+  intros.
+  destruct s.
+  repeat destruct p.
+  reflexivity.
+Defined.  
+
+Lemma LocalState_ι_SellArgsIndex_Embedded_injinj : forall (t1 t2 : XHMap string nat) (s : LedgerLocalState),
+LocalState_ι_SellArgsIndex_Embedded_injEmbed t1 (LocalState_ι_SellArgsIndex_Embedded_injEmbed t2 s) = LocalState_ι_SellArgsIndex_Embedded_injEmbed t1 s.
+Proof.
+  intros.
+  destruct s.
+  repeat destruct p.
+  reflexivity.
+Defined.
+
+
+Global Instance LocalState_ι_SellArgsIndex_Embedded : EmbeddedType LedgerLocalState (XHMap string nat) :=
+{
+  projEmbed := LocalState_ι_SellArgsIndex_Embedded_projEmbed;
+	injEmbed := LocalState_ι_SellArgsIndex_Embedded_injEmbed;
+  projinj := LocalState_ι_SellArgsIndex_Embedded_projinj;
+  injproj := LocalState_ι_SellArgsIndex_Embedded_injproj;
+  injinj := LocalState_ι_SellArgsIndex_Embedded_injinj
+}.
+Definition  LocalState_ι_ITONTokenWalletPtrIndex_Embedded_projEmbed (l:LedgerLocalState ) : XHMap string nat := 
+  LocalState_ι_ITONTokenWalletPtrIndex l.
+
+Definition  LocalState_ι_ITONTokenWalletPtrIndex_Embedded_injEmbed (m: XHMap string nat) (l: LedgerLocalState) : LedgerLocalState := 
+  {$$ l with  LocalState_ι_ITONTokenWalletPtrIndex := m $$}.
+
+Print EmbeddedType.  
+
+Lemma LocalState_ι_ITONTokenWalletPtrIndex_Embedded_projinj : forall (t : XHMap string nat) (s : LedgerLocalState), LocalState_ι_ITONTokenWalletPtrIndex_Embedded_projEmbed (LocalState_ι_ITONTokenWalletPtrIndex_Embedded_injEmbed t s) = t.
+Proof.
+  intros.
+  destruct s.
+  repeat destruct p.
+  reflexivity.
+Defined.
+
+Lemma LocalState_ι_ITONTokenWalletPtrIndex_Embedded_injproj : forall s : LedgerLocalState, LocalState_ι_ITONTokenWalletPtrIndex_Embedded_injEmbed (LocalState_ι_ITONTokenWalletPtrIndex_Embedded_projEmbed s) s = s.
+Proof.
+  intros.
+  destruct s.
+  repeat destruct p.
+  reflexivity.
+Defined.  
+
+Lemma LocalState_ι_ITONTokenWalletPtrIndex_Embedded_injinj : forall (t1 t2 : XHMap string nat) (s : LedgerLocalState),
+LocalState_ι_ITONTokenWalletPtrIndex_Embedded_injEmbed t1 (LocalState_ι_ITONTokenWalletPtrIndex_Embedded_injEmbed t2 s) = LocalState_ι_ITONTokenWalletPtrIndex_Embedded_injEmbed t1 s.
+Proof.
+  intros.
+  destruct s.
+  repeat destruct p.
+  reflexivity.
+Defined.
+
+
+Global Instance LocalState_ι_ITONTokenWalletPtrIndex_Embedded : EmbeddedType LedgerLocalState (XHMap string nat) :=
+{
+  projEmbed := LocalState_ι_ITONTokenWalletPtrIndex_Embedded_projEmbed;
+	injEmbed := LocalState_ι_ITONTokenWalletPtrIndex_Embedded_injEmbed;
+  projinj := LocalState_ι_ITONTokenWalletPtrIndex_Embedded_projinj;
+  injproj := LocalState_ι_ITONTokenWalletPtrIndex_Embedded_injproj;
+  injinj := LocalState_ι_ITONTokenWalletPtrIndex_Embedded_injinj
+}.
+Definition  LocalState_ι_IPricePtrIndex_Embedded_projEmbed (l:LedgerLocalState ) : XHMap string nat := 
+  LocalState_ι_IPricePtrIndex l.
+
+Definition  LocalState_ι_IPricePtrIndex_Embedded_injEmbed (m: XHMap string nat) (l: LedgerLocalState) : LedgerLocalState := 
+  {$$ l with  LocalState_ι_IPricePtrIndex := m $$}.
+
+Print EmbeddedType.  
+
+Lemma LocalState_ι_IPricePtrIndex_Embedded_projinj : forall (t : XHMap string nat) (s : LedgerLocalState), LocalState_ι_IPricePtrIndex_Embedded_projEmbed (LocalState_ι_IPricePtrIndex_Embedded_injEmbed t s) = t.
+Proof.
+  intros.
+  destruct s.
+  repeat destruct p.
+  reflexivity.
+Defined.
+
+Lemma LocalState_ι_IPricePtrIndex_Embedded_injproj : forall s : LedgerLocalState, LocalState_ι_IPricePtrIndex_Embedded_injEmbed (LocalState_ι_IPricePtrIndex_Embedded_projEmbed s) s = s.
+Proof.
+  intros.
+  destruct s.
+  repeat destruct p.
+  reflexivity.
+Defined.  
+
+Lemma LocalState_ι_IPricePtrIndex_Embedded_injinj : forall (t1 t2 : XHMap string nat) (s : LedgerLocalState),
+LocalState_ι_IPricePtrIndex_Embedded_injEmbed t1 (LocalState_ι_IPricePtrIndex_Embedded_injEmbed t2 s) = LocalState_ι_IPricePtrIndex_Embedded_injEmbed t1 s.
+Proof.
+  intros.
+  destruct s.
+  repeat destruct p.
+  reflexivity.
+Defined.
+
+
+Global Instance LocalState_ι_IPricePtrIndex_Embedded : EmbeddedType LedgerLocalState (XHMap string nat) :=
+{
+  projEmbed := LocalState_ι_IPricePtrIndex_Embedded_projEmbed;
+	injEmbed := LocalState_ι_IPricePtrIndex_Embedded_injEmbed;
+  projinj := LocalState_ι_IPricePtrIndex_Embedded_projinj;
+  injproj := LocalState_ι_IPricePtrIndex_Embedded_injproj;
+  injinj := LocalState_ι_IPricePtrIndex_Embedded_injinj
+}.
+Definition  LocalState_ι_intIndex_Embedded_projEmbed (l:LedgerLocalState ) : XHMap string nat := 
+  LocalState_ι_intIndex l.
+
+Definition  LocalState_ι_intIndex_Embedded_injEmbed (m: XHMap string nat) (l: LedgerLocalState) : LedgerLocalState := 
+  {$$ l with  LocalState_ι_intIndex := m $$}.
+
+Print EmbeddedType.  
+
+Lemma LocalState_ι_intIndex_Embedded_projinj : forall (t : XHMap string nat) (s : LedgerLocalState), LocalState_ι_intIndex_Embedded_projEmbed (LocalState_ι_intIndex_Embedded_injEmbed t s) = t.
+Proof.
+  intros.
+  destruct s.
+  repeat destruct p.
+  reflexivity.
+Defined.
+
+Lemma LocalState_ι_intIndex_Embedded_injproj : forall s : LedgerLocalState, LocalState_ι_intIndex_Embedded_injEmbed (LocalState_ι_intIndex_Embedded_projEmbed s) s = s.
+Proof.
+  intros.
+  destruct s.
+  repeat destruct p.
+  reflexivity.
+Defined.  
+
+Lemma LocalState_ι_intIndex_Embedded_injinj : forall (t1 t2 : XHMap string nat) (s : LedgerLocalState),
+LocalState_ι_intIndex_Embedded_injEmbed t1 (LocalState_ι_intIndex_Embedded_injEmbed t2 s) = LocalState_ι_intIndex_Embedded_injEmbed t1 s.
+Proof.
+  intros.
+  destruct s.
+  repeat destruct p.
+  reflexivity.
+Defined.
+
+
+Global Instance LocalState_ι_intIndex_Embedded : EmbeddedType LedgerLocalState (XHMap string nat) :=
+{
+  projEmbed := LocalState_ι_intIndex_Embedded_projEmbed;
+	injEmbed := LocalState_ι_intIndex_Embedded_injEmbed;
+  projinj := LocalState_ι_intIndex_Embedded_projinj;
+  injproj := LocalState_ι_intIndex_Embedded_injproj;
+  injinj := LocalState_ι_intIndex_Embedded_injinj
+}.
+Definition  LocalState_ι_PriceIndex_Embedded_projEmbed (l:LedgerLocalState ) : XHMap string nat := 
+  LocalState_ι_PriceIndex l.
+
+Definition  LocalState_ι_PriceIndex_Embedded_injEmbed (m: XHMap string nat) (l: LedgerLocalState) : LedgerLocalState := 
+  {$$ l with  LocalState_ι_PriceIndex := m $$}.
+
+Print EmbeddedType.  
+
+Lemma LocalState_ι_PriceIndex_Embedded_projinj : forall (t : XHMap string nat) (s : LedgerLocalState), LocalState_ι_PriceIndex_Embedded_projEmbed (LocalState_ι_PriceIndex_Embedded_injEmbed t s) = t.
+Proof.
+  intros.
+  destruct s.
+  repeat destruct p.
+  reflexivity.
+Defined.
+
+Lemma LocalState_ι_PriceIndex_Embedded_injproj : forall s : LedgerLocalState, LocalState_ι_PriceIndex_Embedded_injEmbed (LocalState_ι_PriceIndex_Embedded_projEmbed s) s = s.
+Proof.
+  intros.
+  destruct s.
+  repeat destruct p.
+  reflexivity.
+Defined.  
+
+Lemma LocalState_ι_PriceIndex_Embedded_injinj : forall (t1 t2 : XHMap string nat) (s : LedgerLocalState),
+LocalState_ι_PriceIndex_Embedded_injEmbed t1 (LocalState_ι_PriceIndex_Embedded_injEmbed t2 s) = LocalState_ι_PriceIndex_Embedded_injEmbed t1 s.
+Proof.
+  intros.
+  destruct s.
+  repeat destruct p.
+  reflexivity.
+Defined.
+
+
+Global Instance LocalState_ι_PriceIndex_Embedded : EmbeddedType LedgerLocalState (XHMap string nat) :=
+{
+  projEmbed := LocalState_ι_PriceIndex_Embedded_projEmbed;
+	injEmbed := LocalState_ι_PriceIndex_Embedded_injEmbed;
+  projinj := LocalState_ι_PriceIndex_Embedded_projinj;
+  injproj := LocalState_ι_PriceIndex_Embedded_injproj;
+  injinj := LocalState_ι_PriceIndex_Embedded_injinj
+}.
+Definition  LocalState_ι_uint8Index_Embedded_projEmbed (l:LedgerLocalState ) : XHMap string nat := 
+  LocalState_ι_uint8Index l.
+
+Definition  LocalState_ι_uint8Index_Embedded_injEmbed (m: XHMap string nat) (l: LedgerLocalState) : LedgerLocalState := 
+  {$$ l with  LocalState_ι_uint8Index := m $$}.
+
+Print EmbeddedType.  
+
+Lemma LocalState_ι_uint8Index_Embedded_projinj : forall (t : XHMap string nat) (s : LedgerLocalState), LocalState_ι_uint8Index_Embedded_projEmbed (LocalState_ι_uint8Index_Embedded_injEmbed t s) = t.
+Proof.
+  intros.
+  destruct s.
+  repeat destruct p.
+  reflexivity.
+Defined.
+
+Lemma LocalState_ι_uint8Index_Embedded_injproj : forall s : LedgerLocalState, LocalState_ι_uint8Index_Embedded_injEmbed (LocalState_ι_uint8Index_Embedded_projEmbed s) s = s.
+Proof.
+  intros.
+  destruct s.
+  repeat destruct p.
+  reflexivity.
+Defined.  
+
+Lemma LocalState_ι_uint8Index_Embedded_injinj : forall (t1 t2 : XHMap string nat) (s : LedgerLocalState),
+LocalState_ι_uint8Index_Embedded_injEmbed t1 (LocalState_ι_uint8Index_Embedded_injEmbed t2 s) = LocalState_ι_uint8Index_Embedded_injEmbed t1 s.
+Proof.
+  intros.
+  destruct s.
+  repeat destruct p.
+  reflexivity.
+Defined.
+
+
+Global Instance LocalState_ι_uint8Index_Embedded : EmbeddedType LedgerLocalState (XHMap string nat) :=
+{
+  projEmbed := LocalState_ι_uint8Index_Embedded_projEmbed;
+	injEmbed := LocalState_ι_uint8Index_Embedded_injEmbed;
+  projinj := LocalState_ι_uint8Index_Embedded_projinj;
+  injproj := LocalState_ι_uint8Index_Embedded_injproj;
+  injinj := LocalState_ι_uint8Index_Embedded_injinj
+}.
+Definition  LocalState_ι_uint32Index_Embedded_projEmbed (l:LedgerLocalState ) : XHMap string nat := 
+  LocalState_ι_uint32Index l.
+
+Definition  LocalState_ι_uint32Index_Embedded_injEmbed (m: XHMap string nat) (l: LedgerLocalState) : LedgerLocalState := 
+  {$$ l with  LocalState_ι_uint32Index := m $$}.
+
+Print EmbeddedType.  
+
+Lemma LocalState_ι_uint32Index_Embedded_projinj : forall (t : XHMap string nat) (s : LedgerLocalState), LocalState_ι_uint32Index_Embedded_projEmbed (LocalState_ι_uint32Index_Embedded_injEmbed t s) = t.
+Proof.
+  intros.
+  destruct s.
+  repeat destruct p.
+  reflexivity.
+Defined.
+
+Lemma LocalState_ι_uint32Index_Embedded_injproj : forall s : LedgerLocalState, LocalState_ι_uint32Index_Embedded_injEmbed (LocalState_ι_uint32Index_Embedded_projEmbed s) s = s.
+Proof.
+  intros.
+  destruct s.
+  repeat destruct p.
+  reflexivity.
+Defined.  
+
+Lemma LocalState_ι_uint32Index_Embedded_injinj : forall (t1 t2 : XHMap string nat) (s : LedgerLocalState),
+LocalState_ι_uint32Index_Embedded_injEmbed t1 (LocalState_ι_uint32Index_Embedded_injEmbed t2 s) = LocalState_ι_uint32Index_Embedded_injEmbed t1 s.
+Proof.
+  intros.
+  destruct s.
+  repeat destruct p.
+  reflexivity.
+Defined.
+
+
+Global Instance LocalState_ι_uint32Index_Embedded : EmbeddedType LedgerLocalState (XHMap string nat) :=
+{
+  projEmbed := LocalState_ι_uint32Index_Embedded_projEmbed;
+	injEmbed := LocalState_ι_uint32Index_Embedded_injEmbed;
+  projinj := LocalState_ι_uint32Index_Embedded_projinj;
+  injproj := LocalState_ι_uint32Index_Embedded_injproj;
+  injinj := LocalState_ι_uint32Index_Embedded_injinj
+}.
+Definition  LocalState_ι_Tip3ConfigIndex_Embedded_projEmbed (l:LedgerLocalState ) : XHMap string nat := 
+  LocalState_ι_Tip3ConfigIndex l.
+
+Definition  LocalState_ι_Tip3ConfigIndex_Embedded_injEmbed (m: XHMap string nat) (l: LedgerLocalState) : LedgerLocalState := 
+  {$$ l with  LocalState_ι_Tip3ConfigIndex := m $$}.
+
+Print EmbeddedType.  
+
+Lemma LocalState_ι_Tip3ConfigIndex_Embedded_projinj : forall (t : XHMap string nat) (s : LedgerLocalState), LocalState_ι_Tip3ConfigIndex_Embedded_projEmbed (LocalState_ι_Tip3ConfigIndex_Embedded_injEmbed t s) = t.
+Proof.
+  intros.
+  destruct s.
+  repeat destruct p.
+  reflexivity.
+Defined.
+
+Lemma LocalState_ι_Tip3ConfigIndex_Embedded_injproj : forall s : LedgerLocalState, LocalState_ι_Tip3ConfigIndex_Embedded_injEmbed (LocalState_ι_Tip3ConfigIndex_Embedded_projEmbed s) s = s.
+Proof.
+  intros.
+  destruct s.
+  repeat destruct p.
+  reflexivity.
+Defined.  
+
+Lemma LocalState_ι_Tip3ConfigIndex_Embedded_injinj : forall (t1 t2 : XHMap string nat) (s : LedgerLocalState),
+LocalState_ι_Tip3ConfigIndex_Embedded_injEmbed t1 (LocalState_ι_Tip3ConfigIndex_Embedded_injEmbed t2 s) = LocalState_ι_Tip3ConfigIndex_Embedded_injEmbed t1 s.
+Proof.
+  intros.
+  destruct s.
+  repeat destruct p.
+  reflexivity.
+Defined.
+
+
+Global Instance LocalState_ι_Tip3ConfigIndex_Embedded : EmbeddedType LedgerLocalState (XHMap string nat) :=
+{
+  projEmbed := LocalState_ι_Tip3ConfigIndex_Embedded_projEmbed;
+	injEmbed := LocalState_ι_Tip3ConfigIndex_Embedded_injEmbed;
+  projinj := LocalState_ι_Tip3ConfigIndex_Embedded_projinj;
+  injproj := LocalState_ι_Tip3ConfigIndex_Embedded_injproj;
+  injinj := LocalState_ι_Tip3ConfigIndex_Embedded_injinj
+}.
+Definition  LocalState_ι_PriceXchgIndex_Embedded_projEmbed (l:LedgerLocalState ) : XHMap string nat := 
+  LocalState_ι_PriceXchgIndex l.
+
+Definition  LocalState_ι_PriceXchgIndex_Embedded_injEmbed (m: XHMap string nat) (l: LedgerLocalState) : LedgerLocalState := 
+  {$$ l with  LocalState_ι_PriceXchgIndex := m $$}.
+
+Print EmbeddedType.  
+
+Lemma LocalState_ι_PriceXchgIndex_Embedded_projinj : forall (t : XHMap string nat) (s : LedgerLocalState), LocalState_ι_PriceXchgIndex_Embedded_projEmbed (LocalState_ι_PriceXchgIndex_Embedded_injEmbed t s) = t.
+Proof.
+  intros.
+  destruct s.
+  repeat destruct p.
+  reflexivity.
+Defined.
+
+Lemma LocalState_ι_PriceXchgIndex_Embedded_injproj : forall s : LedgerLocalState, LocalState_ι_PriceXchgIndex_Embedded_injEmbed (LocalState_ι_PriceXchgIndex_Embedded_projEmbed s) s = s.
+Proof.
+  intros.
+  destruct s.
+  repeat destruct p.
+  reflexivity.
+Defined.  
+
+Lemma LocalState_ι_PriceXchgIndex_Embedded_injinj : forall (t1 t2 : XHMap string nat) (s : LedgerLocalState),
+LocalState_ι_PriceXchgIndex_Embedded_injEmbed t1 (LocalState_ι_PriceXchgIndex_Embedded_injEmbed t2 s) = LocalState_ι_PriceXchgIndex_Embedded_injEmbed t1 s.
+Proof.
+  intros.
+  destruct s.
+  repeat destruct p.
+  reflexivity.
+Defined.
+
+
+Global Instance LocalState_ι_PriceXchgIndex_Embedded : EmbeddedType LedgerLocalState (XHMap string nat) :=
+{
+  projEmbed := LocalState_ι_PriceXchgIndex_Embedded_projEmbed;
+	injEmbed := LocalState_ι_PriceXchgIndex_Embedded_injEmbed;
+  projinj := LocalState_ι_PriceXchgIndex_Embedded_projinj;
+  injproj := LocalState_ι_PriceXchgIndex_Embedded_injproj;
+  injinj := LocalState_ι_PriceXchgIndex_Embedded_injinj
+}.
+Definition  LocalState_ι_PayloadArgsIndex_Embedded_projEmbed (l:LedgerLocalState ) : XHMap string nat := 
+  LocalState_ι_PayloadArgsIndex l.
+
+Definition  LocalState_ι_PayloadArgsIndex_Embedded_injEmbed (m: XHMap string nat) (l: LedgerLocalState) : LedgerLocalState := 
+  {$$ l with  LocalState_ι_PayloadArgsIndex := m $$}.
+
+Print EmbeddedType.  
+
+Lemma LocalState_ι_PayloadArgsIndex_Embedded_projinj : forall (t : XHMap string nat) (s : LedgerLocalState), LocalState_ι_PayloadArgsIndex_Embedded_projEmbed (LocalState_ι_PayloadArgsIndex_Embedded_injEmbed t s) = t.
+Proof.
+  intros.
+  destruct s.
+  repeat destruct p.
+  reflexivity.
+Defined.
+
+Lemma LocalState_ι_PayloadArgsIndex_Embedded_injproj : forall s : LedgerLocalState, LocalState_ι_PayloadArgsIndex_Embedded_injEmbed (LocalState_ι_PayloadArgsIndex_Embedded_projEmbed s) s = s.
+Proof.
+  intros.
+  destruct s.
+  repeat destruct p.
+  reflexivity.
+Defined.  
+
+Lemma LocalState_ι_PayloadArgsIndex_Embedded_injinj : forall (t1 t2 : XHMap string nat) (s : LedgerLocalState),
+LocalState_ι_PayloadArgsIndex_Embedded_injEmbed t1 (LocalState_ι_PayloadArgsIndex_Embedded_injEmbed t2 s) = LocalState_ι_PayloadArgsIndex_Embedded_injEmbed t1 s.
+Proof.
+  intros.
+  destruct s.
+  repeat destruct p.
+  reflexivity.
+Defined.
+
+
+Global Instance LocalState_ι_PayloadArgsIndex_Embedded : EmbeddedType LedgerLocalState (XHMap string nat) :=
+{
+  projEmbed := LocalState_ι_PayloadArgsIndex_Embedded_projEmbed;
+	injEmbed := LocalState_ι_PayloadArgsIndex_Embedded_injEmbed;
+  projinj := LocalState_ι_PayloadArgsIndex_Embedded_projinj;
+  injproj := LocalState_ι_PayloadArgsIndex_Embedded_injproj;
+  injinj := LocalState_ι_PayloadArgsIndex_Embedded_injinj
+}.
+(****************************************************************************)
+
+Global Instance LocalState_uint256Index: LocalStateField XInteger256 :=
+{
+  local_index_embedded := LocalState_ι_uint256Index_Embedded;
+  local_state_field := LocalState_ι_uint256; 
+  local_field_type_correct := eq_refl
+}.
+
+ 
+ 
+Global Instance LocalState_cellIndex: LocalStateField TvmCell :=
+{
+  local_index_embedded := LocalState_ι_cellIndex_Embedded;
+  local_state_field := LocalState_ι_cell; 
+  local_field_type_correct := eq_refl
+}.
+
+ 
+ 
+Global Instance LocalState_TonsConfigIndex: LocalStateField TonsConfig :=
+{
+  local_index_embedded := LocalState_ι_TonsConfigIndex_Embedded;
+  local_state_field := LocalState_ι_TonsConfig; 
+  local_field_type_correct := eq_refl
+}.
+
+ 
+ 
+Global Instance LocalState_addressIndex: LocalStateField XAddress :=
+{
+  local_index_embedded := LocalState_ι_addressIndex_Embedded;
+  local_state_field := LocalState_ι_address; 
+  local_field_type_correct := eq_refl
+}.
+
+ 
+ 
+Global Instance LocalState_uint128Index: LocalStateField XInteger128 :=
+{
+  local_index_embedded := LocalState_ι_uint128Index_Embedded;
+  local_state_field := LocalState_ι_uint128; 
+  local_field_type_correct := eq_refl
+}.
+
+ 
+ 
+Global Instance LocalState_TradingPairIndex: LocalStateField TradingPair :=
+{
+  local_index_embedded := LocalState_ι_TradingPairIndex_Embedded;
+  local_state_field := LocalState_ι_TradingPair; 
+  local_field_type_correct := eq_refl
+}.
+
+ 
+ 
+Global Instance LocalState_tplStateInituint256Index: LocalStateField ( StateInit * XInteger256 ) :=
+{
+  local_index_embedded := LocalState_ι_tplStateInituint256Index_Embedded;
+  local_state_field := LocalState_ι_tplStateInituint256; 
+  local_field_type_correct := eq_refl
+}.
+
+ 
+ 
+Global Instance LocalState_StateInitIndex: LocalStateField StateInit :=
+{
+  local_index_embedded := LocalState_ι_StateInitIndex_Embedded;
+  local_state_field := LocalState_ι_StateInit; 
+  local_field_type_correct := eq_refl
+}.
+
+ 
+ 
+Global Instance LocalState_XchgPairIndex: LocalStateField XchgPair :=
+{
+  local_index_embedded := LocalState_ι_XchgPairIndex_Embedded;
+  local_state_field := LocalState_ι_XchgPair; 
+  local_field_type_correct := eq_refl
+}.
+
+ 
+ 
+Global Instance LocalState_tplStateInitaddressIndex: LocalStateField ( StateInit * XAddress * XInteger256 ) :=
+{
+  local_index_embedded := LocalState_ι_tplStateInitaddressIndex_Embedded;
+  local_state_field := LocalState_ι_tplStateInitaddress; 
+  local_field_type_correct := eq_refl
+}.
+
+ 
+ 
+Global Instance LocalState_SellArgsIndex: LocalStateField SellArgs :=
+{
+  local_index_embedded := LocalState_ι_SellArgsIndex_Embedded;
+  local_state_field := LocalState_ι_SellArgs; 
+  local_field_type_correct := eq_refl
+}.
+
+ 
+ 
+Global Instance LocalState_ITONTokenWalletPtrIndex: LocalStateField ITONTokenWalletPtr :=
+{
+  local_index_embedded := LocalState_ι_ITONTokenWalletPtrIndex_Embedded;
+  local_state_field := LocalState_ι_ITONTokenWalletPtr; 
+  local_field_type_correct := eq_refl
+}.
+
+ 
+ 
+Global Instance LocalState_IPricePtrIndex: LocalStateField IPricePtr :=
+{
+  local_index_embedded := LocalState_ι_IPricePtrIndex_Embedded;
+  local_state_field := LocalState_ι_IPricePtr; 
+  local_field_type_correct := eq_refl
+}.
+
+ 
+ 
+Global Instance LocalState_intIndex: LocalStateField XInteger :=
+{
+  local_index_embedded := LocalState_ι_intIndex_Embedded;
+  local_state_field := LocalState_ι_int; 
+  local_field_type_correct := eq_refl
+}.
+
+ 
+ 
+Global Instance LocalState_PriceIndex: LocalStateField Price :=
+{
+  local_index_embedded := LocalState_ι_PriceIndex_Embedded;
+  local_state_field := LocalState_ι_Price; 
+  local_field_type_correct := eq_refl
+}.
+
+ 
+ 
+Global Instance LocalState_uint8Index: LocalStateField XInteger8 :=
+{
+  local_index_embedded := LocalState_ι_uint8Index_Embedded;
+  local_state_field := LocalState_ι_uint8; 
+  local_field_type_correct := eq_refl
+}.
+
+ 
+ 
+Global Instance LocalState_uint32Index: LocalStateField XInteger32 :=
+{
+  local_index_embedded := LocalState_ι_uint32Index_Embedded;
+  local_state_field := LocalState_ι_uint32; 
+  local_field_type_correct := eq_refl
+}.
+
+ 
+ 
+Global Instance LocalState_Tip3ConfigIndex: LocalStateField Tip3Config :=
+{
+  local_index_embedded := LocalState_ι_Tip3ConfigIndex_Embedded;
+  local_state_field := LocalState_ι_Tip3Config; 
+  local_field_type_correct := eq_refl
+}.
+
+ 
+ 
+Global Instance LocalState_PriceXchgIndex: LocalStateField PriceXchg :=
+{
+  local_index_embedded := LocalState_ι_PriceXchgIndex_Embedded;
+  local_state_field := LocalState_ι_PriceXchg; 
+  local_field_type_correct := eq_refl
+}.
+
+ 
+ 
+Global Instance LocalState_PayloadArgsIndex: LocalStateField PayloadArgs :=
+{
+  local_index_embedded := LocalState_ι_PayloadArgsIndex_Embedded;
+  local_state_field := LocalState_ι_PayloadArgs; 
+  local_field_type_correct := eq_refl
+}.
+
+ 
+
+Definition LedgerVMStateEmbedded := embeddedT2. 
+Definition LedgerVMStateField := Ledger_ι_VMState .
+Definition isoVMState := iso_T2.
+
+End LedgerClass .
